@prefix skos: <http://www.w3.org/2004/02/skos/core#> .
@prefix rdfs: <http://www.w3.org/2000/01/rdf-schema#> .
@prefix dct: <http://purl.org/dc/terms/> .

@prefix aphia-trait: <https://aphia.org/ns/attribute-trait/> .

@prefix trait: <https://aphia.org/ns/vocab/attribute-trait/> .

trait:conceptScheme
    a skos:ConceptScheme ;
    rdfs:label "Listing Aphia attributes and traits"@en .

<https://aphia.org/ns/vocab/attribute-trait/>
    a skos:Collection ;
    rdfs:label "Aphia attributes and traits"@en ;
    
    skos:member trait:societal_importance ;
.

trait:ambi_ecological_group
    a skos:Collection ; 
    dct:description "AZTIâ€™s Marine Biotic Index ecological group"@en ;

    skos:member trait:very_sensitive_to_disturbance , trait:indifferent_to_disturbance , trait:tolerant_to_disturbance , trait:second_order_opportunistic , trait:first_order_opportunistic ; 
.

trait:very_sensitive_to_disturbance
    a skos:Concept, aphia-trait:Trait ;
    skos:inScheme trait:conceptScheme ;
    skos:prefLabel "Very sensitive to disturbance"@en ;
    skos:definition "Species very sensitive to disturbance and present under undisturbed conditions (they are present in mature systems)."@en ;
.

trait:indifferent_to_disturbance
    a skos:Concept, aphia-trait:Trait ;
    skos:inScheme trait:conceptScheme ;
    skos:prefLabel "Indifferent to disturbance"@en ;
    skos:definition "Species indifferent to disturbance, always present in low densities with non-significant variations with time (they are present in mature systems and slight unbalanced)."@en ;
.

trait:tolerant_to_disturbance
    a skos:Concept, aphia-trait:Trait ;
    skos:inScheme trait:conceptScheme ;
    skos:prefLabel "Tolerant to disturbance"@en ;
    skos:definition "Species tolerant to disturbance. These species may occur under normal conditions (e.g. in naturally disturbed or enriched conditions, such as estuaries), but their populations are stimulated by some disturbances, such as organic enrichment (present in slight unbalanced situations)."@en ;
.

trait:second_order_opportunistic
    a skos:Concept, aphia-trait:Trait ;
    skos:inScheme trait:conceptScheme ;
    skos:prefLabel "Second-order opportunistic"@en ;
    skos:definition "Second-order opportunistic species, able to resist some periods of low oxygen levels, and some concentration of pollutants (present in slight to pronounced unbalanced situations)."@en ;
.

trait:first_order_opportunistic
    a skos:Concept, aphia-trait:Trait ;
    skos:inScheme trait:conceptScheme ;
    skos:prefLabel "First-order opportunistic"@en ;
    skos:definition "First-order opportunistic species, able to resist very low oxygen levels, episodes of anoxia and high concentration of pollutants, early and successful pioneers (present in pronounced unbalanced situations)."@en ;
.