@prefix skos: <http://www.w3.org/2004/02/skos/core#> .
@prefix rdfs: <http://www.w3.org/2000/01/rdf-schema#> .
@prefix dct: <http://purl.org/dc/terms/> .

@prefix aphia-trait: <https://aphia.org/ns/attribute-trait/> .

@prefix trait: <https://aphia.org/ns/vocab/attribute-trait/> .


trait:body_size_dimension
    a skos:Collection ; 
    dct:description "The dimension of a body size (e.g. length, width, diameter)."@en ;

    skos:member trait:length , 
                trait:width , 
                trait:diameter , 
                trait:height , 
                trait:thickness , 
                trait:wingspan , 
                trait:volume , 
                trait:corresponding_length , 
                trait:corresponding_width , 
                trait:thallus_length , 
                trait:thallus_diameter , 
                trait:weight , 
                trait:corresponding_weight , 
                trait:standard_length , 
                trait:total_length , 
                trait:fork_length , 
                trait:width_of_disk , 
                trait:prosome_length , 
                trait:patch_diameter ;
.

trait:length
    a skos:Concept, aphia-trait:Trait ;
    skos:inScheme trait:conceptScheme ;
    skos:prefLabel "Length"@en ;
    skos:definition "Maximum recorded linear body length (in millimetres) excluding appendages. [Source: https://marinespecies.org/traits/wiki/Traits:Bodylength]"@en ;

    skos:closeMatch ... ; 
.

trait:width
    a skos:Concept, aphia-trait:Trait ;
    skos:inScheme trait:conceptScheme ;
    skos:prefLabel "Width"@en ;
    skos:definition "A measurement or extent of something from side to side; the lesser of two or the least of three dimensions of a body. [Source: https://marinespecies.org/traits/wiki/Traits:Width]"@en ;

    skos:closeMatch ... ; 
.

trait:diameter
    a skos:Concept, aphia-trait:Trait ;
    skos:inScheme trait:conceptScheme ;
    skos:prefLabel "Diameter"@en ;
    skos:definition "The length of a straight line passing from side to side through the centre of a body or figure, especially a circle or sphere."@en ;

    skos:closeMatch ... ; 
.

trait:height
    a skos:Concept, aphia-trait:Trait ;
    skos:inScheme trait:conceptScheme ;
    skos:prefLabel "Height"@en ;
    skos:definition ""@en ;

    skos:closeMatch ... ; 
.

trait:thickness
    a skos:Concept, aphia-trait:Trait ;
    skos:inScheme trait:conceptScheme ;
    skos:prefLabel "Thickness"@en ;
    skos:definition ""@en ;

    skos:exactMatch ... ; 
.

trait:wingspan
    a skos:Concept, aphia-trait:Trait ;
    skos:inScheme trait:conceptScheme ;
    skos:prefLabel "Wingspan"@en ;
    skos:definition "The distance between the wing tips when the wings are held outstretched."@en ;
.

trait:volume
    a skos:Concept, aphia-trait:Trait ;
    skos:inScheme trait:conceptScheme ;
    skos:prefLabel "Volume"@en ;
    skos:definition ""@en ;

    skos:closeMatch ... ; 
.

trait:corresponding_length
    a skos:Concept, aphia-trait:Trait ;
    skos:inScheme trait:conceptScheme ;
    skos:prefLabel "Corresponding length"@en ;
    skos:definition "Corresponding length of a length-width pair for Nematoda."@en ;
.

trait:corresponding_width
    a skos:Concept, aphia-trait:Trait ;
    skos:inScheme trait:conceptScheme ;
    skos:prefLabel "Corresponding width"@en ;
    skos:definition "Corresponding width of a length-width pair for Nematoda."@en ;
.

trait:thallus_length
    a skos:Concept, aphia-trait:Trait ;
    skos:inScheme trait:conceptScheme ;
    skos:prefLabel "Thallus length"@en ;
    skos:definition "Maximum length observed for the regarding thallus feature."@en ;

    skos:exactMatch ... ; 
.

trait:thallus_diameter
    a skos:Concept, aphia-trait:Trait ;
    skos:inScheme trait:conceptScheme ;
    skos:prefLabel "Thallus diameter"@en ;
    skos:definition "Maximum diameter observed for the regarding thallus feature."@en ;

    skos:exactMatch ... ; 
.

trait:weight
    a skos:Concept, aphia-trait:Trait ;
    skos:inScheme trait:conceptScheme ;
    skos:prefLabel "Weight"@en ;
    skos:definition ""@en ;

    skos:closeMatch ... ; 
.

trait:corresponding_weight
    a skos:Concept, aphia-trait:Trait ;
    skos:inScheme trait:conceptScheme ;
    skos:prefLabel "Corresponding weight"@en ;
    skos:definition ""@en ;
.

trait:standard_length
    a skos:Concept, aphia-trait:Trait ;
    skos:inScheme trait:conceptScheme ;
    skos:prefLabel "Standard length (SL)"@en ;
    skos:definition "The measurement from the most anterior tip of the body to the midlateral posterior edge of the hypural plate (in fish with a hypural plate) or to the posterior end of the vertebral column (in fish lacking hypural plates). It may be restricted to the tip of the snout if the lower jaw projects. The base of the caudal fin (end of the vertebral column or posterior edge of the hypural plate) is determined by flexing the tail up while the caudal peduncle is held down. The resultant wrinkle or caudal flexure indicates the caudal base. It may also be determined by probing or dissection. Sometimes the posteriormost point is the last scale, the last pored scale or the beginning of the caudal fin rays. It is the usual scientific measurement for length of a fish except in Myxini, Petromyzontiformes, Elasmobranchii and Holocephali. This measurement is used because long-preserved fish often lose the tips of the caudal fin rays through breakage after the desiccation effect of alcohol. See total length and fork length. In Holocephali the length is usually taken from the tip of the snout to the origin of the upper caudal fin because the caudal filament breaks off frequently. In Scaridae it is taken back to the rear margin of the second to last lateral line scale {because the large scales obscure the point of caudal flexure. In small dead fish, the end point is detected by bending the caudal fin to one side. In fishery work, as a result of the use of the measuring board, standard-, fork- and total length are taken from the most anterior part of the head. Abbreviated as SL."@en ;

    skos:exactMatch ... ; 
.

trait:total_length
    a skos:Concept, aphia-trait:Trait ;
    skos:inScheme trait:conceptScheme ;
    skos:prefLabel "Total length (TL)"@en ;
    skos:definition "The greatest length of the whole body between the most anterior point of the body and the most posterior point, in a straight line, not over the curve of the body. Sometimes, when there are two equal lobes, the caudal rays are squeezed together and their tip is taken as the most posterior point (excluding the caudal filaments), or the longest lobe is squeezed to the midline (maximum length or extreme tip length). Also an imaginary line may be drawn between the two lobe tips and length to its mid-point taken as the most posterior point (total auxiliary length or bilobular length). Usually the tip of the most posterior lobe of the fin in normal position is taken as the posteriormost point (total normal length or natural tip length). Total length is used by taxonomists in Myxini, Petromyzontiformes, usually in Elasmobranchii and sometimes in other fishes. Standard length is usually employed with Teleostei. Abbreviated TL."@en ;

    skos:exactMatch ... ; 
.

trait:fork_length
    a skos:Concept, aphia-trait:Trait ;
    skos:inScheme trait:conceptScheme ;
    skos:prefLabel "Fork length (FL)"@en ;
    skos:definition "Length of a fish measured from the tip of the snout to the posterior end of the middle caudal rays. This measurement is used instead of standard length for fishes on which it is difficult to ascertain the end of the vertebral column, and instead of total length in fish with stiff, forked tail, e.g., tuna. Mostly used in fishery biology and not in systematics."@en ;

    skos:exactMatch ... ; 
.

trait:width_of_disk
    a skos:Concept, aphia-trait:Trait ;
    skos:inScheme trait:conceptScheme ;
    skos:prefLabel "Width of disk (WD)"@en ;
    skos:definition "The greatest distance between the lateral tips of the pectoral fins in Rajiformes."@en ;

    skos:exactMatch ... ; 
.

trait:prosome_length
    a skos:Concept, aphia-trait:Trait ;
    skos:inScheme trait:conceptScheme ;
    skos:prefLabel "Prosome length"@en ;
    skos:definition "Length of the promose, which is the anterior tagma of the copepod body comprising the cephalosome plus the first to fifth pedigerous somites in gymnoplean copepods, and the cephalosome plus the first to fourth pedigerous somites in podoplean copepods."@en ;
.

trait:patch_diameter
    a skos:Concept, aphia-trait:Trait ;
    skos:inScheme trait:conceptScheme ;
    skos:prefLabel "Patch diameter"@en ;
    skos:definition "Diameter of a mat, cluster or tuft of individuals."@en ;
.