@prefix skos: <http://www.w3.org/2004/02/skos/core#> .
@prefix rdfs: <http://www.w3.org/2000/01/rdf-schema#> .
@prefix dct: <http://purl.org/dc/terms/> .
@prefix aphia-trait: <https://aphia.org/ns/attribute-trait/> .

@base <https://aphia.org/ns/traits/cites_annex> .

<>
    a skos:Collection ; 
    dct:description "Convention on International Trade in Endangered Species of Wild Fauna and Flora (CITES). Consulted April 2015."@en ;

    skos:member <#cites_annex_I> , <#cites_annex_II> , <#cites_annex_III> ;
.

<#cites_annex_I>
    a skos:Concept, aphia-trait:Trait ;
    skos:inScheme <https://aphia.org/ns/traits/> ;
    skos:prefLabel "CITES annex I"@en ;
    skos:definition "Species threatened with extinction. Trade in specimens of these species is permitted only in exceptional circumstances."@en ;
.

<#cites_annex_II>
    a skos:Concept, aphia-trait:Trait ;
    skos:inScheme <https://aphia.org/ns/traits/> ;
    skos:prefLabel "CITES annex II"@en ;
    skos:definition "Species not necessarily threatened with extinction, but in which trade must be controlled in order to avoid utilization incompatible with their survival."@en ;
.

<#cites_annex_III>
    a skos:Concept, aphia-trait:Trait ;
    skos:inScheme <https://aphia.org/ns/traits/> ;
    skos:prefLabel "CITES annex III"@en ;
    skos:definition "Species that are protected in at least one country, which has asked other CITES Parties for assistance in controlling the trade."@en ;
.