@prefix skos: <http://www.w3.org/2004/02/skos/core#> .
@prefix rdfs: <http://www.w3.org/2000/01/rdf-schema#> .
@prefix dct: <http://purl.org/dc/terms/> .

@prefix aphia-trait: <https://aphia.org/ns/attribute-trait/> .

@prefix trait: <https://aphia.org/ns/vocab/attribute-trait/> .


trait:habitats_directive_annex
    a skos:Collection ; 
    dct:description "Council Directive 92/43/EEC of 21 May 1992 on the conservation of natural habitats and of wild fauna and flora."@en ;

    skos:member trait:habitats_directive_annex_I , 
                trait:habitats_directive_annex_II , 
                trait:habitats_directive_annex_III , 
                trait:habitats_directive_annex_IV , 
                trait:habitats_directive_annex_V , 
                trait:habitats_directive_annex_VI ;
.

trait:habitats_directive_annex_I
    a skos:Concept, aphia-trait:Trait ;
    skos:inScheme trait:conceptScheme ;
    skos:prefLabel "Habitats Directive Annex I"@en ;
    skos:definition "Natural habitat types of community interest whose conservation requires the designation of specia areas of conservation."@en ;
.

trait:habitats_directive_annex_II
    a skos:Concept, aphia-trait:Trait ;
    skos:inScheme trait:conceptScheme ;
    skos:prefLabel "Habitats Directive Annex II"@en ;
    skos:definition "Animal and plant species of community interest whose conservation requires the designation of special areas of conservation."@en ;
.

trait:habitats_directive_annex_III
    a skos:Concept, aphia-trait:Trait ;
    skos:inScheme trait:conceptScheme ;
    skos:prefLabel "Habitats Directive Annex III"@en ;
    skos:definition "Criteria for selecting sites eligible for identification as sites of community importance and designation as specieal areas of conservation."@en ;
.

trait:habitats_directive_annex_IV
    a skos:Concept, aphia-trait:Trait ;
    skos:inScheme trait:conceptScheme ;
    skos:prefLabel "Habitats Directive Annex IV"@en ;
    skos:definition "Animal and plant species of comminity interest in need of strict protection."@en ;
.

trait:habitats_directive_annex_V
    a skos:Concept, aphia-trait:Trait ;
    skos:inScheme trait:conceptScheme ;
    skos:prefLabel "Habitats Directive Annex V"@en ;
    skos:definition "Animal and plant species of community interest whose taking in the wild and exploitation may be subject to management measures."@en ;
.

trait:habitats_directive_annex_VI
    a skos:Concept, aphia-trait:Trait ;
    skos:inScheme trait:conceptScheme ;
    skos:prefLabel "Habitats Directive Annex VI"@en ;
    skos:definition "Prohibited methods and means of capture and killing and modes of transport."@en ;
.