@prefix skos: <http://www.w3.org/2004/02/skos/core#> .
@prefix rdfs: <http://www.w3.org/2000/01/rdf-schema#> .
@prefix dct: <http://purl.org/dc/terms/> .
@prefix aphia-trait: <https://aphia.org/ns/attribute-trait/> .

@base <https://aphia.org/ns/traits/plant_habit> .

<>
    a skos:Collection ; 
    dct:description "The characteristic form in which a given species of plant grows"@en ;

    skos:member <#tree> , 
                <#shrub> , 
                <#herb> , 
                    <#annual_herb> , 
                    <#biennial_herb> , 
                    <#perennial_herb> , 
                <#vine> ;
.

<#tree>
    a skos:Concept, aphia-trait:Trait ;
    skos:inScheme <https://aphia.org/ns/traits/> ;
    skos:prefLabel "Tree"@en ;
    skos:definition "A woody perennial plant which has a single main trunk at least 7.5 cm in diameter at 1.3 m height, a definitely formed crown of foliage, and a height of at least 4 m."@en ;
.

<#shrub>
    a skos:Concept, aphia-trait:Trait ;
    skos:inScheme <https://aphia.org/ns/traits/> ;
    skos:prefLabel "Shrub"@en ;
    skos:definition "Low-growing woody plant, usually less than 6 m high, that does not have a main trunk and which branches from the base."@en ;
.

<#herb>
    a skos:Concept, aphia-trait:Trait ;
    skos:inScheme <https://aphia.org/ns/traits/> ;
    skos:prefLabel "Herb"@en ;
    skos:definition "Any seed plant with non-woody green stems."@en ;

    skos:narrower <#annual_herb> , <#biennial_herb> , <#perennial_herb> ;
.

<#annual_herb>
    a skos:Concept, aphia-trait:Trait ;
    skos:inScheme <https://aphia.org/ns/traits/> ;
    skos:prefLabel "Annual herb"@en ;
    skos:definition "(1) appl. structures or growth features that are marked off or completed yearly; (2) living for a year only; (3) completing life-cycle in a year from germination; (4) n. plant that completes its life-cycle in a year."@en ;

    skos:broader <#herb> ; 
.

<#biennial_herb>
    a skos:Concept, aphia-trait:Trait ;
    skos:inScheme <https://aphia.org/ns/traits/> ;
    skos:prefLabel "Biennial herb"@en ;
    skos:definition "Plant living for two years and fruiting only in the second."@en ;

    skos:broader <#herb> ; 
.

<#perennial_herb>
    a skos:Concept, aphia-trait:Trait ;
    skos:inScheme <https://aphia.org/ns/traits/> ;
    skos:prefLabel "Perennial herb"@en ;
    skos:definition "Plant which persists for several years."@en ;

    skos:broader <#herb> ; 
.

<#vine>
    a skos:Concept, aphia-trait:Trait ;
    skos:inScheme <https://aphia.org/ns/traits/> ;
    skos:prefLabel "Vine"@en ;
    skos:definition ""@en ;
.