@prefix skos: <http://www.w3.org/2004/02/skos/core#> .
@prefix rdfs: <http://www.w3.org/2000/01/rdf-schema#> .
@prefix dct: <http://purl.org/dc/terms/> .

@prefix aphia-trait: <https://aphia.org/ns/attribute-trait/> .

@prefix trait: <https://aphia.org/ns/vocab/attribute-trait/> .

trait:conceptScheme
    a skos:ConceptScheme ;
    rdfs:label "Listing Aphia attributes and traits"@en .

<https://aphia.org/ns/vocab/attribute-trait/>
    a skos:Collection ;
    rdfs:label "Aphia attributes and traits"@en ;
    
    skos:member trait:plant_habit ;
.

trait:plant_habit
    a skos:Collection ; 
    dct:description "The characteristic form in which a given species of plant grows"@en ;

    skos:member trait:tree , 
                trait:shrub , 
                trait:herb , 
                    trait:annual_herb , 
                    trait:biennial_herb , 
                    trait:perennial_herb , 
                trait:vine ;
.

trait:tree
    a skos:Concept, aphia-trait:Trait ;
    skos:inScheme trait:conceptScheme ;
    skos:prefLabel "Tree"@en ;
    skos:definition "A woody perennial plant which has a single main trunk at least 7.5 cm in diameter at 1.3 m height, a definitely formed crown of foliage, and a height of at least 4 m."@en ;
.

trait:shrub
    a skos:Concept, aphia-trait:Trait ;
    skos:inScheme trait:conceptScheme ;
    skos:prefLabel "Shrub"@en ;
    skos:definition "Low-growing woody plant, usually less than 6 m high, that does not have a main trunk and which branches from the base."@en ;
.

trait:herb
    a skos:Concept, aphia-trait:Trait ;
    skos:inScheme trait:conceptScheme ;
    skos:prefLabel "Herb"@en ;
    skos:definition "Any seed plant with non-woody green stems."@en ;

    skos:narrower trait:annual_herb , trait:biennial_herb , trait:perennial_herb ;
.

trait:annual_herb
    a skos:Concept, aphia-trait:Trait ;
    skos:inScheme trait:conceptScheme ;
    skos:prefLabel "Annual herb"@en ;
    skos:definition "(1) appl. structures or growth features that are marked off or completed yearly; (2) living for a year only; (3) completing life-cycle in a year from germination; (4) n. plant that completes its life-cycle in a year."@en ;

    skos:broader trait:herb ; 
.

trait:biennial_herb
    a skos:Concept, aphia-trait:Trait ;
    skos:inScheme trait:conceptScheme ;
    skos:prefLabel "Biennial herb"@en ;
    skos:definition "Plant living for two years and fruiting only in the second."@en ;

    skos:broader trait:herb ; 
.

trait:perennial_herb
    a skos:Concept, aphia-trait:Trait ;
    skos:inScheme trait:conceptScheme ;
    skos:prefLabel "Perennial herb"@en ;
    skos:definition "Plant which persists for several years."@en ;

    skos:broader trait:herb ; 
.

trait:vine
    a skos:Concept, aphia-trait:Trait ;
    skos:inScheme trait:conceptScheme ;
    skos:prefLabel "Vine"@en ;
    skos:definition ""@en ;
.