@prefix skos: <http://www.w3.org/2004/02/skos/core#> .
@prefix rdfs: <http://www.w3.org/2000/01/rdf-schema#> .
@prefix dct: <http://purl.org/dc/terms/> .

@prefix aphia-trait: <https://aphia.org/ns/attribute-trait/> .

@prefix trait: <https://aphia.org/ns/vocab/attribute-trait/> .

trait:conceptScheme
    a skos:ConceptScheme ;
    rdfs:label "Listing Aphia attributes and traits"@en .

<https://aphia.org/ns/vocab/attribute-trait/>
    a skos:Collection ;
    rdfs:label "Aphia attributes and traits"@en ;
    
    skos:member trait:structure ;
.

trait:structure
    a skos:Collection ; 
    dct:description ""@en ;

    skos:member trait:solid , 
                trait:non_solid_cement , 
                trait:non_solid_particles ;
.

trait:solid
    a skos:Concept, aphia-trait:Trait ;
    skos:inScheme trait:conceptScheme ;
    skos:prefLabel "Solid"@en ;
    skos:definition "Massive structure, i.e. not consisting of loose agglutinated particles (derived from Lawrence 2005 - Henderson's Dictionary of Biology, and discussed and agreed upon by the WoRMS/Aphia editor community)."@en ;
.

trait:non_solid_cement
    a skos:Concept, aphia-trait:Trait ;
    skos:inScheme trait:conceptScheme ;
    skos:prefLabel "Non-solid, cement"@en ;
    skos:definition "Component that keeps the agglutinated particles of the non-massive skeleton together (derived from Lawrence 2005 - Henderson's Dictionary of Biology, and discussed and agreed upon by the WoRMS/Aphia editor community)."@en ;
.

trait:non_solid_particles
    a skos:Concept, aphia-trait:Trait ;
    skos:inScheme trait:conceptScheme ;
    skos:prefLabel "Non-solid, particles"@en ;
    skos:definition "Small and individual structural elements that function as supporting structure/enclosure, e.g. spicules in sponges (derived from Lawrence 2005 - Henderson's Dictionary of Biology, and discussed and agreed upon by the WoRMS/Aphia editor community)."@en ;
.
