@prefix skos: <http://www.w3.org/2004/02/skos/core#> .
@prefix rdfs: <http://www.w3.org/2000/01/rdf-schema#> .
@prefix dct: <http://purl.org/dc/terms/> .

@prefix aphia-trait: <https://aphia.org/ns/attribute-trait/> .

@base <https://aphia.org/ns/term/structure> .

<>
    a skos:Collection ; 
    dct:description ""@en ;

    skos:member <#solid> , 
                <#non_solid_cement> , 
                <#non_solid_particles> ;
.

<#solid>
    a skos:Concept, aphia-trait:Trait ;
    skos:inScheme <https://aphia.org/ns/vocab/attribute-trait/> ;
    skos:prefLabel "Solid"@en ;
    skos:definition "Massive structure, i.e. not consisting of loose agglutinated particles (derived from Lawrence 2005 - Henderson's Dictionary of Biology, and discussed and agreed upon by the WoRMS/Aphia editor community)."@en ;
.

<#non_solid_cement>
    a skos:Concept, aphia-trait:Trait ;
    skos:inScheme <https://aphia.org/ns/vocab/attribute-trait/> ;
    skos:prefLabel "Non-solid, cement"@en ;
    skos:definition "Component that keeps the agglutinated particles of the non-massive skeleton together (derived from Lawrence 2005 - Henderson's Dictionary of Biology, and discussed and agreed upon by the WoRMS/Aphia editor community)."@en ;
.

<#non_solid_particles>
    a skos:Concept, aphia-trait:Trait ;
    skos:inScheme <https://aphia.org/ns/vocab/attribute-trait/> ;
    skos:prefLabel "Non-solid, particles"@en ;
    skos:definition "Small and individual structural elements that function as supporting structure/enclosure, e.g. spicules in sponges (derived from Lawrence 2005 - Henderson's Dictionary of Biology, and discussed and agreed upon by the WoRMS/Aphia editor community)."@en ;
.
