@prefix skos: <http://www.w3.org/2004/02/skos/core#> .
@prefix rdfs: <http://www.w3.org/2000/01/rdf-schema#> .
@prefix dct: <http://purl.org/dc/terms/> .
@prefix aphia-trait: <https://aphia.org/ns/attribute-trait/> .

@base <https://aphia.org/ns/traits/wave_exposure> .

<>
    a skos:Collection ; 
    dct:description "Trait that describes the range of exposure to wave action in which the organism is recorded."@en ;

    skos:member <#exposed> , 
                    <#high_energy_rock> , 
                <#features_of_rock> , 
                <#semi_exposed> , 
                    <#moderate_energy_rock> , 
                <#sheltered> , 
                    <#coarse_sediments> , 
                    <#low_energy_rock> , 
                    <#macrophyte_dominated_sediments> , 
                    <#mud_dominated_sediments> , 
                    <#sand_dominated_sediments> , 
                <#unreported_wave_exposure> ; 
.

<#exposed>
    a skos:Concept, aphia-trait:Trait ;
    skos:inScheme <https://aphia.org/ns/traits/> ;
    skos:prefLabel "Exposed"@en ;
    skos:definition "Subject to high energy wave forces. (Definition composed by Line Le Gall, Olivier De Clerck, Sofie Vranken and Marine Robuchon, based on diverse literature sources, in the framework of compiling macroalgae traits.)"@en ;

    skos:narrower <#high_energy_rock> ; 
.

<#high_energy_rock>
    a skos:Concept, aphia-trait:Trait ;
    skos:inScheme <https://aphia.org/ns/traits/> ;
    skos:prefLabel "High energy rock"@en ;
    skos:definition "Rocky substrate subject to high energy wave forces. (Definition composed by Line Le Gall, Olivier De Clerck, Sofie Vranken and Marine Robuchon, based on diverse literature sources, in the framework of compiling macroalgae traits.)"@en ;

    skos:broader <#exposed> ; 
.

<#features_of_rock>
    a skos:Concept, aphia-trait:Trait ;
    skos:inScheme <https://aphia.org/ns/traits/> ;
    skos:prefLabel "Features of rock"@en ;
    skos:definition "Specific characteristics of rocky substrate such as pools, caves, overhangs, surge gulleys, artificial hard substrata. (Definition composed by Line Le Gall, Olivier De Clerck, Sofie Vranken and Marine Robuchon, based on diverse literature sources, in the framework of compiling macroalgae traits.)"@en ;
.

<#semi_exposed>
    a skos:Concept, aphia-trait:Trait ;
    skos:inScheme <https://aphia.org/ns/traits/> ;
    skos:prefLabel "Semi-exposed"@en ;
    skos:definition "Subject to moderate energy wave forces. (Definition composed by Line Le Gall, Olivier De Clerck, Sofie Vranken and Marine Robuchon, based on diverse literature sources, in the framework of compiling macroalgae traits.)"@en ;

    skos:narrower <#moderate_energy_rock> ;
.

<#moderate_energy_rock>
    a skos:Concept, aphia-trait:Trait ;
    skos:inScheme <https://aphia.org/ns/traits/> ;
    skos:prefLabel "Moderate energy rock"@en ;
    skos:definition "Rocky substrate subject to moderate energy wave forces. (Definition composed by Line Le Gall, Olivier De Clerck, Sofie Vranken and Marine Robuchon, based on diverse literature sources, in the framework of compiling macroalgae traits.)"@en ;

    skos:broader <#semi_exposed> ; 
.
<#sheltered>
    a skos:Concept, aphia-trait:Trait ;
    skos:inScheme <https://aphia.org/ns/traits/> ;
    skos:prefLabel "Sheltered"@en ;
    skos:definition "Subject to low energy wave forces. (Definition composed by Line Le Gall, Olivier De Clerck, Sofie Vranken and Marine Robuchon, based on diverse literature sources, in the framework of compiling macroalgae traits.)"@en ;

    skos:narrower <#coarse_sediments> , <#low_energy_rock> , <#macrophyte_dominated_sediments> , <#mud_dominated_sediments> , <#sand_dominated_sediments> ;
.
<#coarse_sediments>
    a skos:Concept, aphia-trait:Trait ;
    skos:inScheme <https://aphia.org/ns/traits/> ;
    skos:prefLabel "Coarse sediments"@en ;
    skos:definition "Coarse sediments such as gravel, pebbles, shingles and cobbles ocurring at sheltered locations. (Definition composed by Line Le Gall, Olivier De Clerck, Sofie Vranken and Marine Robuchon, based on diverse literature sources, in the framework of compiling macroalgae traits.)"@en ;

    skos:broader <#sheltered> ; 
.
<#low_energy_rock>
    a skos:Concept, aphia-trait:Trait ;
    skos:inScheme <https://aphia.org/ns/traits/> ;
    skos:prefLabel "Low energy rock"@en ;
    skos:definition "Rocky substrate subject to low energy wave forces. (Definition composed by Line Le Gall, Olivier De Clerck, Sofie Vranken and Marine Robuchon, based on diverse literature sources, in the framework of compiling macroalgae traits.)"@en ;

    skos:broader <#sheltered> ; 
.
<#macrophyte_dominated_sediments>
    a skos:Concept, aphia-trait:Trait ;
    skos:inScheme <https://aphia.org/ns/traits/> ;
    skos:prefLabel "Macrophyte-dominated sediments"@en ;
    skos:definition "Sediments with a high cover of macroalgae or seagrasses. (Definition composed by Line Le Gall, Olivier De Clerck, Sofie Vranken and Marine Robuchon, based on diverse literature sources, in the framework of compiling macroalgae traits.)"@en ;

    skos:broader <#sheltered> ; 
.
<#mud_dominated_sediments>
    a skos:Concept, aphia-trait:Trait ;
    skos:inScheme <https://aphia.org/ns/traits/> ;
    skos:prefLabel "Mud-dominated sediments"@en ;
    skos:definition "Sediments composed of a mixture of clay (< 2 um) and silt (4 - 62 um) typically deposited in a low energy environment. (Definition composed by Line Le Gall, Olivier De Clerck, Sofie Vranken and Marine Robuchon, based on diverse literature sources, in the framework of compiling macroalgae traits.)"@en ;

    skos:broader <#sheltered> ; 
.
<#sand_dominated_sediments>
    a skos:Concept, aphia-trait:Trait ;
    skos:inScheme <https://aphia.org/ns/traits/> ;
    skos:prefLabel "Sand-dominated sediments"@en ;
    skos:definition "Sediments composed of a mixture of sand particles (0.074 - 4.75 mm) typically deposited in a low energy environment. (Definition composed by Line Le Gall, Olivier De Clerck, Sofie Vranken and Marine Robuchon, based on diverse literature sources, in the framework of compiling macroalgae traits.)"@en ;

    skos:broader <#sheltered> ; 
.
<#unreported_wave_exposure>
    a skos:Concept, aphia-trait:Trait ;
    skos:inScheme <https://aphia.org/ns/traits/> ;
    skos:prefLabel "Unreported wave exposure"@en ;
    skos:definition "So far it has not been reported in literature which wave exposure this organism has."@en ;
.