@prefix skos: <http://www.w3.org/2004/02/skos/core#> .
@prefix rdfs: <http://www.w3.org/2000/01/rdf-schema#> .
@prefix dct: <http://purl.org/dc/terms/> .

@prefix aphia-trait: <https://aphia.org/ns/attribute-trait/> .

@prefix trait: <https://aphia.org/ns/vocab/attribute-trait/> .


trait:body_shape
    a skos:Collection ; 
    dct:description "The general shape of the body of an organism."@en ;

    skos:member trait:branched , 
                trait:capitate , 
                trait:crustose , 
                trait:cushion_like , 
                trait:discoid , 
                trait:erect , 
                trait:filamentous , 
                trait:flabellate , 
                trait:foliose , 
                trait:pinnate , 
                trait:prostrate , 
                trait:saccate , 
                trait:spheric , 
                trait:tubular , 
                trait:unreported_body_shape , 
                trait:filiform , 
                trait:mucilaginous , 
                trait:stoloniferous ; 
.

trait:branched
    a skos:Concept, aphia-trait:Trait ;
    skos:inScheme trait:conceptScheme ;
    skos:prefLabel "Branched"@en ;
    skos:definition "Forming main and lateral branches (and branchlets) (macroalgae thallus; Womersley, 1987)."@en ;

    skos:exactMatch ... ; 
.
trait:capitate
    a skos:Concept, aphia-trait:Trait ;
    skos:inScheme trait:conceptScheme ;
    skos:prefLabel "Capitate"@en ;
    skos:definition "(1) Enlarged or swollen at tip; (2) Gathered into a mass at tip of stem or apex (Adapted from Lawrence, 2005 - Henderson's dictionary of Biology)."@en ;

    skos:exactMatch ... ; 
.
trait:crustose
    a skos:Concept, aphia-trait:Trait ;
    skos:inScheme trait:conceptScheme ;
    skos:prefLabel "Crustose"@en ;
    skos:definition "Forming a thin crust on the substratum, appl. certain lichens, sponges, algae (adapted from Henderson's Dictionary of Biology; Lawrence, 2005)."@en ;

    skos:exactMatch ... ; 
.
trait:cushion_like
    a skos:Concept, aphia-trait:Trait ;
    skos:inScheme trait:conceptScheme ;
    skos:prefLabel "Cushion-like"@en ;
    skos:definition "Approximating the shape of a cushion (macroalgae thallus; Womersley, 1987)."@en ;

    skos:exactMatch ... ; 
.
trait:discoid
    a skos:Concept, aphia-trait:Trait ;
    skos:inScheme trait:conceptScheme ;
    skos:prefLabel "Discoid"@en ;
    skos:definition "(1) Flat and circular; (2) Disc-shaped (Henderson's Dictionary of Biology; Lawrence, 2005)."@en ;

    skos:exactMatch ... ; 
.
trait:erect
    a skos:Concept, aphia-trait:Trait ;
    skos:inScheme trait:conceptScheme ;
    skos:prefLabel "Erect"@en ;
    skos:definition "Upright; (1) appl. ovule, directed towards summit of ovary; (2) appl. plants, growing upright, not decumbent."@en ;

    skos:exactMatch ... ; 
.
trait:filamentous
    a skos:Concept, aphia-trait:Trait ;
    skos:inScheme trait:conceptScheme ;
    skos:prefLabel "Filamentous"@en ;
    skos:definition "Existing out of a branched or unbranched row of cells joined end to end (macroalgae thallus; Womersley, 1987)."@en ;

    skos:exactMatch ... ; 
.
trait:flabellate
    a skos:Concept, aphia-trait:Trait ;
    skos:inScheme trait:conceptScheme ;
    skos:prefLabel "Flabellate"@en ;
    skos:definition "With projecting flaps on one side, appl. to certain insect antennae (Henderson's Dictionary of Biology; Lawrence, 2005). Fan-shaped, thallus usually expanding upward from a narrow base. (macroalgae thallus; Definition composed by Line Le Gall, Olivier De Clerck, Sofie Vranken and Marine Robuchon, based on diverse literature sources, in the framework of compiling macroalgae traits.)"@en ;

    skos:exactMatch ... ; 
.
trait:foliose
    a skos:Concept, aphia-trait:Trait ;
    skos:inScheme trait:conceptScheme ;
    skos:prefLabel "Foliose"@en ;
    skos:definition "(1) With many leaves; (2) Having leaf-like lobes, appl. the thallus of some lichens and liverworts (Henderson's Dictionary of Biology; Lawrence, 2005). Leaf-like (macroalgae thallus; Womersley, 1987)."@en ;

    skos:exactMatch ... ; 
.
trait:pinnate
    a skos:Concept, aphia-trait:Trait ;
    skos:inScheme trait:conceptScheme ;
    skos:prefLabel "Pinnate"@en ;
    skos:definition "(1) Divided in a feathery manner; (2) having lateral processes; (3) (bot.) of a compound leaf, having leaflets on each side of an axis or midrib (Henderson's Dictionary of Biology; Lawrence, 2005). With laterals or branches arranged along each side of an axis or branch (macroalgae thallus; Womersley, 1987)."@en ;

    skos:exactMatch ... ; 
.
trait:prostrate
    a skos:Concept, aphia-trait:Trait ;
    skos:inScheme trait:conceptScheme ;
    skos:prefLabel "Prostrate"@en ;
    skos:definition "Trailing on the ground or lying closely along a surface (Henderson's Dictionary of Biology; Lawrence, 2005)."@en ;

    skos:exactMatch ... ; 
.
trait:saccate
    a skos:Concept, aphia-trait:Trait ;
    skos:inScheme trait:conceptScheme ;
    skos:prefLabel "Saccate"@en ;
    skos:definition "Pouched (Henderson's Dictionary of Biology; Lawrence, 2005). Inflated, or sac-like (macroalgae thallus; Womersley, 1987)."@en ;

    skos:exactMatch ... ; 
.
trait:spheric
    a skos:Concept, aphia-trait:Trait ;
    skos:inScheme trait:conceptScheme ;
    skos:prefLabel "Spheric"@en ;
    skos:definition "Approximating the shape of a sphere (macroalgae thallus; Womersley, 1987)."@en ;

    skos:exactMatch ... ; 
.
trait:tubular
    a skos:Concept, aphia-trait:Trait ;
    skos:inScheme trait:conceptScheme ;
    skos:prefLabel "Tubular"@en ;
    skos:definition "In the form of a tube, having tubes, consisting of tubes (Henderson's Dictionary of Biology; Lawrence, 2005)."@en ;

    skos:exactMatch ... ; 
.
trait:unreported_body_shape
    a skos:Concept, aphia-trait:Trait ;
    skos:inScheme trait:conceptScheme ;
    skos:prefLabel "Unreported body shape"@en ;
    skos:definition "So far it has not been reported in literature what the body shape (thallus) is for this taxon."@en ;
.
trait:filiform
    a skos:Concept, aphia-trait:Trait ;
    skos:inScheme trait:conceptScheme ;
    skos:prefLabel "Filiform"@en ;
    skos:definition "Resembling a filament (Olivier De Clerck). Thread-like."@en ;

    skos:exactMatch ... ; 
.
trait:mucilaginous
    a skos:Concept, aphia-trait:Trait ;
    skos:inScheme trait:conceptScheme ;
    skos:prefLabel "Mucilaginous"@en ;
    skos:definition "Consisting of a slippery and slimy texture (Maggs & Hommersand, 1993). Containing, or composed of mucilage (Henderson's Dictionary of Biology; Lawrence, 2005)."@en ;

    skos:exactMatch ... ; 
.
trait:stoloniferous
    a skos:Concept, aphia-trait:Trait ;
    skos:inScheme trait:conceptScheme ;
    skos:prefLabel "Stoloniferous"@en ;
    skos:definition "Forming a prostrate axis, lying on or in the substrate, from which erect branches arise (Womersley, 1984). Bearing a stolon or stolons (Henderson's Dictionary of Biology; Lawrence, 2005)."@en ;

    skos:exactMatch ... ; 
.