@prefix skos: <http://www.w3.org/2004/02/skos/core#> .
@prefix rdfs: <http://www.w3.org/2000/01/rdf-schema#> .
@prefix dct: <http://purl.org/dc/terms/> .

@prefix aphia-trait: <https://aphia.org/ns/attribute-trait/> .

@base <https://aphia.org/ns/term/body_shape> .

<>
    a skos:Collection ; 
    dct:description "The general shape of the body of an organism."@en ;

    skos:member <#branched> , 
                <#capitate> , 
                <#crustose> , 
                <#cushion_like> , 
                <#discoid> , 
                <#erect> , 
                <#filamentous> , 
                <#flabellate> , 
                <#foliose> , 
                <#pinnate> , 
                <#prostrate> , 
                <#saccate> , 
                <#spheric> , 
                <#tubular> , 
                <#unreported_body_shape> , 
                <#filiform> , 
                <#mucilaginous> , 
                <#stoloniferous> ; 
.

<#branched>
    a skos:Concept, aphia-trait:Trait ;
    skos:inScheme <https://aphia.org/ns/vocab/attribute-trait/> ;
    skos:prefLabel "Branched"@en ;
    skos:definition "Forming main and lateral branches (and branchlets) (macroalgae thallus; Womersley, 1987)."@en ;

    skos:exactMatch ... ; 
.
<#capitate>
    a skos:Concept, aphia-trait:Trait ;
    skos:inScheme <https://aphia.org/ns/vocab/attribute-trait/> ;
    skos:prefLabel "Capitate"@en ;
    skos:definition "(1) Enlarged or swollen at tip; (2) Gathered into a mass at tip of stem or apex (Adapted from Lawrence, 2005 - Henderson's dictionary of Biology)."@en ;

    skos:exactMatch ... ; 
.
<#crustose>
    a skos:Concept, aphia-trait:Trait ;
    skos:inScheme <https://aphia.org/ns/vocab/attribute-trait/> ;
    skos:prefLabel "Crustose"@en ;
    skos:definition "Forming a thin crust on the substratum, appl. certain lichens, sponges, algae (adapted from Henderson's Dictionary of Biology; Lawrence, 2005)."@en ;

    skos:exactMatch ... ; 
.
<#cushion_like>
    a skos:Concept, aphia-trait:Trait ;
    skos:inScheme <https://aphia.org/ns/vocab/attribute-trait/> ;
    skos:prefLabel "Cushion-like"@en ;
    skos:definition "Approximating the shape of a cushion (macroalgae thallus; Womersley, 1987)."@en ;

    skos:exactMatch ... ; 
.
<#discoid>
    a skos:Concept, aphia-trait:Trait ;
    skos:inScheme <https://aphia.org/ns/vocab/attribute-trait/> ;
    skos:prefLabel "Discoid"@en ;
    skos:definition "(1) Flat and circular; (2) Disc-shaped (Henderson's Dictionary of Biology; Lawrence, 2005)."@en ;

    skos:exactMatch ... ; 
.
<#erect>
    a skos:Concept, aphia-trait:Trait ;
    skos:inScheme <https://aphia.org/ns/vocab/attribute-trait/> ;
    skos:prefLabel "Erect"@en ;
    skos:definition "Upright; (1) appl. ovule, directed towards summit of ovary; (2) appl. plants, growing upright, not decumbent."@en ;

    skos:exactMatch ... ; 
.
<#filamentous>
    a skos:Concept, aphia-trait:Trait ;
    skos:inScheme <https://aphia.org/ns/vocab/attribute-trait/> ;
    skos:prefLabel "Filamentous"@en ;
    skos:definition "Existing out of a branched or unbranched row of cells joined end to end (macroalgae thallus; Womersley, 1987)."@en ;

    skos:exactMatch ... ; 
.
<#flabellate>
    a skos:Concept, aphia-trait:Trait ;
    skos:inScheme <https://aphia.org/ns/vocab/attribute-trait/> ;
    skos:prefLabel "Flabellate"@en ;
    skos:definition "With projecting flaps on one side, appl. to certain insect antennae (Henderson's Dictionary of Biology; Lawrence, 2005). Fan-shaped, thallus usually expanding upward from a narrow base. (macroalgae thallus; Definition composed by Line Le Gall, Olivier De Clerck, Sofie Vranken and Marine Robuchon, based on diverse literature sources, in the framework of compiling macroalgae traits.)"@en ;

    skos:exactMatch ... ; 
.
<#foliose>
    a skos:Concept, aphia-trait:Trait ;
    skos:inScheme <https://aphia.org/ns/vocab/attribute-trait/> ;
    skos:prefLabel "Foliose"@en ;
    skos:definition "(1) With many leaves; (2) Having leaf-like lobes, appl. the thallus of some lichens and liverworts (Henderson's Dictionary of Biology; Lawrence, 2005). Leaf-like (macroalgae thallus; Womersley, 1987)."@en ;

    skos:exactMatch ... ; 
.
<#pinnate>
    a skos:Concept, aphia-trait:Trait ;
    skos:inScheme <https://aphia.org/ns/vocab/attribute-trait/> ;
    skos:prefLabel "Pinnate"@en ;
    skos:definition "(1) Divided in a feathery manner; (2) having lateral processes; (3) (bot.) of a compound leaf, having leaflets on each side of an axis or midrib (Henderson's Dictionary of Biology; Lawrence, 2005). With laterals or branches arranged along each side of an axis or branch (macroalgae thallus; Womersley, 1987)."@en ;

    skos:exactMatch ... ; 
.
<#prostrate>
    a skos:Concept, aphia-trait:Trait ;
    skos:inScheme <https://aphia.org/ns/vocab/attribute-trait/> ;
    skos:prefLabel "Prostrate"@en ;
    skos:definition "Trailing on the ground or lying closely along a surface (Henderson's Dictionary of Biology; Lawrence, 2005)."@en ;

    skos:exactMatch ... ; 
.
<#saccate>
    a skos:Concept, aphia-trait:Trait ;
    skos:inScheme <https://aphia.org/ns/vocab/attribute-trait/> ;
    skos:prefLabel "Saccate"@en ;
    skos:definition "Pouched (Henderson's Dictionary of Biology; Lawrence, 2005). Inflated, or sac-like (macroalgae thallus; Womersley, 1987)."@en ;

    skos:exactMatch ... ; 
.
<#spheric>
    a skos:Concept, aphia-trait:Trait ;
    skos:inScheme <https://aphia.org/ns/vocab/attribute-trait/> ;
    skos:prefLabel "Spheric"@en ;
    skos:definition "Approximating the shape of a sphere (macroalgae thallus; Womersley, 1987)."@en ;

    skos:exactMatch ... ; 
.
<#tubular>
    a skos:Concept, aphia-trait:Trait ;
    skos:inScheme <https://aphia.org/ns/vocab/attribute-trait/> ;
    skos:prefLabel "Tubular"@en ;
    skos:definition "In the form of a tube, having tubes, consisting of tubes (Henderson's Dictionary of Biology; Lawrence, 2005)."@en ;

    skos:exactMatch ... ; 
.
<#unreported_body_shape>
    a skos:Concept, aphia-trait:Trait ;
    skos:inScheme <https://aphia.org/ns/vocab/attribute-trait/> ;
    skos:prefLabel "Unreported body shape"@en ;
    skos:definition "So far it has not been reported in literature what the body shape (thallus) is for this taxon."@en ;
.
<#filiform>
    a skos:Concept, aphia-trait:Trait ;
    skos:inScheme <https://aphia.org/ns/vocab/attribute-trait/> ;
    skos:prefLabel "Filiform"@en ;
    skos:definition "Resembling a filament (Olivier De Clerck). Thread-like."@en ;

    skos:exactMatch ... ; 
.
<#mucilaginous>
    a skos:Concept, aphia-trait:Trait ;
    skos:inScheme <https://aphia.org/ns/vocab/attribute-trait/> ;
    skos:prefLabel "Mucilaginous"@en ;
    skos:definition "Consisting of a slippery and slimy texture (Maggs & Hommersand, 1993). Containing, or composed of mucilage (Henderson's Dictionary of Biology; Lawrence, 2005)."@en ;

    skos:exactMatch ... ; 
.
<#stoloniferous>
    a skos:Concept, aphia-trait:Trait ;
    skos:inScheme <https://aphia.org/ns/vocab/attribute-trait/> ;
    skos:prefLabel "Stoloniferous"@en ;
    skos:definition "Forming a prostrate axis, lying on or in the substrate, from which erect branches arise (Womersley, 1984). Bearing a stolon or stolons (Henderson's Dictionary of Biology; Lawrence, 2005)."@en ;

    skos:exactMatch ... ; 
.