@prefix skos: <http://www.w3.org/2004/02/skos/core#> .
@prefix rdfs: <http://www.w3.org/2000/01/rdf-schema#> .
@prefix dct: <http://purl.org/dc/terms/> .

@prefix aphia-trait: <https://aphia.org/ns/attribute-trait/> .

@base <https://aphia.org/ns/term/calcification> .

<>
    a skos:Collection ; 
    dct:description "Mode of calcification of seaweed."@en ;

    skos:member <#calcified_articulated> , <#calcified_non_articulated> , <#non_calcified> , <#unreported> ; 
.

<#calcified_articulated>
    a skos:Concept, aphia-trait:Trait ;
    skos:inScheme <https://aphia.org/ns/vocab/attribute-trait/> ;
    skos:prefLabel "calcified articulated"@en ;
    skos:definition "Algal thallus that is encrusted or impregnated with lime with non-calcified articulae rendering the thallus a segmented nature (macroalgae)."@en ;
.

<#calcified_non_articulated>
    a skos:Concept, aphia-trait:Trait ;
    skos:inScheme <https://aphia.org/ns/vocab/attribute-trait/> ;
    skos:prefLabel "calcified non-articulated"@en ;
    skos:definition "Algal thallus that is encrusted or impregnated with lime lacking non-calcified articulae (macroalgae)."@en ;
.

<#non_calcified>
    a skos:Concept, aphia-trait:Trait ;
    skos:inScheme <https://aphia.org/ns/vocab/attribute-trait/> ;
    skos:prefLabel "Non-calcified"@en ;
    skos:definition "Algal thallus not encrusted or impregnated with lime (macroalgae)."@en ;
.

<#unreported>
    a skos:Concept, aphia-trait:Trait ;
    skos:inScheme <https://aphia.org/ns/vocab/attribute-trait/> ;
    skos:prefLabel "Unreported"@en ;
    skos:definition "So far it has not been reported in literature whether or not the algal thallus is calcified (macroalgae)."@en ;
.
