@prefix skos: <http://www.w3.org/2004/02/skos/core#> .
@prefix rdfs: <http://www.w3.org/2000/01/rdf-schema#> .
@prefix dct: <http://purl.org/dc/terms/> .

@prefix aphia-trait: <https://aphia.org/ns/attribute-trait/> .

@prefix trait: <https://aphia.org/ns/vocab/attribute-trait/> .

trait:conceptScheme
    a skos:ConceptScheme ;
    rdfs:label "Listing Aphia attributes and traits"@en .

<https://aphia.org/ns/vocab/attribute-trait/>
    a skos:Collection ;
    rdfs:label "Aphia attributes and traits"@en ;
    
    skos:member trait:calcification ;
.

trait:calcification
    a skos:Collection ; 
    dct:description "Mode of calcification of seaweed."@en ;

    skos:member trait:calcified_articulated , trait:calcified_non_articulated , trait:non_calcified , trait:unreported ; 
.

trait:calcified_articulated
    a skos:Concept, aphia-trait:Trait ;
    skos:inScheme trait:conceptScheme ;
    skos:prefLabel "calcified articulated"@en ;
    skos:definition "Algal thallus that is encrusted or impregnated with lime with non-calcified articulae rendering the thallus a segmented nature (macroalgae)."@en ;
.

trait:calcified_non_articulated
    a skos:Concept, aphia-trait:Trait ;
    skos:inScheme trait:conceptScheme ;
    skos:prefLabel "calcified non-articulated"@en ;
    skos:definition "Algal thallus that is encrusted or impregnated with lime lacking non-calcified articulae (macroalgae)."@en ;
.

trait:non_calcified
    a skos:Concept, aphia-trait:Trait ;
    skos:inScheme trait:conceptScheme ;
    skos:prefLabel "Non-calcified"@en ;
    skos:definition "Algal thallus not encrusted or impregnated with lime (macroalgae)."@en ;
.

trait:unreported
    a skos:Concept, aphia-trait:Trait ;
    skos:inScheme trait:conceptScheme ;
    skos:prefLabel "Unreported"@en ;
    skos:definition "So far it has not been reported in literature whether or not the algal thallus is calcified (macroalgae)."@en ;
.
