@prefix skos: <http://www.w3.org/2004/02/skos/core#> .
@prefix rdfs: <http://www.w3.org/2000/01/rdf-schema#> .

@prefix aphia-trait: <https://aphia.org/ns/attribute-trait/> .

@base <https://aphia.org/ns/term/functional_group> .

<>
    a skos:Collection ; 

    skos:member <#benthos> , 
                    <#megabenthos> , 
                    <#macrobenthos> , 
                    <#meiobenthos> , 
                    <#microbenthos> , 
                    <#hyperbenthos> , 
                    <#epibenthos> , 
                    <#endobenthos> , 
                    <#phytobenthos> , 
                <#plankton> ,
                    <#megaplankton>, 
                    <#macroplankton>, 
                    <#mesoplankton>, 
                    <#microplankton>, 
                    <#nanoplankton>, 
                    <#picoplankton>, 
                    <#femtoplankton>, 
                    <#zooplankton> , 
                    <#phytoplankton> ,
                    <#mixoplankton> , 
                        <#endosymbiotic_specialist_non_constitutive_mixoplankton> , 
                        <#constitutive_mixoplankton> , 
                        <#plastid_specialists_non_constitutive_mixoplankton> , 
                        <#general_non_constitutive_mixoplankton> , 
                <#nekton> , 
                <#neuston> , 
                <#pleuston> , 
                <#benthopelagic> , 
                <#edaphofauna> , 
                    <#macroedaphofauna> , 
                    <#mesoedaphofauna> , 
                <#functional_group_not_applicable> ; 
. 

<#benthos>
    a skos:Concept, aphia-trait:Trait ;
    skos:inScheme <https://aphia.org/ns/vocab/attribute-trait/> ;
    skos:prefLabel "Benthos"@en ;
    skos:definition "Benthic organisms, or the benthos, are those that live on or burried in the bottom."@en ;

    skos:narrower <#megabenthos>, <#macrobenthos>, <#meiobenthos>, <#microbenthos>, <#hyperbenthos>, <#epibenthos>, <#endobenthos>, <#phytobenthos> ;

    skos:closeMatch ... ; 
.

<#megabenthos>
    a skos:Concept, aphia-trait:Trait ;
    skos:inScheme <https://aphia.org/ns/vocab/attribute-trait/> ;
    skos:prefLabel "Megabenthos"@en ;
    skos:definition "The component of the benthos that consists of very large organisms over 20 cm in size (as defined, agreed and applied by the WoRMS Steering Committee)."@en ;

    skos:broader <#benthos> ; 
.

<#macrobenthos>
    a skos:Concept, aphia-trait:Trait ;
    skos:inScheme <https://aphia.org/ns/vocab/attribute-trait/> ;
    skos:prefLabel "Macrobenthos"@en ;
    skos:definition "The component of the benthos that consists of large organisms 2 to 200 mm in size (as defined, agreed and applied by the WoRMS Steering Committee)."@en ;

    skos:broader <#benthos> ; 
.

<#meiobenthos>
    a skos:Concept, aphia-trait:Trait ;
    skos:inScheme <https://aphia.org/ns/vocab/attribute-trait/> ;
    skos:prefLabel "Meiobenthos"@en ;
    skos:definition "The component of the benthos that consists of organisms 0,2 to 2 mm in size (as defined, agreed and applied by the WoRMS Steering Committee)."@en ;

    skos:broader <#benthos> ; 
.

<#microbenthos>
    a skos:Concept, aphia-trait:Trait ;
    skos:inScheme <https://aphia.org/ns/vocab/attribute-trait/> ;
    skos:prefLabel "Microbenthos"@en ;
    skos:definition "The component of the benthos that consists of organisms 20 to 200 microns (µm) (0,02 to 0,2 mm) in size (as defined, agreed and applied by the WoRMS Steering Committee)."@en ;

    skos:broader <#benthos> ; 
.

<#hyperbenthos>
    a skos:Concept, aphia-trait:Trait ;
    skos:inScheme <https://aphia.org/ns/vocab/attribute-trait/> ;
    skos:prefLabel "Hyperbenthos"@en ;
    skos:definition "Organisms living above but close to the substratum."@en ;

    skos:broader <#benthos> ; 
.

<#epibenthos>
    a skos:Concept, aphia-trait:Trait ;
    skos:inScheme <https://aphia.org/ns/vocab/attribute-trait/> ;
    skos:prefLabel "Epibenthos"@en ;
    skos:definition "Organisms living on the surface of the bottom. Epifaunal or epifloral."@en ;

    skos:broader <#benthos> ; 

    skos:closeMatch ... ; 
.

<#endobenthos>
    a skos:Concept, aphia-trait:Trait ;
    skos:inScheme <https://aphia.org/ns/vocab/attribute-trait/> ;
    skos:prefLabel "Endobenthos"@en ;
    skos:definition "Organisms living within the sediment of a lake or sea floor; infauna. Also called endobiontic."@en ;

    skos:broader <#benthos> ; 

    skos:closeMatch ... ; 
.

<#phytobenthos>
    a skos:Concept, aphia-trait:Trait ;
    skos:inScheme <https://aphia.org/ns/vocab/attribute-trait/> ;
    skos:prefLabel "Phytobenthos"@en ;
    skos:definition "1: A bottom-living plant community; phytobenthon. 2: That part of the bottom of a stream or lake covered by vegetation; cf. geobenthos."@en ;

    skos:broader <#benthos> ; 
.

<#plankton>
    a skos:Concept, aphia-trait:Trait ;
    skos:inScheme <https://aphia.org/ns/vocab/attribute-trait/> ;
    skos:prefLabel "Plankton"@en ;
    skos:definition "Organisms that cannot maintain a fixed location in the water column, and are thus moved by the tides and currents."@en ;

    skos:narrower <#megaplankton>, <#macroplankton>, <#mesoplankton>, <#microplankton>, <#nanoplankton>, <#picoplankton>, <#femtoplankton>, <#zooplankton> , <#phytoplankton> ,
        <#mixoplankton> , <#endosymbiotic_specialist_non_constitutive_mixoplankton> , <#constitutive_mixoplankton> , <#plastid_specialists_non_constitutive_mixoplankton> , <#general_non_constitutive_mixoplankton> ;
.

<#megaplankton>
    a skos:Concept, aphia-trait:Trait ;
    skos:inScheme <https://aphia.org/ns/vocab/attribute-trait/> ;
    skos:prefLabel "Megaplankton"@en ;
    skos:definition "The component of the plankton that consists of very large organisms over 20 cm in size."@en ;

    skos:broader <#plankton> ; 
.

<#macroplankton>
    a skos:Concept, aphia-trait:Trait ;
    skos:inScheme <https://aphia.org/ns/vocab/attribute-trait/> ;
    skos:prefLabel "Macroplankton"@en ;
    skos:definition "The component of the plankton that consists of large organisms 2 to 200 mm in size (as defined, agreed and applied by the WoRMS Steering Committee)."@en ;

    skos:broader <#plankton> ; 
.

<#mesoplankton>
    a skos:Concept, aphia-trait:Trait ;
    skos:inScheme <https://aphia.org/ns/vocab/attribute-trait/> ;
    skos:prefLabel "Mesoplankton"@en ;
    skos:definition "The component of the plankton that consists of organisms 0,2 to 2 mm in size."@en ;

    skos:broader <#plankton> ; 
.

<#microplankton>
    a skos:Concept, aphia-trait:Trait ;
    skos:inScheme <https://aphia.org/ns/vocab/attribute-trait/> ;
    skos:prefLabel "Microplankton"@en ;
    skos:definition "The component of the plankton that consists of organisms 20 to 200 microns (µm) (0,02 to 0,2 mm) in size."@en ;

    skos:broader <#plankton> ; 
.

<#nanoplankton>
    a skos:Concept, aphia-trait:Trait ;
    skos:inScheme <https://aphia.org/ns/vocab/attribute-trait/> ;
    skos:prefLabel "Nanoplankton"@en ;
    skos:definition "The component of the plankton that consists of very small organisms 2 to 20 microns (µm) (0,002 to 0,02 mm) in size; they are too small to catch in a standard plankton net."@en ;

    skos:broader <#plankton> ; 
.

<#picoplankton>
    a skos:Concept, aphia-trait:Trait ;
    skos:inScheme <https://aphia.org/ns/vocab/attribute-trait/> ;
    skos:prefLabel "Picoplankton"@en ;
    skos:definition "The component of the plankton that consists of extremely small organisms, 0,2 to 2 microns (µm) (0,0002 to 0,002 mm) in size; they are too small to catch in a standard plankton net."@en ;

    skos:broader <#plankton> ; 
.

<#femtoplankton>
    a skos:Concept, aphia-trait:Trait ;
    skos:inScheme <https://aphia.org/ns/vocab/attribute-trait/> ;
    skos:prefLabel "Femtoplankton"@en ;
    skos:definition "The component of the plankton that consists of extremely small organisms, 0,02 to 0,2 microns (µm) (0,00002 to 0,0002 mm) in size; they are too small to catch in a standard plankton net."@en ;

    skos:broader <#plankton> ; 
.

<#zooplankton>
    a skos:Concept, aphia-trait:Trait ;
    skos:inScheme <https://aphia.org/ns/vocab/attribute-trait/> ;
    skos:prefLabel "Zooplankton"@en ;
    skos:definition "Plankton obtaining nourishment via heterotrophy. They are incapable of phototrophy; cf. mixoplankton."@en ;

    skos:broader <#plankton> ; 
.

<#phytoplankton>
    a skos:Concept, aphia-trait:Trait ;
    skos:inScheme <https://aphia.org/ns/vocab/attribute-trait/> ;
    skos:prefLabel "Phytoplankton"@en ;
    skos:definition "Plankton obtaining nourishment via photo(auto)trophy and osmo(hetero)trophy. They are incapable of phagotrophy; cf. mixoplankton."@en ;

    skos:broader <#plankton> ; 
.

<#mixoplankton>
    a skos:Concept, aphia-trait:Trait ;
    skos:inScheme <https://aphia.org/ns/vocab/attribute-trait/> ;
    skos:prefLabel "Mixoplankton"@en ;
    skos:definition "Plankton protists capable of obtaining nourishment via photo(auto)trophy and phago(hetero)trophy, as well as via osmo(hetero)trophy."@en ;

    skos:broader <#plankton> ; 
.

<#endosymbiotic_specialist_non_constitutive_mixoplankton>
    a skos:Concept, aphia-trait:Trait ;
    skos:inScheme <https://aphia.org/ns/vocab/attribute-trait/> ;
    skos:prefLabel "Endosymbiotic Specialist Non-Constitutive Mixoplankton"@en ;
    skos:definition "Specialist non-constitutive mixoplankton (SNCMs) are NCMs that acquire their capacity for phototrophy from specific phototrophic prey (cf. GNCM). Endosymbiotic Specialist Non-Constitutive Mixoplankton (eSNCM) are endosymbiotic acquiring phototrophy by harbouring specific phototrophic prey."@en ;

    skos:broader <#mixoplankton> ; 
.

<#constitutive_mixoplankton>
    a skos:Concept, aphia-trait:Trait ;
    skos:inScheme <https://aphia.org/ns/vocab/attribute-trait/> ;
    skos:prefLabel "Constitutive Mixoplankton"@en ;
    skos:definition "Protist plankton with an inherent capacity for phototrophy that can also exhibit phagotrophy."@en ;

    skos:broader <#mixoplankton> ; 
.

<#plastid_specialists_non_constitutive_mixoplankton>
    a skos:Concept, aphia-trait:Trait ;
    skos:inScheme <https://aphia.org/ns/vocab/attribute-trait/> ;
    skos:prefLabel "Plastid Specialists Non-Constitutive Mixoplankton"@en ;
    skos:definition "Specialist non-constitutive mixoplankton (SNCMs) are NCMs that acquire their capacity for phototrophy from specific phototrophic prey (cf. GNCM). Plastid Specialists Non-Constitutive Mixoplankton (pSNCMs) are plastidic specialists acquiring phototrophy from specialist prey type(s)."@en ;

    skos:broader <#mixoplankton> ; 
.

<#general_non_constitutive_mixoplankton>
    a skos:Concept, aphia-trait:Trait ;
    skos:inScheme <https://aphia.org/ns/vocab/attribute-trait/> ;
    skos:prefLabel "General Non-Constitutive Mixoplankton"@en ;
    skos:definition "NCMs that acquire their capacity for phototrophy from general (i.e. non-specific) phototrophic prey (cf. SNCM). Non-constitutive mixoplankton (NCMs) is protist plankton that acquire the capability for phototrophy from consumption (via phagotrophy) of phototrophic prey."@en ;

    skos:broader <#mixoplankton> ; 
.

<#nekton>
    a skos:Concept, aphia-trait:Trait ;
    skos:inScheme <https://aphia.org/ns/vocab/attribute-trait/> ;
    skos:prefLabel "Nekton"@en ;
    skos:definition "Organisms that swim strongly enough to move against the current."@en ;
.

<#neuston>
    a skos:Concept, aphia-trait:Trait ;
    skos:inScheme <https://aphia.org/ns/vocab/attribute-trait/> ;
    skos:prefLabel "Neuston"@en ;
    skos:definition "Organisms that live right at the sea surface but remain underwater."@en ;

    skos:closeMatch ... ; 
.

<#pleuston>
    a skos:Concept, aphia-trait:Trait ;
    skos:inScheme <https://aphia.org/ns/vocab/attribute-trait/> ;
    skos:prefLabel "Pleuston"@en ;
    skos:definition "Organisms that live right at the sea surface, with part of the body projecting into the air."@en ;

    skos:closeMatch ... ; 
.

<#benthopelagic>
    a skos:Concept, aphia-trait:Trait ;
    skos:inScheme <https://aphia.org/ns/vocab/attribute-trait/> ;
    skos:prefLabel "Benthopelagic"@en ;
    skos:definition "Organisms living and feeding near the bottom as well as in midwaters or near the surface. Feeding on benthic as well as free swimming organisms. Many freshwater fish are opportunistic feeders that forage on the bottom as well as in midwater and near the surface, also pertaining to forms which hover or swim just over the floor of the sea, e.g. Halosauridae, Macrouridae, Moridae, Brotulidae; the depth zone about 100 metres off the bottom at all depths below the edge of the continental shelf. "@en ;

    skos:exactMatch ... ; 
.

<#edaphofauna>
    a skos:Concept, aphia-trait:Trait ;
    skos:inScheme <https://aphia.org/ns/vocab/attribute-trait/> ;
    skos:prefLabel "Edaphofauna"@en ;
    skos:definition "Animals that spend a significant portion of their life cycle within a soil profile or at the soil-litter interface"@en ;

    skos:narrower <#edaphofauna> ; 
.

<#macroedaphofauna>
    a skos:Concept, aphia-trait:Trait ;
    skos:inScheme <https://aphia.org/ns/vocab/attribute-trait/> ;
    skos:prefLabel "Marco Edaphofauna"@en ;
    skos:definition "Macro edaphofauna."@en ; 

    skos:broader <#edaphofauna> ; 
.

<#mesoedaphofauna>
    a skos:Concept, aphia-trait:Trait ;
    skos:inScheme <https://aphia.org/ns/vocab/attribute-trait/> ;
    skos:prefLabel "Meso Edaphofauna"@en ;
    skos:definition "Meso edaphofauna."@en ;

    skos:broader <#edaphofauna> ; 
.

<#functional_group_not_applicable>
    a skos:Concept, aphia-trait:Trait ;
    skos:inScheme <https://aphia.org/ns/vocab/attribute-trait/> ;
    skos:prefLabel "Functional group not applicable"@en ;
    skos:definition "The attribute 'functional group' is not applicable for this taxon. This is e.g. used for parasitic taxa, to overwrite the functional group inherited from higher taxa."@en ;
.