@prefix skos: <http://www.w3.org/2004/02/skos/core#> .
@prefix rdfs: <http://www.w3.org/2000/01/rdf-schema#> .
@prefix dct: <http://purl.org/dc/terms/> .

@prefix aphia-trait: <https://aphia.org/ns/attribute-trait/> .

@base <https://aphia.org/ns/term/gamete_type> .

<>
    a skos:Collection ; 
    dct:description "Descriptors of the relative size of gametes."@en ;

    skos:member <#anisogamous> , 
                <#isogamous> , 
                <#oogamous> , 
                <#gamete_type_not_applicable> ,
                <#gamete_type_unknown> ,
                <#gamete_type_unreported> ; 
.

<#anisogamous>
    a skos:Concept, aphia-trait:Trait ;
    skos:inScheme <https://aphia.org/ns/vocab/attribute-trait/> ;
    skos:prefLabel "Anisogamous"@en ;
    skos:definition "Having gametes of dissimilar size, shape or behaviour; cf. isogamous (Lincoln et al., 1998)."@en ;
.
<#isogamous>
    a skos:Concept, aphia-trait:Trait ;
    skos:inScheme <https://aphia.org/ns/vocab/attribute-trait/> ;
    skos:prefLabel "Isogamous"@en ;
    skos:definition "Having gametes that are similar in size, shape and behaviour; having gametes (isogametes) not differentiated into male and female; cf. anisogamous (Lincoln et al., 1998)."@en ;
.
<#oogamous>
    a skos:Concept, aphia-trait:Trait ;
    skos:inScheme <https://aphia.org/ns/vocab/attribute-trait/> ;
    skos:prefLabel "Oogamous"@en ;
    skos:definition "Having a reproduction involving a large, non-motile female gamete (egg cell) and a small, motile male gamete (sperm cell or equivalent), except for red algae in which the male gamete is also non-motile (macroalgae; Womersley, 1987)."@en ;
.
<#gamete_type_not_applicable>
    a skos:Concept, aphia-trait:Trait ;
    skos:inScheme <https://aphia.org/ns/vocab/attribute-trait/> ;
    skos:prefLabel "Gamete type not applicable"@en ;
    skos:definition "The attribute 'gamete type' is not applicable for this taxon."@en ;
.
<#gamete_type_unknown>
    a skos:Concept, aphia-trait:Trait ;
    skos:inScheme <https://aphia.org/ns/vocab/attribute-trait/> ;
    skos:prefLabel "Gamete type unknown"@en ;
    skos:definition "According to literature it is unknown which gamete type this organism has."@en ;
.
<#gamete_type_unreported>
    a skos:Concept, aphia-trait:Trait ;
    skos:inScheme <https://aphia.org/ns/vocab/attribute-trait/> ;
    skos:prefLabel "Gamete type unreported"@en ;
    skos:definition "So far it has not been reported in literature what the gamete type is for this taxon."@en ;
.