@prefix skos: <http://www.w3.org/2004/02/skos/core#> .
@prefix rdfs: <http://www.w3.org/2000/01/rdf-schema#> .
@prefix dct: <http://purl.org/dc/terms/> .

@prefix aphia-trait: <https://aphia.org/ns/attribute-trait/> .

@prefix trait: <https://aphia.org/ns/vocab/attribute-trait/> .

trait:conceptScheme
    a skos:ConceptScheme ;
    rdfs:label "Listing Aphia attributes and traits"@en .

<https://aphia.org/ns/vocab/attribute-trait/>
    a skos:Collection ;
    rdfs:label "Aphia attributes and traits"@en ;
    
    skos:member trait:gametophyte_arrangement ;
.

trait:gametophyte_arrangement
    a skos:Collection ; 
    dct:description "Trait that describes the male and female reproductive structures."@en ;

    skos:member trait:dioecious , 
                trait:dioicous , 
                trait:mixed , 
                trait:monoecious , 
                trait:monoicous ,
                trait:gametophyte_arrangement_not_applicable ,
                trait:gametophyte_arrangement_unknown ,
                trait:gametophyte_arrangement_unreported ; 
.

trait:dioecious
    a skos:Concept, aphia-trait:Trait ;
    skos:inScheme trait:conceptScheme ;
    skos:prefLabel "Dioecious"@en ;
    skos:definition "When male and female reproductive structures are formed on the separate individual and the sex is determined in diploid phase."@en ;
.

trait:dioicous
    a skos:Concept, aphia-trait:Trait ;
    skos:inScheme trait:conceptScheme ;
    skos:prefLabel "Dioicous"@en ;
    skos:definition "When male and female reproductive structures are formed on the separate individual and the sex is determined in haploid phase."@en ;
.

trait:mixed
    a skos:Concept, aphia-trait:Trait ;
    skos:inScheme trait:conceptScheme ;
    skos:prefLabel "Mixed"@en ;
    skos:definition "With individuals bearing only male or female reproductive structures and indivduals bearing both male and female reproductive structures in one species."@en ;
.

trait:monoecious
    a skos:Concept, aphia-trait:Trait ;
    skos:inScheme trait:conceptScheme ;
    skos:prefLabel "Monoecious"@en ;
    skos:definition "When male and female reproductive structures are formed on same individuals and the sex is determined in diploid phase."@en ;
.

trait:monoicous
    a skos:Concept, aphia-trait:Trait ;
    skos:inScheme trait:conceptScheme ;
    skos:prefLabel "Monoicous"@en ;
    skos:definition "When male and female reproductive structures are formed on same individuals and the sex is determined in haploid phase."@en ;
.

trait:gametophyte_arrangement_not_applicable
    a skos:Concept, aphia-trait:Trait ;
    skos:inScheme trait:conceptScheme ;
    skos:prefLabel "Gametophyte arrangement not applicable"@en ;
    skos:definition "The attribute 'gametophyte arrangement' is not applicable for this taxon."@en ;
.

trait:gametophyte_arrangement_unknown
    a skos:Concept, aphia-trait:Trait ;
    skos:inScheme trait:conceptScheme ;
    skos:prefLabel "Unknown gametophyte arrangement"@en ;
    skos:definition "According to literature it is unknown which gametophyte arrangement this organism has."@en ;
.

trait:gametophyte_arrangement_unreported
    a skos:Concept, aphia-trait:Trait ;
    skos:inScheme trait:conceptScheme ;
    skos:prefLabel "Unreported gametophyte arrangement"@en ;
    skos:definition "So far it has not been reported in literature what the gametophyte arrangement is for this taxon."@en ;
.