@prefix skos: <http://www.w3.org/2004/02/skos/core#> .
@prefix rdfs: <http://www.w3.org/2000/01/rdf-schema#> .
@prefix dct: <http://purl.org/dc/terms/> .

@prefix aphia-trait: <https://aphia.org/ns/attribute-trait/> .

@prefix trait: <https://aphia.org/ns/vocab/attribute-trait/> .

trait:conceptScheme
    a skos:ConceptScheme ;
    rdfs:label "Listing Aphia attributes and traits"@en .

<https://aphia.org/ns/vocab/attribute-trait/>
    a skos:Collection ;
    rdfs:label "Aphia attributes and traits"@en ;
    
    skos:member trait:gamete_type ;
.

trait:gamete_type
    a skos:Collection ; 
    dct:description "Descriptors of the relative size of gametes."@en ;

    skos:member trait:anisogamous , 
                trait:isogamous , 
                trait:oogamous , 
                trait:gamete_type_not_applicable ,
                trait:gamete_type_unknown ,
                trait:gamete_type_unreported ; 
.

trait:anisogamous
    a skos:Concept, aphia-trait:Trait ;
    skos:inScheme trait:conceptScheme ;
    skos:prefLabel "Anisogamous"@en ;
    skos:definition "Having gametes of dissimilar size, shape or behaviour; cf. isogamous (Lincoln et al., 1998)."@en ;
.
trait:isogamous
    a skos:Concept, aphia-trait:Trait ;
    skos:inScheme trait:conceptScheme ;
    skos:prefLabel "Isogamous"@en ;
    skos:definition "Having gametes that are similar in size, shape and behaviour; having gametes (isogametes) not differentiated into male and female; cf. anisogamous (Lincoln et al., 1998)."@en ;
.
trait:oogamous
    a skos:Concept, aphia-trait:Trait ;
    skos:inScheme trait:conceptScheme ;
    skos:prefLabel "Oogamous"@en ;
    skos:definition "Having a reproduction involving a large, non-motile female gamete (egg cell) and a small, motile male gamete (sperm cell or equivalent), except for red algae in which the male gamete is also non-motile (macroalgae; Womersley, 1987)."@en ;
.
trait:gamete_type_not_applicable
    a skos:Concept, aphia-trait:Trait ;
    skos:inScheme trait:conceptScheme ;
    skos:prefLabel "Gamete type not applicable"@en ;
    skos:definition "The attribute 'gamete type' is not applicable for this taxon."@en ;
.
trait:gamete_type_unknown
    a skos:Concept, aphia-trait:Trait ;
    skos:inScheme trait:conceptScheme ;
    skos:prefLabel "Gamete type unknown"@en ;
    skos:definition "According to literature it is unknown which gamete type this organism has."@en ;
.
trait:gamete_type_unreported
    a skos:Concept, aphia-trait:Trait ;
    skos:inScheme trait:conceptScheme ;
    skos:prefLabel "Gamete type unreported"@en ;
    skos:definition "So far it has not been reported in literature what the gamete type is for this taxon."@en ;
.