@prefix skos: <http://www.w3.org/2004/02/skos/core#> .
@prefix rdfs: <http://www.w3.org/2000/01/rdf-schema#> .
@prefix dct: <http://purl.org/dc/terms/> .

@prefix aphia-trait: <https://aphia.org/ns/attribute-trait/> .

@base <https://aphia.org/ns/term/gametophyte_arrangement> .

<>
    a skos:Collection ; 
    dct:description "Trait that describes the male and female reproductive structures."@en ;

    skos:member <#dioecious> , 
                <#dioicous> , 
                <#mixed> , 
                <#monoecious> , 
                <#monoicous> ,
                <#gametophyte_arrangement_not_applicable> ,
                <#gametophyte_arrangement_unknown> ,
                <#gametophyte_arrangement_unreported> ; 
.

<#dioecious>
    a skos:Concept, aphia-trait:Trait ;
    skos:inScheme <https://aphia.org/ns/vocab/attribute-trait/> ;
    skos:prefLabel "Dioecious"@en ;
    skos:definition "When male and female reproductive structures are formed on the separate individual and the sex is determined in diploid phase."@en ;
.

<#dioicous>
    a skos:Concept, aphia-trait:Trait ;
    skos:inScheme <https://aphia.org/ns/vocab/attribute-trait/> ;
    skos:prefLabel "Dioicous"@en ;
    skos:definition "When male and female reproductive structures are formed on the separate individual and the sex is determined in haploid phase."@en ;
.

<#mixed>
    a skos:Concept, aphia-trait:Trait ;
    skos:inScheme <https://aphia.org/ns/vocab/attribute-trait/> ;
    skos:prefLabel "Mixed"@en ;
    skos:definition "With individuals bearing only male or female reproductive structures and indivduals bearing both male and female reproductive structures in one species."@en ;
.

<#monoecious>
    a skos:Concept, aphia-trait:Trait ;
    skos:inScheme <https://aphia.org/ns/vocab/attribute-trait/> ;
    skos:prefLabel "Monoecious"@en ;
    skos:definition "When male and female reproductive structures are formed on same individuals and the sex is determined in diploid phase."@en ;
.

<#monoicous>
    a skos:Concept, aphia-trait:Trait ;
    skos:inScheme <https://aphia.org/ns/vocab/attribute-trait/> ;
    skos:prefLabel "Monoicous"@en ;
    skos:definition "When male and female reproductive structures are formed on same individuals and the sex is determined in haploid phase."@en ;
.

<#gametophyte_arrangement_not_applicable>
    a skos:Concept, aphia-trait:Trait ;
    skos:inScheme <https://aphia.org/ns/vocab/attribute-trait/> ;
    skos:prefLabel "Gametophyte arrangement not applicable"@en ;
    skos:definition "The attribute 'gametophyte arrangement' is not applicable for this taxon."@en ;
.

<#gametophyte_arrangement_unknown>
    a skos:Concept, aphia-trait:Trait ;
    skos:inScheme <https://aphia.org/ns/vocab/attribute-trait/> ;
    skos:prefLabel "Unknown gametophyte arrangement"@en ;
    skos:definition "According to literature it is unknown which gametophyte arrangement this organism has."@en ;
.

<#gametophyte_arrangement_unreported>
    a skos:Concept, aphia-trait:Trait ;
    skos:inScheme <https://aphia.org/ns/vocab/attribute-trait/> ;
    skos:prefLabel "Unreported gametophyte arrangement"@en ;
    skos:definition "So far it has not been reported in literature what the gametophyte arrangement is for this taxon."@en ;
.