@prefix skos: <http://www.w3.org/2004/02/skos/core#> .
@prefix rdfs: <http://www.w3.org/2000/01/rdf-schema#> .
@prefix dct: <http://purl.org/dc/terms/> .

@prefix aphia-trait: <https://aphia.org/ns/attribute-trait/> .

@prefix trait: <https://aphia.org/ns/vocab/attribute-trait/> .


trait:life_span
    a skos:Collection ; 
    dct:description "Longevity; the maximum or mean duration of life of an individual or group."@en ;

    skos:member trait:annual , 
                    trait:ephemeral ,
                trait:perennial , 
                    trait:long_perennial ,
                    trait:short_perennial ,
                trait:unreported_life_span ;

    skos:exactMatch ... ; 
.

trait:annual
    a skos:Concept, aphia-trait:Trait ;
    skos:inScheme trait:conceptScheme ;
    skos:prefLabel "Annual"@en ;
    skos:definition "(1) Appl. structures or growth features that are marked off or completed yearly; (2) living for a year only; (3) completing life-cycle in a year from germination; (4) n. plant that completes its life-cycle in a year. (Henderson's Dictionary of Biology; Lawrence, 2005). Thallus which survives only one growing season (less than 1 year) (macroalgae; Womersley, 1987)."@en ;

    skos:narrower trait:ephemeral ;

    skos:exactMatch ... ; 
.

trait:ephemeral
    a skos:Concept, aphia-trait:Trait ;
    skos:inScheme trait:conceptScheme ;
    skos:prefLabel "Ephemeral"@en ;
    skos:definition "(1) Short-lived; (2) taking place once only, appl. plant movements as expanding buds; (3) completing life-cycle within a brief period; (4) n. a short-lived plant or animal species (Henderson's Dictionary of Biology; Lawrence, 2005). Thallus which survives for only a few weeks (less than 1 month) (macroalgae; Womersley, 1987)."@en ;

    skos:broader trait:annual ; 

    skos:exactMatch ... ; 
.

trait:perennial
    a skos:Concept, aphia-trait:Trait ;
    skos:inScheme trait:conceptScheme ;
    skos:prefLabel "Perennial"@en ;
    skos:definition "Plant which persists for several years."@en ;

    skos:narrower trait:long_perennial , trait:short_perennial ; 

    skos:exactMatch ... ; 
.

trait:long_perennial
    a skos:Concept, aphia-trait:Trait ;
    skos:inScheme trait:conceptScheme ;
    skos:prefLabel "Long perennial"@en ;
    skos:definition "Thallus or part thereof with a lifespan exceeding 3 years (more than 3 years) (macroalgae; Definition composed by Line Le Gall, Olivier De Clerck, Sofie Vranken and Marine Robuchon, based on diverse literature sources, in the framework of compiling macroalgae traits.)"@en ;

    skos:broader trait:perennial ; 

    skos:exactMatch ... ; 
.

trait:short_perennial
    a skos:Concept, aphia-trait:Trait ;
    skos:inScheme trait:conceptScheme ;
    skos:prefLabel "Short perennial"@en ;
    skos:definition "Thallus or part thereof with a lifespan exceeding 1 year but under 3 years (macroalgae; Definition composed by Line Le Gall, Olivier De Clerck, Sofie Vranken and Marine Robuchon, based on diverse literature sources, in the framework of compiling macroalgae traits.)"@en ;

    skos:broader trait:perennial ; 

    skos:exactMatch ... ; 
.

trait:unreported_life_span
    a skos:Concept, aphia-trait:Trait ;
    skos:inScheme trait:conceptScheme ;
    skos:prefLabel "Unreported life span"@en ;
    skos:definition "So far it has not been reported in literature which life span this organism has."@en ;
.