@prefix skos: <http://www.w3.org/2004/02/skos/core#> .
@prefix rdfs: <http://www.w3.org/2000/01/rdf-schema#> .
@prefix dct: <http://purl.org/dc/terms/> .

@prefix aphia-trait: <https://aphia.org/ns/attribute-trait/> .

@base <https://aphia.org/ns/term/life_cycle> .

<>
    a skos:Collection ; 
    dct:description "The type of life cycle an organism has. Life cycle according to Lincoln et al., 1998: 1: The sequence of events from the origin as a zygote, to the death of an individual. 2: Those stages through which an organism passes between the production of gametes by one generation and the production of gametes by the next."@en ;

    skos:member <#diplontic> , 
                <#haplodiplontic> , 
                    <#heteromorphic> , 
                    <#isomorphic> , 
                    <#haplodiplontic_not_applicable> , 
                    <#haplodiplontic_unknown> , 
                    <#haplodiplontic_unreported> , 
                <#haplontic> , 
                <#life_cycle_unknown> , 
                <#life_cycle_unreported> ; 

    skos:closeMatch <https://kos.lifewatch.eu/thesauri/traits/c_d2f533e2> ; 
.

<#diplontic>
    a skos:Concept, aphia-trait:Trait ;
    skos:inScheme <https://aphia.org/ns/vocab/attribute-trait/> ;
    skos:prefLabel "Diplontic"@en ;
    skos:definition "Having a life cycle in which the direct products of meiosis act as gametes; only the gametes of diplonts are haploid; cf. haplont (Lincoln et al., 1998)."@en ;

    skos:exactMatch <https://kos.lifewatch.eu/thesauri/traits/c_34dd49a6> ; 
.
<#haplodiplontic>
    a skos:Concept, aphia-trait:Trait ;
    skos:inScheme <https://aphia.org/ns/vocab/attribute-trait/> ;
    skos:prefLabel "Haplodiplontic"@en ;
    skos:definition "Having a life cycle with alternating free-living gametophyte and sporophyte phases (macroalgae; Womersley, 1987)."@en ;

    skos:narrower <#heteromorphic> , <#haplodiplontic_not_applicable> , <#haplodiplontic_unknown> , <#haplodiplontic_unreported> ;

    skos:exactMatch <https://kos.lifewatch.eu/thesauri/traits/c_92fb480e> ; 
.
<#heteromorphic>
    a skos:Concept, aphia-trait:Trait ;
    skos:inScheme <https://aphia.org/ns/vocab/attribute-trait/> ;
    skos:prefLabel "Heteromorphic"@en ;
    skos:definition "Organisms with the gametophyte and sporophyte of different morphology and size (macroalgae; Womersley, 1987). Having different forms at different times or at different stages of the life cycle; used of a plant having an alternation of vegetatively dissimilar generations; heteromorphous; cf. homomorphic (Lincoln et al., 1998)."@en ;

    skos:closeMatch <https://kos.lifewatch.eu/thesauri/traits/c_5237d7a1> ; 
.
<#isomorphic>
    a skos:Concept, aphia-trait:Trait ;
    skos:inScheme <https://aphia.org/ns/vocab/attribute-trait/> ;
    skos:prefLabel "Isomorphic"@en ;
    skos:definition "Organisms with the gametophyte and sporophyte of similar morphology and size (macroalgae; Womersley, 1987). Used of a plant having an alternation between diploid and haploid generations which are morphologically similar in appearance; homomoprhic; isomorphous; cf. heteromorphic (Lincoln et al., 1998)."@en ;

    skos:closeMatch <https://kos.lifewatch.eu/thesauri/traits/c_7a809af2> ; 
.
<#haplodiplontic_not_applicable>
    a skos:Concept, aphia-trait:Trait ;
    skos:inScheme <https://aphia.org/ns/vocab/attribute-trait/> ;
    skos:prefLabel "Haplodiplontic not applicable"@en ;
    skos:definition "It is not applicable whether this taxon is heteromorphic or isomorphic."@en ;
.
<#haplodiplontic_unknown>
    a skos:Concept, aphia-trait:Trait ;
    skos:inScheme <https://aphia.org/ns/vocab/attribute-trait/> ;
    skos:prefLabel "Haplodiplontic unknown"@en ;
    skos:definition "According to literature it is unknown whether this organism is heteromorphic or isomorphic."@en ;
.
<#haplodiplontic_unreported>
    a skos:Concept, aphia-trait:Trait ;
    skos:inScheme <https://aphia.org/ns/vocab/attribute-trait/> ;
    skos:prefLabel "Haplodiplontic unreported"@en ;
    skos:definition "So far it has not been reported in literature whether this taxon is heteromorphic or isomorphic."@en ;
.
<#haplontic>
    a skos:Concept, aphia-trait:Trait ;
    skos:inScheme <https://aphia.org/ns/vocab/attribute-trait/> ;
    skos:prefLabel "Haplontic"@en ;
    skos:definition "Having a life cycle in which meiosis occurs in the zygote to produce the haploid phase; only the zygote of the haplonts is diploid; cf. diplont."@en ;

    skos:exactMatch <https://kos.lifewatch.eu/thesauri/traits/c_2d18402c> ; 
.
<#life_cycle_unknown>
    a skos:Concept, aphia-trait:Trait ;
    skos:inScheme <https://aphia.org/ns/vocab/attribute-trait/> ;
    skos:prefLabel "Unknown life cycle"@en ;
    skos:definition "According to literature it is unknown what life cycle this organism has."@en ;
.
<#life_cycle_unreported>
    a skos:Concept, aphia-trait:Trait ;
    skos:inScheme <https://aphia.org/ns/vocab/attribute-trait/> ;
    skos:prefLabel "Unreported life cycle"@en ;
    skos:definition "So far it has not been reported in literature what life cycle this taxon has."@en ;
.