@prefix skos: <http://www.w3.org/2004/02/skos/core#> .
@prefix rdfs: <http://www.w3.org/2000/01/rdf-schema#> .
@prefix dct: <http://purl.org/dc/terms/> .

@prefix aphia-trait: <https://aphia.org/ns/attribute-trait/> .

@base <https://aphia.org/ns/term/reproductive_frequency> .

<>
    a skos:Collection ; 
    dct:description "Trait that describes the fertility period of an organism."@en ;

    skos:member <#all_over_the_year> , 
                <#one_long_period_a_year> , 
                <#one_short_period_a_year> , 
                <#several_long_periods_a_year> , 
                <#several_short_periods_a_year> ; 

    skos:exactMatch ... ; 
.

<#all_over_the_year>
    a skos:Concept, aphia-trait:Trait ;
    skos:inScheme <https://aphia.org/ns/vocab/attribute-trait/> ;
    skos:prefLabel "All over the year"@en ;
    skos:definition "Fertile individuals observed all over the year. (Definition composed by Line Le Gall, Olivier De Clerck, Sofie Vranken and Marine Robuchon, based on diverse literature sources, in the framework of compiling macroalgae traits.)"@en ;
.

<#one_long_period_a_year>
    a skos:Concept, aphia-trait:Trait ;
    skos:inScheme <https://aphia.org/ns/vocab/attribute-trait/> ;
    skos:prefLabel "One long period a year"@en ;
    skos:definition "A unique fertility period lasting more than 1 month. (Definition composed by Line Le Gall, Olivier De Clerck, Sofie Vranken and Marine Robuchon, based on diverse literature sources, in the framework of compiling macroalgae traits.)"@en ;
.

<#one_short_period_a_year>
    a skos:Concept, aphia-trait:Trait ;
    skos:inScheme <https://aphia.org/ns/vocab/attribute-trait/> ;
    skos:prefLabel "One short period a year"@en ;
    skos:definition "A unique fertility period lasting less than 1 month. (Definition composed by Line Le Gall, Olivier De Clerck, Sofie Vranken and Marine Robuchon, based on diverse literature sources, in the framework of compiling macroalgae traits.)"@en ;
.

<#several_long_periods_a_year>
    a skos:Concept, aphia-trait:Trait ;
    skos:inScheme <https://aphia.org/ns/vocab/attribute-trait/> ;
    skos:prefLabel "Several long periods a year"@en ;
    skos:definition "Several distinct fertility periods lasting more than 1 month each. (Definition composed by Line Le Gall, Olivier De Clerck, Sofie Vranken and Marine Robuchon, based on diverse literature sources, in the framework of compiling macroalgae traits.)"@en ;
.

<#several_short_periods_a_year>
    a skos:Concept, aphia-trait:Trait ;
    skos:inScheme <https://aphia.org/ns/vocab/attribute-trait/> ;
    skos:prefLabel "Several short periods a year"@en ;
    skos:definition "Several distinct fertility periods lasting less than 1 month each."@en ;
.