@prefix skos: <http://www.w3.org/2004/02/skos/core#> .
@prefix rdfs: <http://www.w3.org/2000/01/rdf-schema#> .
@prefix dct: <http://purl.org/dc/terms/> .

@prefix aphia-trait: <https://aphia.org/ns/attribute-trait/> .

@prefix trait: <https://aphia.org/ns/vocab/attribute-trait/> .


trait:spawning
    a skos:Collection ; 
    dct:description "The release of gametes or eggs into the water (Lincoln et al., 1998)."@en ;

    skos:member trait:fertilisation_in_the_water_column , 
                trait:fertilisation_on_female_gametophyte , 
                trait:spawning_not_applicable , 
                trait:spawning_unknown , 
                trait:spawning_unreported ; 
.

trait:fertilisation_in_the_water_column
    a skos:Concept, aphia-trait:Trait ;
    skos:inScheme trait:conceptScheme ;
    skos:prefLabel "Fertilisation in the water column"@en ;
    skos:definition "Fertilization with gametes released in the water column."@en ;
.
trait:fertilisation_on_female_gametophyte
    a skos:Concept, aphia-trait:Trait ;
    skos:inScheme trait:conceptScheme ;
    skos:prefLabel "Fertilisation on female gametophyte"@en ;
    skos:definition "Female gamete retained on the female gametophyte (e.g. Rhodophyta)."@en ;
.
trait:spawning_not_applicable
    a skos:Concept, aphia-trait:Trait ;
    skos:inScheme trait:conceptScheme ;
    skos:prefLabel "Spawning not applicable"@en ;
    skos:definition "The attribute 'spawning' is not applicable for this taxon."@en ;
.
trait:spawning_unknown
    a skos:Concept, aphia-trait:Trait ;
    skos:inScheme trait:conceptScheme ;
    skos:prefLabel "Spawning unknown"@en ;
    skos:definition "According to literature it is unknown which spawning mechanism this organism has."@en ;
.
trait:spawning_unreported
    a skos:Concept, aphia-trait:Trait ;
    skos:inScheme trait:conceptScheme ;
    skos:prefLabel "Spawning unreported"@en ;
    skos:definition "So far it has not been reported in literature whether or not there is spawning for this taxon."@en ;
.