<?xml version="1.0"?>
<rdf:RDF xmlns="https://aphia.org/ns/attribute-trait/"
     xml:base="https://aphia.org/ns/attribute-trait/"
     xmlns:dct="http://purl.org/dc/terms/"
     xmlns:owl="http://www.w3.org/2002/07/owl#"
     xmlns:rdf="http://www.w3.org/1999/02/22-rdf-syntax-ns#"
     xmlns:xml="http://www.w3.org/XML/1998/namespace"
     xmlns:xsd="http://www.w3.org/2001/XMLSchema#"
     xmlns:foaf="http://xmlns.com/foaf/0.1/"
     xmlns:prov="http://www.w3.org/ns/prov#"
     xmlns:rdfs="http://www.w3.org/2000/01/rdf-schema#"
     xmlns:skos="http://www.w3.org/2004/02/skos/core#">
    <owl:Ontology rdf:about="https://aphia.org/ns/attribute-trait">
        <owl:versionIRI rdf:resource="https://aphia.org/ns/attribute-trait/0.3"/>
        <owl:imports rdf:resource="https://aphia.org/ns/top-level"/>
        <dct:creator rdf:resource="https://aphia.org/resource/organisation/dv"/>
        <dct:creator rdf:resource="https://ror.org/0496vr396"/>
        <dct:creator rdf:resource="https://w3id.org/italia/data/organization/support-unit/cnr-Z6HZEH/stlab"/>
        <dct:description xml:lang="nl">Dit is de attribuut- en eigenschapontologie van het APHIA-ontologienetwerk. Het importeert de ontologie op het hoogste niveau van het APHIA-netwerk en stelt het gebruik voor van een specifiek ontwerppatroon &apos;Beschrijving&apos; om attributen, eigenschappen en hun contextinformatie te modelleren die mogelijk niet a priori bekend zijn en in de toekomst worden uitgebreid.</dct:description>
        <dct:description xml:lang="it">Questa è l&apos;ontologia degli attributi e dei tratti (delle specie) della rete di ontologie APHIA. Importa l&apos;ontologia di primo livello della rete APHIA e propone l&apos;uso di un ontology design pattern specifico &apos;Descrizione&apos; per poter modellare attributi, tratti e loro informazioni di contesto che potrebbero anche non essere noti a priori ed estesi in futuro.</dct:description>
        <dct:description xml:lang="en">This is the attribute and trait of species ontology of the APHIA ontology network. It imports the top-level ontology of the APHIA network and proposes the use of a specific ontology design pattern &apos;Description&apos; in order to model attributes, traits and their context information that may not even be known a priori and extended in the future.</dct:description>
        <dct:issued rdf:datatype="http://www.w3.org/2001/XMLSchema#date">2023-08-30</dct:issued>
        <dct:language rdf:resource="http://publications.europa.eu/resource/authority/language/ENG"/>
        <dct:language rdf:resource="http://publications.europa.eu/resource/authority/language/ITA"/>
        <dct:language rdf:resource="http://publications.europa.eu/resource/authority/language/NLD"/>
        <dct:license rdf:resource="http://publications.europa.eu/resource/authority/licence/CC_BY_4_0"/>
        <dct:modified>2025-05-28</dct:modified>
        <dct:title xml:lang="en">APHIA - (Species) attributes and traits ontology</dct:title>
        <dct:title xml:lang="it">APHIA - Ontologia degli attributi e dei tratti delle specie</dct:title>
        <dct:title xml:lang="nl">APHIA - ontologie van (soort)eigenschappen en kenmerken</dct:title>
        <rdfs:comment xml:lang="nl">Dit is de attribuut- en eigenschapontologie van het APHIA-ontologienetwerk. Het importeert de ontologie op het hoogste niveau van het APHIA-netwerk en stelt het gebruik voor van een specifiek ontwerppatroon &apos;Beschrijving&apos; om attributen, eigenschappen en hun contextinformatie te modelleren die mogelijk niet a priori bekend zijn en in de toekomst worden uitgebreid.</rdfs:comment>
        <rdfs:comment xml:lang="it">Questa è l&apos;ontologia degli attributi e dei tratti (delle specie) della rete di ontologie APHIA. Importa l&apos;ontologia di primo livello della rete APHIA e propone l&apos;uso di un ontology design pattern specifico &apos;Descrizione&apos; per poter modellare attributi, tratti e loro informazioni di contesto che potrebbero anche non essere noti a priori ed estesi in futuro.</rdfs:comment>
        <rdfs:comment xml:lang="en">This is the attribute and trait of species ontology of the APHIA ontology network. It imports the top-level ontology of the APHIA network and proposes the use of a specific ontology design pattern &apos;Description&apos; in order to model attributes, traits and their context information that may not even be known a priori and extended in the future.</rdfs:comment>
        <rdfs:label xml:lang="en">APHIA - (Species) attributes and traits ontology</rdfs:label>
        <rdfs:label xml:lang="it">APHIA - Ontologia degli attributi e dei tratti delle specie</rdfs:label>
        <rdfs:label xml:lang="nl">APHIA - ontologie van (soort)eigenschappen en kenmerken</rdfs:label>
        <owl:versionInfo xml:lang="nl">Derde versie 0.3 - hiërarchie-eigenschappen geïntroduceerd voor SpecificationContext en TaxonCharacteristic</owl:versionInfo>
        <owl:versionInfo xml:lang="it">Terza versione 0.3 - introdotte le proprietà di gerarchia per SpecificationContext e TaxonCharacteristic</owl:versionInfo>
        <owl:versionInfo xml:lang="en">Third version 0.3 - introduced hierarchy properties for SpecificationContext and TaxonCharacteristic</owl:versionInfo>
    </owl:Ontology>
    


    <!-- 
    ///////////////////////////////////////////////////////////////////////////////////////
    //
    // Annotation properties
    //
    ///////////////////////////////////////////////////////////////////////////////////////
     -->

    


    <!-- http://purl.org/dc/terms/creator -->

    <owl:AnnotationProperty rdf:about="http://purl.org/dc/terms/creator"/>
    


    <!-- http://purl.org/dc/terms/description -->

    <owl:AnnotationProperty rdf:about="http://purl.org/dc/terms/description"/>
    


    <!-- http://purl.org/dc/terms/issued -->

    <owl:AnnotationProperty rdf:about="http://purl.org/dc/terms/issued"/>
    


    <!-- http://purl.org/dc/terms/language -->

    <owl:AnnotationProperty rdf:about="http://purl.org/dc/terms/language"/>
    


    <!-- http://purl.org/dc/terms/license -->

    <owl:AnnotationProperty rdf:about="http://purl.org/dc/terms/license"/>
    


    <!-- http://purl.org/dc/terms/modified -->

    <owl:AnnotationProperty rdf:about="http://purl.org/dc/terms/modified"/>
    


    <!-- http://purl.org/dc/terms/title -->

    <owl:AnnotationProperty rdf:about="http://purl.org/dc/terms/title"/>
    


    <!-- http://www.w3.org/2002/07/owl#maxQualifiedCardinality -->

    <owl:AnnotationProperty rdf:about="http://www.w3.org/2002/07/owl#maxQualifiedCardinality"/>
    


    <!-- http://www.w3.org/ns/prov#wasDerivedFrom -->

    <owl:AnnotationProperty rdf:about="http://www.w3.org/ns/prov#wasDerivedFrom"/>
    


    <!-- http://www.w3.org/ns/prov#wasInfluencedBy -->

    <owl:AnnotationProperty rdf:about="http://www.w3.org/ns/prov#wasInfluencedBy"/>
    


    <!-- http://xmlns.com/foaf/0.1/name -->

    <owl:AnnotationProperty rdf:about="http://xmlns.com/foaf/0.1/name"/>
    


    <!-- 
    ///////////////////////////////////////////////////////////////////////////////////////
    //
    // Datatypes
    //
    ///////////////////////////////////////////////////////////////////////////////////////
     -->

    


    <!-- http://www.w3.org/2001/XMLSchema#date -->

    <rdfs:Datatype rdf:about="http://www.w3.org/2001/XMLSchema#date"/>
    


    <!-- 
    ///////////////////////////////////////////////////////////////////////////////////////
    //
    // Object Properties
    //
    ///////////////////////////////////////////////////////////////////////////////////////
     -->

    


    <!-- http://purl.org/dc/terms/source -->

    <owl:ObjectProperty rdf:about="http://purl.org/dc/terms/source"/>
    


    <!-- http://www.ontologydesignpatterns.org/ont/dul/DUL.owl#associatedWith -->

    <owl:ObjectProperty rdf:about="http://www.ontologydesignpatterns.org/ont/dul/DUL.owl#associatedWith"/>
    


    <!-- http://www.ontologydesignpatterns.org/ont/dul/DUL.owl#defines -->

    <owl:ObjectProperty rdf:about="http://www.ontologydesignpatterns.org/ont/dul/DUL.owl#defines"/>
    


    <!-- http://www.ontologydesignpatterns.org/ont/dul/DUL.owl#describes -->

    <owl:ObjectProperty rdf:about="http://www.ontologydesignpatterns.org/ont/dul/DUL.owl#describes"/>
    


    <!-- http://www.ontologydesignpatterns.org/ont/dul/DUL.owl#isDescribedBy -->

    <owl:ObjectProperty rdf:about="http://www.ontologydesignpatterns.org/ont/dul/DUL.owl#isDescribedBy"/>
    


    <!-- http://www.ontologydesignpatterns.org/ont/dul/DUL.owl#isRelatedToDescription -->

    <owl:ObjectProperty rdf:about="http://www.ontologydesignpatterns.org/ont/dul/DUL.owl#isRelatedToDescription"/>
    


    <!-- https://aphia.org/ns/attribute-trait/definesParameter -->

    <owl:ObjectProperty rdf:about="https://aphia.org/ns/attribute-trait/definesParameter">
        <rdfs:subPropertyOf rdf:resource="http://www.ontologydesignpatterns.org/ont/dul/DUL.owl#defines"/>
        <rdfs:domain rdf:resource="https://aphia.org/ns/attribute-trait/SpecificationContext"/>
        <rdfs:range rdf:resource="http://www.ontologydesignpatterns.org/ont/dul/DUL.owl#Parameter"/>
        <rdfs:comment xml:lang="nl">Eigenschap gebruikt om een parameter te specificeren in de extra specificatie bij het beschrijven van kenmerken en eigenschappen. In essentie is het de eigenschap die toelaat om parameters zoals geslacht, geografische eenheid, levensfase enz. aan te duiden voor elk kenmerk en eigenschap.</rdfs:comment>
        <rdfs:comment xml:lang="en">Property used to specify a parameter in the extra specification when describing attributes and traits. In essence, it is the property that allows one to indicate parameter such gender, geographical unit, life stage etc. for each attribute and trait.</rdfs:comment>
        <rdfs:comment xml:lang="it">Proprietà utilizzata per specificare un parametro nella specifica aggiuntiva quando si descrivono attributi e tratti delle specie. In sostanza, è la proprietà che consente di indicare parametri quali il sesso, l&apos;unità geografica, lo stadio di vita, ecc. per ogni attributo e tratto.</rdfs:comment>
        <rdfs:isDefinedBy rdf:resource="https://aphia.org/ns/attribute-trait"/>
        <rdfs:label xml:lang="en">defines parameter</rdfs:label>
        <rdfs:label xml:lang="nl">definieert parameter</rdfs:label>
        <rdfs:label xml:lang="it">definisce parametro</rdfs:label>
    </owl:ObjectProperty>
    


    <!-- https://aphia.org/ns/attribute-trait/hasAdditionalDescription -->

    <owl:ObjectProperty rdf:about="https://aphia.org/ns/attribute-trait/hasAdditionalDescription">
        <rdfs:subPropertyOf rdf:resource="http://www.ontologydesignpatterns.org/ont/dul/DUL.owl#isDescribedBy"/>
        <owl:inverseOf rdf:resource="https://aphia.org/ns/attribute-trait/isAdditionalDescriptionOf"/>
        <rdfs:domain rdf:resource="https://aphia.org/ns/taxon-name/Taxon"/>
        <rdfs:range rdf:resource="https://aphia.org/ns/attribute-trait/TaxonDescription"/>
        <rdfs:comment xml:lang="nl">Eigenschap gebruikt om de beschrijving van het taxon weer te geven in termen van kenmerken en eigenschappen, en gerelateerde extra specificaties met parameters zoals geslacht, geografische eenheden, levensfase, enz.).</rdfs:comment>
        <rdfs:comment xml:lang="en">Property used to represent the description of the taxon in terms of attributes and traits, and related extra specifications with parameters such as gender, geographical units, lifestage, etc.).</rdfs:comment>
        <rdfs:comment xml:lang="it">Proprietà utilizzata per rappresentare la descrizione del taxon in termini di attributi e tratti, e relative specifiche ulteriori con parametri quali sesso, unità geografiche, stadio di vita, ecc.).</rdfs:comment>
        <rdfs:isDefinedBy rdf:resource="https://aphia.org/ns/attribute-trait"/>
        <rdfs:label xml:lang="it">ha ulteriore descrizione</rdfs:label>
        <rdfs:label xml:lang="en">has additional description</rdfs:label>
        <rdfs:label xml:lang="nl">heeft aanvullende beschrijving</rdfs:label>
    </owl:ObjectProperty>
    


    <!-- https://aphia.org/ns/attribute-trait/hasExtraSpecification -->

    <owl:ObjectProperty rdf:about="https://aphia.org/ns/attribute-trait/hasExtraSpecification">
        <rdfs:subPropertyOf rdf:resource="http://www.ontologydesignpatterns.org/ont/dul/DUL.owl#isRelatedToDescription"/>
        <rdfs:domain rdf:resource="https://aphia.org/ns/attribute-trait/TaxonDescription"/>
        <rdfs:range rdf:resource="https://aphia.org/ns/attribute-trait/SpecificationContext"/>
        <rdfs:comment xml:lang="en">Property used to represent the occurrence of the species in its documented attribute-trait.</rdfs:comment>
        <rdfs:comment xml:lang="it">Proprietà utilizzata per rappresentare la presenza della specie nella sua distribuzione documentata.</rdfs:comment>
        <rdfs:isDefinedBy rdf:resource="https://aphia.org/ns/attribute-trait"/>
        <rdfs:label xml:lang="it">ha specifica aggiuntiva</rdfs:label>
        <rdfs:label xml:lang="en">has extra specification</rdfs:label>
        <rdfs:label xml:lang="nl">heeft extra specificatie</rdfs:label>
    </owl:ObjectProperty>
    


    <!-- https://aphia.org/ns/attribute-trait/hasHabitat -->

    <owl:ObjectProperty rdf:about="https://aphia.org/ns/attribute-trait/hasHabitat">
        <rdfs:subPropertyOf rdf:resource="http://www.ontologydesignpatterns.org/ont/dul/DUL.owl#associatedWith"/>
        <owl:inverseOf rdf:resource="https://aphia.org/ns/attribute-trait/isHabitatOf"/>
        <rdfs:domain rdf:resource="https://aphia.org/ns/taxon-name/Taxon"/>
        <rdfs:range rdf:resource="https://aphia.org/ns/attribute-trait/Environment"/>
        <rdfs:comment xml:lang="nl">Eigenschap die wordt gebruikt om de habitat van de soort weer te geven.</rdfs:comment>
        <rdfs:comment xml:lang="en">Property used to represent the habitat of the species.</rdfs:comment>
        <rdfs:comment xml:lang="it">Proprietà utilizzata per rappresentare l&apos;habitat della specie.</rdfs:comment>
        <rdfs:isDefinedBy rdf:resource="https://aphia.org/ns/attribute-trait"/>
        <rdfs:label xml:lang="it">ha habitat</rdfs:label>
        <rdfs:label xml:lang="en">has habitat</rdfs:label>
        <rdfs:label xml:lang="nl">heeft habitat</rdfs:label>
    </owl:ObjectProperty>
    


    <!-- https://aphia.org/ns/attribute-trait/hasTaxonCharateristic -->

    <owl:ObjectProperty rdf:about="https://aphia.org/ns/attribute-trait/hasTaxonCharateristic">
        <rdfs:subPropertyOf rdf:resource="http://www.ontologydesignpatterns.org/ont/dul/DUL.owl#defines"/>
        <rdfs:domain rdf:resource="https://aphia.org/ns/attribute-trait/TaxonDescription"/>
        <rdfs:range rdf:resource="https://aphia.org/ns/attribute-trait/TaxonCharacteristic"/>
        <rdfs:comment xml:lang="nl">Eigenschap die wordt gebruikt om het kenmerk te specificeren dat attributen en eigenschappen zijn.</rdfs:comment>
        <rdfs:comment xml:lang="en">Property used to specify the characteristic that is attributes and traits.</rdfs:comment>
        <rdfs:comment xml:lang="it">Proprietà utilizzata per specificare le caratteristiche che sono attributi e tratti.</rdfs:comment>
        <rdfs:isDefinedBy rdf:resource="https://aphia.org/ns/attribute-trait"/>
        <rdfs:label xml:lang="it">ha caratteristica del taxon</rdfs:label>
        <rdfs:label xml:lang="en">has taxon characteristic</rdfs:label>
        <rdfs:label xml:lang="nl">heeft taxonkenmerk</rdfs:label>
    </owl:ObjectProperty>
    


    <!-- https://aphia.org/ns/attribute-trait/isAdditionalDescriptionOf -->

    <owl:ObjectProperty rdf:about="https://aphia.org/ns/attribute-trait/isAdditionalDescriptionOf">
        <rdfs:subPropertyOf rdf:resource="http://www.ontologydesignpatterns.org/ont/dul/DUL.owl#describes"/>
        <rdfs:domain rdf:resource="https://aphia.org/ns/attribute-trait/TaxonDescription"/>
        <rdfs:range rdf:resource="https://aphia.org/ns/taxon-name/Taxon"/>
        <rdfs:comment xml:lang="nl">Inverse eigenschap van &apos;heeft aanvullende beschrijving&apos; gebruikt om informatie over het taxon te verkrijgen uit zijn beschrijving in termen van attributen en eigenschappen.</rdfs:comment>
        <rdfs:comment xml:lang="en">Inverse property of &apos;has additional description&apos; used to get information about the taxon from its description in terms of attributes and traits.</rdfs:comment>
        <rdfs:comment xml:lang="it">Proprietà inversa di &apos;ha descrizione aggiuntiva&apos;, utilizzata per ottenere informazioni sul taxon dalla sua descrizione in termini di attributi e tratti.</rdfs:comment>
        <rdfs:isDefinedBy rdf:resource="https://aphia.org/ns/attribute-trait"/>
        <rdfs:label xml:lang="en">is additional description of</rdfs:label>
        <rdfs:label xml:lang="nl">is een aanvullende beschrijving van</rdfs:label>
        <rdfs:label xml:lang="it">è ulteriore descrizione di</rdfs:label>
    </owl:ObjectProperty>
    


    <!-- https://aphia.org/ns/attribute-trait/isHabitatOf -->

    <owl:ObjectProperty rdf:about="https://aphia.org/ns/attribute-trait/isHabitatOf">
        <rdfs:subPropertyOf rdf:resource="http://www.ontologydesignpatterns.org/ont/dul/DUL.owl#associatedWith"/>
        <rdfs:domain rdf:resource="https://aphia.org/ns/attribute-trait/Environment"/>
        <rdfs:range rdf:resource="https://aphia.org/ns/taxon-name/Taxon"/>
        <rdfs:comment xml:lang="nl">Inverse eigenschap van &apos;heeft habitat&apos; om informatie over het taxon uit de omgeving te halen.</rdfs:comment>
        <rdfs:comment xml:lang="en">Inverse property of &apos;has habitat&apos; to get information about the taxon from the environment.</rdfs:comment>
        <rdfs:comment xml:lang="it">Proprietà inversa di &quot;ha un habitat&quot; per ottenere informazioni sul taxon dall&apos;ambiente.</rdfs:comment>
        <rdfs:isDefinedBy rdf:resource="https://aphia.org/ns/attribute-trait"/>
        <rdfs:label xml:lang="nl">is de habitat van</rdfs:label>
        <rdfs:label xml:lang="en">is habitat of</rdfs:label>
        <rdfs:label xml:lang="it">è habitat di</rdfs:label>
    </owl:ObjectProperty>
    


    <!-- https://aphia.org/ns/attribute-trait/isSubSpecificationContextOf -->

    <owl:ObjectProperty rdf:about="https://aphia.org/ns/attribute-trait/isSubSpecificationContextOf">
        <rdfs:subPropertyOf rdf:resource="http://www.ontologydesignpatterns.org/ont/dul/DUL.owl#associatedWith"/>
        <rdfs:domain rdf:resource="https://aphia.org/ns/attribute-trait/SpecificationContext"/>
        <rdfs:range rdf:resource="https://aphia.org/ns/attribute-trait/SpecificationContext"/>
        <rdfs:comment xml:lang="nl">Eigenschap waarmee gebruikers hiërarchieën van specificatiecontexten kunnen maken voor de taxonbeschrijving. Het is vergelijkbaar met de skos:narrower eigenschap in de SKOS ontologie</rdfs:comment>
        <rdfs:comment xml:lang="it">Proprietà che consente agli utenti di creare gerarchie di contesti di specificazione per la descrizione del taxon. È simile alla proprietà skos:narrower dell&apos;ontologia SKOS.</rdfs:comment>
        <rdfs:isDefinedBy rdf:resource="https://aphia.org/ns/attribute-trait"/>
        <rdfs:label xml:lang="en">Property that allows users to create hierarchies of specification contexts for the taxon description. It is similar to the skos:narrower property in the SKOS ontology.</rdfs:label>
        <rdfs:label xml:lang="nl">is de subspecificatiecontext van</rdfs:label>
        <rdfs:label xml:lang="en">is sub specification context of</rdfs:label>
        <rdfs:label xml:lang="it">è sotto contesto di</rdfs:label>
    </owl:ObjectProperty>
    


    <!-- https://aphia.org/ns/top-level/hasType -->

    <owl:ObjectProperty rdf:about="https://aphia.org/ns/top-level/hasType"/>
    


    <!-- https://aphia.org/ns/top-level/hasValue -->

    <owl:ObjectProperty rdf:about="https://aphia.org/ns/top-level/hasValue"/>
    


    <!-- https://aphia.org/ns/top-level/isSubTaxonCharacteristicOf -->

    <owl:ObjectProperty rdf:about="https://aphia.org/ns/top-level/isSubTaxonCharacteristicOf">
        <rdfs:subPropertyOf rdf:resource="http://www.ontologydesignpatterns.org/ont/dul/DUL.owl#associatedWith"/>
        <rdfs:domain rdf:resource="https://aphia.org/ns/attribute-trait/TaxonCharacteristic"/>
        <rdfs:range rdf:resource="https://aphia.org/ns/attribute-trait/TaxonCharacteristic"/>
        <rdfs:comment xml:lang="nl">Eigenschap waarmee gebruikers hiërarchieën van taxonkenmerken kunnen maken en vervolgens hiërarchieën van attributen en eigenschappen. Het is vergelijkbaar met de skos:narrower eigenschap in de SKOS ontologie.</rdfs:comment>
        <rdfs:comment xml:lang="en">Property that allows users to create hierarchies of taxon characteristics and then hierarchies of attributes and traits. It is similar to the skos:narrower property in the SKOS ontology.</rdfs:comment>
        <rdfs:comment xml:lang="it">Proprietà che consente agli utenti di creare gerarchie di caratteristiche dei taxon e poi gerarchie di attributi e tratti. È simile alla proprietà skos:narrower dell&apos;ontologia SKOS.</rdfs:comment>
        <rdfs:isDefinedBy rdf:resource="https://aphia.org/ns/attribute-trait"/>
        <rdfs:label xml:lang="en">is sub taxon characteristic of</rdfs:label>
        <rdfs:label xml:lang="nl">is subtaxonkenmerkend voor</rdfs:label>
        <rdfs:label xml:lang="it">è sotto caratteristica di</rdfs:label>
    </owl:ObjectProperty>
    


    <!-- 
    ///////////////////////////////////////////////////////////////////////////////////////
    //
    // Data properties
    //
    ///////////////////////////////////////////////////////////////////////////////////////
     -->

    


    <!-- http://www.w3.org/2004/02/skos/core#note -->

    <owl:DatatypeProperty rdf:about="http://www.w3.org/2004/02/skos/core#note"/>
    


    <!-- 
    ///////////////////////////////////////////////////////////////////////////////////////
    //
    // Classes
    //
    ///////////////////////////////////////////////////////////////////////////////////////
     -->

    


    <!-- http://www.ontologydesignpatterns.org/ont/d0.owl#Characteristic -->

    <owl:Class rdf:about="http://www.ontologydesignpatterns.org/ont/d0.owl#Characteristic"/>
    


    <!-- http://www.ontologydesignpatterns.org/ont/dul/DUL.owl#Concept -->

    <owl:Class rdf:about="http://www.ontologydesignpatterns.org/ont/dul/DUL.owl#Concept"/>
    


    <!-- http://www.ontologydesignpatterns.org/ont/dul/DUL.owl#Description -->

    <owl:Class rdf:about="http://www.ontologydesignpatterns.org/ont/dul/DUL.owl#Description"/>
    


    <!-- http://www.ontologydesignpatterns.org/ont/dul/DUL.owl#Parameter -->

    <owl:Class rdf:about="http://www.ontologydesignpatterns.org/ont/dul/DUL.owl#Parameter"/>
    


    <!-- http://www.w3.org/2004/02/skos/core#Concept -->

    <owl:Class rdf:about="http://www.w3.org/2004/02/skos/core#Concept"/>
    


    <!-- http://xmlns.com/foaf/0.1/Organization -->

    <owl:Class rdf:about="http://xmlns.com/foaf/0.1/Organization"/>
    


    <!-- https://aphia.org/ns/attribute-trait/Attribute -->

    <owl:Class rdf:about="https://aphia.org/ns/attribute-trait/Attribute">
        <rdfs:subClassOf rdf:resource="http://www.w3.org/2004/02/skos/core#Concept"/>
        <rdfs:subClassOf rdf:resource="https://aphia.org/ns/attribute-trait/TaxonCharacteristic"/>
        <owl:disjointWith rdf:resource="https://aphia.org/ns/attribute-trait/Trait"/>
        <rdfs:comment xml:lang="nl">Deze klasse vertegenwoordigt attributen geassocieerd met een taxon; dat wil zeggen, kwaliteiten of kenmerken waarmee een taxon kan worden onderscheiden. De attributen zijn typisch geassocieerd met categoriale waarden. Voorbeelden zijn: IUCN Rode Lijst Categorie, Ondersteunende structuur &amp; behuizing, AMBI ecologische groep, Seizoensgebondenheid, enz.</rdfs:comment>
        <rdfs:comment xml:lang="it">Questa classe rappresenta gli attributi associati a un taxon, ossia le qualità o le caratteristiche che permettono di distinguere un taxon. Gli attributi sono tipicamente associati a valori categoriali. Esempi sono: Categoria della Lista Rossa IUCN, Struttura di supporto e involucro, Gruppo ecologico AMBI, Stagionalità, ecc.</rdfs:comment>
        <rdfs:comment xml:lang="en">This class represents attributes associated with a taxon; that is, qualities or characteristics whereby a taxon can be distinguished. The attributes are typically associated with categorial values. Examples are: IUCN Red List Category, Supporting structure &amp; enclosure, AMBI ecological group, Seasonality, etc.</rdfs:comment>
        <rdfs:isDefinedBy rdf:resource="https://aphia.org/ns/attribute-trait"/>
        <rdfs:label xml:lang="en">Attribute</rdfs:label>
        <rdfs:label xml:lang="it">Attributo</rdfs:label>
        <rdfs:label xml:lang="nl">Attribuut</rdfs:label>
        <prov:wasInfluencedBy rdf:resource="https://kos.lifewatch.eu/thesauri/fishtraits/c_4"/>
    </owl:Class>
    


    <!-- https://aphia.org/ns/attribute-trait/Environment -->

    <owl:Class rdf:about="https://aphia.org/ns/attribute-trait/Environment">
        <rdfs:subClassOf rdf:resource="http://www.ontologydesignpatterns.org/ont/dul/DUL.owl#Concept"/>
        <rdfs:subClassOf rdf:resource="http://www.w3.org/2004/02/skos/core#Concept"/>
        <rdfs:subClassOf>
            <owl:Restriction>
                <owl:onProperty rdf:resource="https://aphia.org/ns/attribute-trait/isHabitatOf"/>
                <owl:allValuesFrom rdf:resource="https://aphia.org/ns/taxon-name/Taxon"/>
            </owl:Restriction>
        </rdfs:subClassOf>
        <rdfs:comment xml:lang="nl">De klasse van de milieus waarvan bekend is dat het taxon er voorkomt. De individuen van deze klasse kunnen concepten zijn van een gecontroleerde woordenlijst van de habitats.</rdfs:comment>
        <rdfs:comment xml:lang="it">La classe degli ambienti in cui il taxon è conosciuto. Gli individui di questa classe possono essere concetti di un vocabolario controllato degli habitat.</rdfs:comment>
        <rdfs:comment xml:lang="en">The class of the environmnets the taxon is known to exist in. The individuals of this class can be concepts of a controlled vocabulary of the habitats.</rdfs:comment>
        <rdfs:isDefinedBy rdf:resource="https://aphia.org/ns/attribute-trait"/>
        <rdfs:label xml:lang="it">Ambiente</rdfs:label>
        <rdfs:label xml:lang="en">Environment</rdfs:label>
        <rdfs:label xml:lang="nl">Milieu</rdfs:label>
    </owl:Class>
    


    <!-- https://aphia.org/ns/attribute-trait/SpecificationContext -->

    <owl:Class rdf:about="https://aphia.org/ns/attribute-trait/SpecificationContext">
        <rdfs:subClassOf rdf:resource="http://www.ontologydesignpatterns.org/ont/dul/DUL.owl#Description"/>
        <rdfs:subClassOf>
            <owl:Restriction>
                <owl:onProperty rdf:resource="https://aphia.org/ns/attribute-trait/definesParameter"/>
                <owl:someValuesFrom rdf:resource="http://www.ontologydesignpatterns.org/ont/dul/DUL.owl#Parameter"/>
            </owl:Restriction>
        </rdfs:subClassOf>
        <rdfs:subClassOf>
            <owl:Restriction>
                <owl:onProperty rdf:resource="https://aphia.org/ns/top-level/hasValue"/>
                <owl:someValuesFrom rdf:resource="https://aphia.org/ns/top-level/Value"/>
            </owl:Restriction>
        </rdfs:subClassOf>
        <rdfs:subClassOf>
            <owl:Restriction>
                <owl:onProperty rdf:resource="https://aphia.org/ns/top-level/hasValue"/>
                <owl:allValuesFrom rdf:resource="https://aphia.org/ns/top-level/Value"/>
            </owl:Restriction>
        </rdfs:subClassOf>
        <rdfs:comment xml:lang="nl">De klasse voor het representeren van een verdere specificatie van de taxonbeschrijving. De klasse combineert aanvullende parameters en hun waarden die de kenmerken en eigenschappen van de taxonbeschrijving weergeven. Voorbeelden zijn: geslacht, levensstadium enz. met hun toegestane waarden.</rdfs:comment>
        <rdfs:comment xml:lang="it">La classe che consente di rappresentare un&apos;ulteriore specifica della descrizione del taxon. La classe unisce parametri aggiuntivi, e relativi valori, che connotano gli attributi e tratti della descrizione del taxon. Esempi includono: il sesso, lo stadio di vita, ecc. con i loro valori ammessi.</rdfs:comment>
        <rdfs:comment xml:lang="en">The class for representing a further specification of the taxon description. The class combines additional parameters, and their values, that connote the attributes and traits of the taxon description. Examples include: sex, life stage etc. with their permitted values.</rdfs:comment>
        <rdfs:isDefinedBy rdf:resource="https://aphia.org/ns/attribute-trait"/>
        <rdfs:label xml:lang="it">Specifica di Contesto</rdfs:label>
        <rdfs:label xml:lang="nl">Specificatie Context</rdfs:label>
        <rdfs:label xml:lang="en">Specification Context</rdfs:label>
    </owl:Class>
    


    <!-- https://aphia.org/ns/attribute-trait/TaxonCharacteristic -->

    <owl:Class rdf:about="https://aphia.org/ns/attribute-trait/TaxonCharacteristic">
        <rdfs:subClassOf rdf:resource="http://www.ontologydesignpatterns.org/ont/d0.owl#Characteristic"/>
        <rdfs:subClassOf>
            <owl:Restriction>
                <owl:onProperty rdf:resource="https://aphia.org/ns/top-level/hasType"/>
                <owl:maxQualifiedCardinality rdf:datatype="http://www.w3.org/2001/XMLSchema#nonNegativeInteger">1</owl:maxQualifiedCardinality>
                <owl:onClass rdf:resource="https://aphia.org/ns/top-level/Type"/>
            </owl:Restriction>
        </rdfs:subClassOf>
        <rdfs:comment xml:lang="nl">Dit is de klasse van de eigenschappen of kenmerken die meetbaar of waarneembaar en categoriaal zijn voor een taxon.</rdfs:comment>
        <rdfs:comment xml:lang="en">This is the class of the qualities or characteristics measurable or observable and categorial for a taxon.</rdfs:comment>
        <rdfs:comment xml:lang="it">È la classe delle qualità o caratteristiche misurabili o osservabili e categorizzabili per un taxon.</rdfs:comment>
        <rdfs:isDefinedBy rdf:resource="https://aphia.org/ns/attribute-trait"/>
        <rdfs:label xml:lang="it">Caratteristica del Taxon</rdfs:label>
        <rdfs:label xml:lang="en">Taxon Characteristic</rdfs:label>
        <rdfs:label xml:lang="nl">Taxonkenmerk</rdfs:label>
    </owl:Class>
    


    <!-- https://aphia.org/ns/attribute-trait/TaxonDescription -->

    <owl:Class rdf:about="https://aphia.org/ns/attribute-trait/TaxonDescription">
        <rdfs:subClassOf rdf:resource="http://www.ontologydesignpatterns.org/ont/dul/DUL.owl#Description"/>
        <rdfs:subClassOf>
            <owl:Restriction>
                <owl:onProperty rdf:resource="https://aphia.org/ns/attribute-trait/hasTaxonCharateristic"/>
                <owl:someValuesFrom rdf:resource="http://www.ontologydesignpatterns.org/ont/d0.owl#Characteristic"/>
            </owl:Restriction>
        </rdfs:subClassOf>
        <rdfs:subClassOf>
            <owl:Restriction>
                <owl:onProperty rdf:resource="https://aphia.org/ns/attribute-trait/isAdditionalDescriptionOf"/>
                <owl:someValuesFrom rdf:resource="https://aphia.org/ns/taxon-name/Taxon"/>
            </owl:Restriction>
        </rdfs:subClassOf>
        <rdfs:subClassOf>
            <owl:Restriction>
                <owl:onProperty rdf:resource="https://aphia.org/ns/top-level/hasValue"/>
                <owl:someValuesFrom rdf:resource="https://aphia.org/ns/top-level/Value"/>
            </owl:Restriction>
        </rdfs:subClassOf>
        <rdfs:subClassOf>
            <owl:Restriction>
                <owl:onProperty rdf:resource="http://purl.org/dc/terms/source"/>
                <owl:allValuesFrom rdf:resource="https://aphia.org/ns/top-level/Source"/>
            </owl:Restriction>
        </rdfs:subClassOf>
        <rdfs:subClassOf>
            <owl:Restriction>
                <owl:onProperty rdf:resource="https://aphia.org/ns/attribute-trait/hasExtraSpecification"/>
                <owl:allValuesFrom rdf:resource="https://aphia.org/ns/attribute-trait/SpecificationContext"/>
            </owl:Restriction>
        </rdfs:subClassOf>
        <rdfs:subClassOf>
            <owl:Restriction>
                <owl:onProperty rdf:resource="https://aphia.org/ns/attribute-trait/hasTaxonCharateristic"/>
                <owl:allValuesFrom rdf:resource="http://www.ontologydesignpatterns.org/ont/d0.owl#Characteristic"/>
            </owl:Restriction>
        </rdfs:subClassOf>
        <rdfs:subClassOf>
            <owl:Restriction>
                <owl:onProperty rdf:resource="https://aphia.org/ns/top-level/hasValue"/>
                <owl:allValuesFrom rdf:resource="https://aphia.org/ns/top-level/Value"/>
            </owl:Restriction>
        </rdfs:subClassOf>
        <rdfs:subClassOf>
            <owl:Restriction>
                <owl:onProperty rdf:resource="http://www.w3.org/2004/02/skos/core#note"/>
                <owl:allValuesFrom rdf:resource="http://www.w3.org/1999/02/22-rdf-syntax-ns#PlainLiteral"/>
            </owl:Restriction>
        </rdfs:subClassOf>
        <rdfs:comment xml:lang="nl">Deze klasse geeft een beschrijving van het taxon in termen van aanvullende kenmerken, met betrekking tot de habitat die al gedefinieerd is in de verwante klasse, en kenmerken met hun waarden.</rdfs:comment>
        <rdfs:comment xml:lang="it">Questa classe rappresenta una descrizione del taxon in termini di ulteriori attributi, rispetto all&apos;habitat definito con la relativa classe, e di tratti con i valori assunti.</rdfs:comment>
        <rdfs:comment xml:lang="en">This class represents a description of the taxon in terms of additional attributes, with respect to the habitat already defined in the related class, and traits with their values.</rdfs:comment>
        <rdfs:isDefinedBy rdf:resource="https://aphia.org/ns/attribute-trait"/>
        <rdfs:label xml:lang="it">Descrizione del Taxon</rdfs:label>
        <rdfs:label xml:lang="nl">Taxon Beschrijving</rdfs:label>
        <rdfs:label xml:lang="en">Taxon Description</rdfs:label>
    </owl:Class>
    


    <!-- https://aphia.org/ns/attribute-trait/Trait -->

    <owl:Class rdf:about="https://aphia.org/ns/attribute-trait/Trait">
        <owl:equivalentClass rdf:resource="https://kos.lifewatch.eu/thesauri/fishtraits/c_4"/>
        <rdfs:subClassOf rdf:resource="http://www.w3.org/2004/02/skos/core#Concept"/>
        <rdfs:subClassOf rdf:resource="https://aphia.org/ns/attribute-trait/TaxonCharacteristic"/>
        <rdfs:comment xml:lang="nl">De klasse van eigenschappen voor een taxon; dat is elk meetbaar of waarneembaar kenmerk van een organisme. In de WoRMS-database is er op dit moment maar één eigenschap; dat is de &apos;lichaamsgrootte&apos;. Individuen van deze klasse kunnen concepten zijn die gedefinieerd zijn in gecontroleerde domeinwoordenboeken (bijv. trait tesauri).</rdfs:comment>
        <rdfs:comment xml:lang="it">La classe dei tratti di un taxon, cioè qualsiasi caratteristica misurabile o osservabile di un organismo. Nel database WoRMS, al momento, c&apos;è solo un tratto, cioè la &apos;dimensione corporea&apos;. Gli individui di questa classe possono essere concetti definiti in vocabolari controllati di dominio (tesauri sui tratti).</rdfs:comment>
        <rdfs:comment xml:lang="en">The class of traits for a taxon; that is, any measurable or observable characteristic of an organism. In the WoRMS database, at the time being, there is only one trait; that is, the &apos;body size&apos;. Individuals of this class can be concepts defined in controlled domain vocabularies (e.g., trait tesauri).</rdfs:comment>
        <rdfs:isDefinedBy rdf:resource="https://aphia.org/ns/attribute-trait"/>
        <rdfs:label xml:lang="nl">Eigenschap</rdfs:label>
        <rdfs:label xml:lang="en">Trait</rdfs:label>
        <rdfs:label xml:lang="it">Tratto</rdfs:label>
    </owl:Class>
    


    <!-- https://aphia.org/ns/taxon-name/Taxon -->

    <owl:Class rdf:about="https://aphia.org/ns/taxon-name/Taxon"/>
    


    <!-- https://aphia.org/ns/top-level/Source -->

    <owl:Class rdf:about="https://aphia.org/ns/top-level/Source"/>
    


    <!-- https://aphia.org/ns/top-level/Type -->

    <owl:Class rdf:about="https://aphia.org/ns/top-level/Type"/>
    


    <!-- https://aphia.org/ns/top-level/Value -->

    <owl:Class rdf:about="https://aphia.org/ns/top-level/Value"/>
    


    <!-- https://kos.lifewatch.eu/thesauri/fishtraits/c_4 -->

    <owl:Class rdf:about="https://kos.lifewatch.eu/thesauri/fishtraits/c_4"/>
    


    <!-- 
    ///////////////////////////////////////////////////////////////////////////////////////
    //
    // Individuals
    //
    ///////////////////////////////////////////////////////////////////////////////////////
     -->

    


    <!-- https://aphia.org/resource/organisation/dv -->

    <owl:NamedIndividual rdf:about="https://aphia.org/resource/organisation/dv">
        <rdf:type rdf:resource="http://xmlns.com/foaf/0.1/Organization"/>
        <rdfs:label xml:lang="nl">Digitaal Vlaanderen</rdfs:label>
        <rdfs:label xml:lang="en">Digital Flanders</rdfs:label>
        <foaf:name xml:lang="nl">Digitaal Vlaanderen</foaf:name>
        <foaf:name xml:lang="en">Digital Flanders</foaf:name>
    </owl:NamedIndividual>
    <rdf:Description>
        <owl:maxQualifiedCardinality rdf:datatype="http://www.w3.org/2001/XMLSchema#nonNegativeInteger">1</owl:maxQualifiedCardinality>
    </rdf:Description>
</rdf:RDF>



<!-- Generated by the OWL API (version 4.5.29.2024-05-13T12:11:03Z) https://github.com/owlcs/owlapi -->

