@prefix skos: <http://www.w3.org/2004/02/skos/core#> .
@prefix rdfs: <http://www.w3.org/2000/01/rdf-schema#> .
@prefix dct: <http://purl.org/dc/terms/> .

@prefix aphia-trait: <https://aphia.org/ns/attribute-trait/> .

@prefix trait: <https://aphia.org/ns/vocab/attribute-trait/> .

trait:conceptScheme
    a skos:ConceptScheme ;
    rdfs:label "Listing Aphia attributes and traits"@en .

<https://aphia.org/ns/vocab/attribute-trait/>
    a skos:Collection ;
    rdfs:label "Aphia attributes and traits"@en ;
    
    skos:member trait:life_cycle ;
.

trait:life_cycle
    a skos:Collection ; 
    dct:description "The type of life cycle an organism has. Life cycle according to Lincoln et al., 1998: 1: The sequence of events from the origin as a zygote, to the death of an individual. 2: Those stages through which an organism passes between the production of gametes by one generation and the production of gametes by the next."@en ;

    skos:member trait:diplontic , 
                trait:haplodiplontic , 
                    trait:heteromorphic , 
                    trait:isomorphic , 
                    trait:haplodiplontic_not_applicable , 
                    trait:haplodiplontic_unknown , 
                    trait:haplodiplontic_unreported , 
                trait:haplontic , 
                trait:life_cycle_unknown , 
                trait:life_cycle_unreported ; 
.

trait:diplontic
    a skos:Concept, aphia-trait:Trait ;
    skos:inScheme trait:conceptScheme ;
    skos:prefLabel "Diplontic"@en ;
    skos:definition "Having a life cycle in which the direct products of meiosis act as gametes; only the gametes of diplonts are haploid; cf. haplont (Lincoln et al., 1998)."@en ;
.
trait:haplodiplontic
    a skos:Concept, aphia-trait:Trait ;
    skos:inScheme trait:conceptScheme ;
    skos:prefLabel "Haplodiplontic"@en ;
    skos:definition "Having a life cycle with alternating free-living gametophyte and sporophyte phases (macroalgae; Womersley, 1987)."@en ;

    skos:narrower trait:heteromorphic , trait:haplodiplontic_not_applicable , trait:haplodiplontic_unknown , trait:haplodiplontic_unreported ;
.
trait:heteromorphic
    a skos:Concept, aphia-trait:Trait ;
    skos:inScheme trait:conceptScheme ;
    skos:prefLabel "Heteromorphic"@en ;
    skos:definition "Organisms with the gametophyte and sporophyte of different morphology and size (macroalgae; Womersley, 1987). Having different forms at different times or at different stages of the life cycle; used of a plant having an alternation of vegetatively dissimilar generations; heteromorphous; cf. homomorphic (Lincoln et al., 1998)."@en ;
.
trait:isomorphic
    a skos:Concept, aphia-trait:Trait ;
    skos:inScheme trait:conceptScheme ;
    skos:prefLabel "Isomorphic"@en ;
    skos:definition "Organisms with the gametophyte and sporophyte of similar morphology and size (macroalgae; Womersley, 1987). Used of a plant having an alternation between diploid and haploid generations which are morphologically similar in appearance; homomoprhic; isomorphous; cf. heteromorphic (Lincoln et al., 1998)."@en ;
.
trait:haplodiplontic_not_applicable
    a skos:Concept, aphia-trait:Trait ;
    skos:inScheme trait:conceptScheme ;
    skos:prefLabel "Haplodiplontic not applicable"@en ;
    skos:definition "It is not applicable whether this taxon is heteromorphic or isomorphic."@en ;
.
trait:haplodiplontic_unknown
    a skos:Concept, aphia-trait:Trait ;
    skos:inScheme trait:conceptScheme ;
    skos:prefLabel "Haplodiplontic unknown"@en ;
    skos:definition "According to literature it is unknown whether this organism is heteromorphic or isomorphic."@en ;
.
trait:haplodiplontic_unreported
    a skos:Concept, aphia-trait:Trait ;
    skos:inScheme trait:conceptScheme ;
    skos:prefLabel "Haplodiplontic unreported"@en ;
    skos:definition "So far it has not been reported in literature whether this taxon is heteromorphic or isomorphic."@en ;
.
trait:haplontic
    a skos:Concept, aphia-trait:Trait ;
    skos:inScheme trait:conceptScheme ;
    skos:prefLabel "Haplontic"@en ;
    skos:definition "Having a life cycle in which meiosis occurs in the zygote to produce the haploid phase; only the zygote of the haplonts is diploid; cf. diplont."@en ;
.
trait:life_cycle_unknown
    a skos:Concept, aphia-trait:Trait ;
    skos:inScheme trait:conceptScheme ;
    skos:prefLabel "Unknown life cycle"@en ;
    skos:definition "According to literature it is unknown what life cycle this organism has."@en ;
.
trait:life_cycle_unreported
    a skos:Concept, aphia-trait:Trait ;
    skos:inScheme trait:conceptScheme ;
    skos:prefLabel "Unreported life cycle"@en ;
    skos:definition "So far it has not been reported in literature what life cycle this taxon has."@en ;
.