@prefix skos: <http://www.w3.org/2004/02/skos/core#> .
@prefix rdfs: <http://www.w3.org/2000/01/rdf-schema#> .
@prefix dct: <http://purl.org/dc/terms/> .

@prefix aphia-trait: <https://aphia.org/ns/attribute-trait/> .

@prefix trait: <https://aphia.org/ns/vocab/attribute-trait/> .

trait:conceptScheme
    a skos:ConceptScheme ;
    rdfs:label "Listing Aphia attributes and traits"@en .

<https://aphia.org/ns/vocab/attribute-trait/>
    a skos:Collection ;
    rdfs:label "Aphia attributes and traits"@en ;
    
    skos:member trait:reproduction_modes ;
.

trait:reproduction_modes
    a skos:Collection ; 
    dct:description "This trait describes which mode of reproduction animals use to produce their young."@en ;

    skos:member trait:oviparous , 
                    trait:oviparous_no_parental_care , 
                    trait:oviparous_parental_care , 
                trait:ovoviviparous , 
                trait:viviparous , 
                    trait:viviparous_no_parental_care , 
                    trait:viviparous_parental_care ; 

    skos:closeMatch ... ; 
.

trait:oviparous
    a skos:Concept, aphia-trait:Trait ;
    skos:inScheme trait:conceptScheme ;
    skos:prefLabel "Oviparous"@en ;
    skos:definition "Egg laying; producing eggs that are laid and hatch externally (Lincoln et al., 1998). Egg-laying (Henderson's Dictionary of Biology; Lawrence, 2005)."@en ;

    skos:narrower trait:oviparous_no_parental_care , trait:oviparous_parental_care ;

    skos:exactMatch ... ; 
.

trait:oviparous_no_parental_care
    a skos:Concept, aphia-trait:Trait ;
    skos:inScheme trait:conceptScheme ;
    skos:prefLabel "Oviparous, without parental care"@en ;
    skos:definition "Egg laying; producing eggs that are laid and hatch externally (Lincoln et al., 1998). Egg-laying (Henderson's Dictionary of Biology; Lawrence, 2005). There is no form of parental behaviour (adapted from Lincoln et al., 1998)."@en ;

    skos:broader trait:oviparous ;
.

trait:oviparous_parental_care
    a skos:Concept, aphia-trait:Trait ;
    skos:inScheme trait:conceptScheme ;
    skos:prefLabel "Oviparous, with parental care"@en ;
    skos:definition "Egg laying; producing eggs that are laid and hatch externally (Lincoln et al., 1998). Egg-laying (Henderson's Dictionary of Biology; Lawrence, 2005). Any form of parental behaviour that appears likely to increase the fitness of a parent's offspring."@en ;

    skos:broader trait:oviparous ;
.

trait:ovoviviparous
    a skos:Concept, aphia-trait:Trait ;
    skos:inScheme trait:conceptScheme ;
    skos:prefLabel "Ovoviviparous"@en ;
    skos:definition "Fully formed eggs are retained and hatched inside the maternal body and are released as live offspring. No nutrition is derived from the mother (Lincoln et al., 1998). Pert. organisms that produce an egg with a persistent outer covering, but which hatches within the maternal body (Henderson's Dictionary of Biology; Lawrence, 2005)."@en ;

    skos:exactMatch ... ; 
.

trait:viviparous
    a skos:Concept, aphia-trait:Trait ;
    skos:inScheme trait:conceptScheme ;
    skos:prefLabel ""@en ;
    skos:definition "1: Producing live offspring from within the body of the parent; zoogonous; viviparity, vivipary; cf. larvipary, oviparous, ovoviviparous. 2: Germinating while still attached to the parent plant (Lincoln et al., 1998). Development of an embryo within the body of the parent, in part, resources passing directly from parent to embryo (Barnes et al., 2006). (1) producing young alive rather than laying eggs, appl. all mammals except monotremes, and some animals in other groups; (2) appl. plants, having seeds that germinate while still attached to the parent plant, e.g. mangrove (Henderson's Dictionary of Biology; Lawrence, 2005)."@en ;

    skos:narrower trait:viviparous_no_parental_care , trait:viviparous_parental_care ;

    skos:exactMatch ... ; 
.

trait:viviparous_no_parental_care
    a skos:Concept, aphia-trait:Trait ;
    skos:inScheme trait:conceptScheme ;
    skos:prefLabel "viviparous, without parental care"@en ;
    skos:definition "1: Producing live offspring from within the body of the parent; zoogonous; viviparity, vivipary; cf. larvipary, oviparous, ovoviviparous. 2: Germinating while still attached to the parent plant (Lincoln et al., 1998). Development of an embryo within the body of the parent, in part, resources passing directly from parent to embryo (Barnes et al., 2006). (1) producing young alive rather than laying eggs, appl. all mammals except monotremes, and some animals in other groups; (2) appl. plants, having seeds that germinate while still attached to the parent plant, e.g. mangrove (Henderson's Dictionary of Biology; Lawrence, 2005). There is no form of parental behaviour (adapted from Lincoln et al., 1998)."@en ;

    skos:broader trait:viviparous ;
.

trait:viviparous_parental_care
    a skos:Concept, aphia-trait:Trait ;
    skos:inScheme trait:conceptScheme ;
    skos:prefLabel "viviparous, with parental care"@en ;
    skos:definition "1: Producing live offspring from within the body of the parent; zoogonous; viviparity, vivipary; cf. larvipary, oviparous, ovoviviparous. 2: Germinating while still attached to the parent plant (Lincoln et al., 1998). Development of an embryo within the body of the parent, in part, resources passing directly from parent to embryo (Barnes et al., 2006). (1) producing young alive rather than laying eggs, appl. all mammals except monotremes, and some animals in other groups; (2) appl. plants, having seeds that germinate while still attached to the parent plant, e.g. mangrove (Henderson's Dictionary of Biology; Lawrence, 2005). Any form of parental behaviour that appears likely to increase the fitness of a parent's offspring."@en ;

    skos:broader trait:viviparous ;
.