<?xml version="1.0"?>
<rdf:RDF xmlns="https://aphia.org/ns/taxon-name/"
     xml:base="https://aphia.org/ns/taxon-name/"
     xmlns:dct="http://purl.org/dc/terms/"
     xmlns:owl="http://www.w3.org/2002/07/owl#"
     xmlns:rdf="http://www.w3.org/1999/02/22-rdf-syntax-ns#"
     xmlns:xml="http://www.w3.org/XML/1998/namespace"
     xmlns:xsd="http://www.w3.org/2001/XMLSchema#"
     xmlns:foaf="http://xmlns.com/foaf/0.1/"
     xmlns:prov="http://www.w3.org/ns/prov#"
     xmlns:rdfs="http://www.w3.org/2000/01/rdf-schema#"
     xmlns:skos="http://www.w3.org/2004/02/skos/core#">
    <owl:Ontology rdf:about="https://aphia.org/ns/taxon-name">
        <owl:versionIRI rdf:resource="https://aphia.org/ns/taxon-name/0.2"/>
        <owl:imports rdf:resource="http://www.w3.org/2008/05/skos-xl"/>
        <owl:imports rdf:resource="https://aphia.org/ns/top-level"/>
        <dct:creator rdf:resource="https://aphia.org/resource/organisation/dv"/>
        <dct:creator rdf:resource="https://ror.org/0496vr396"/>
        <dct:creator rdf:resource="https://w3id.org/italia/data/organization/support-unit/cnr-Z6HZEH/stlab"/>
        <dct:description xml:lang="it">Questa è l&apos;ontologia dei nomi dei taxon e di tutte le informazione tassonomiche, come disponibili dal sistema WoRMS. Essa importa l&apos;ontologia di primo livello top-level ed è allineata a skos-xl.</dct:description>
        <dct:description xml:lang="en">This is the ontology of taxon names and all taxonomic information, as available from the WoRMS system. It imports the top-level ontology of the APHIA network of ontologies, and is aligned to skos-xl.</dct:description>
        <dct:description xml:lang="nl">Dit is de ontologie van taxanamen en alle taxonomische informatie zoals beschikbaar in het WoRMS-systeem. Het importeert de APHIA top-level ontologie en is afgestemd op skos-xl.</dct:description>
        <dct:issued rdf:datatype="http://www.w3.org/2001/XMLSchema#date">2023-08-30</dct:issued>
        <dct:language rdf:resource="http://publications.europa.eu/resource/authority/language/ENG"/>
        <dct:language rdf:resource="http://publications.europa.eu/resource/authority/language/ITA"/>
        <dct:language rdf:resource="http://publications.europa.eu/resource/authority/language/NLD"/>
        <dct:license rdf:resource="http://publications.europa.eu/resource/authority/licence/CC_BY_4_0"/>
        <dct:modified rdf:datatype="http://www.w3.org/2001/XMLSchema#date">2024-02-10</dct:modified>
        <dct:title xml:lang="it">APHIA - Ontologia dei nomi dei taxon</dct:title>
        <dct:title xml:lang="en">APHIA - Taxon names ontology</dct:title>
        <dct:title xml:lang="nl">APHIA - Ontologie van taxanamen</dct:title>
        <rdfs:comment xml:lang="it">Questa è l&apos;ontologia dei nomi dei taxon e di tutte le informazione tassonomiche come disponibili dal sistema WoRMS. Essa importa l&apos;ontologia di primo livello top-level ed è allineata a skos-xl.</rdfs:comment>
        <rdfs:comment xml:lang="en">This is the ontology of taxon names and all taxonomic information as available from the WoRMS system. It imports the top-level ontology of the APHIA network of ontologies, and is aligned to skos-xl.</rdfs:comment>
        <rdfs:comment xml:lang="nl">Dit is de ontologie van taxanamen en alle taxonomische informatie zoals beschikbaar in het WoRMS-systeem. Het importeert de APHIA top-level ontologie en is afgestemd op skos-xl.</rdfs:comment>
        <rdfs:label xml:lang="it">APHIA - Ontologia dei nomi dei taxon</rdfs:label>
        <rdfs:label xml:lang="en">APHIA - Taxon names ontology</rdfs:label>
        <rdfs:label xml:lang="nl">APHIA - Ontologie van taxanamen</rdfs:label>
        <owl:versionInfo xml:lang="en">Second version 0.2 - changed URIs from w3id.org/ to aphia.org/; changed the name of the ontology from taxon-name to taxon-name; introduced some alignments to Darwin Core for some properties; changed some definitions (e.g., authorship).</owl:versionInfo>
        <owl:versionInfo xml:lang="it">Seconda versione 0.2 - cambiati tutti gli URI da w3id.org/ a aphia.org/; cambiato il nome dell&apos;ontologia da taxon-name a taxon-name; introdotti alcuni allineamenti a Darwin core per alcune proprietà; cambiate alcune definizioni (e.g., authorship).</owl:versionInfo>
        <owl:versionInfo xml:lang="nl">Tweede versie 0.2 - URI's gewijzigd van w3id.org/ naar aphia.org/; de naam van de ontologie gewijzigd van taxanaam in taxonnaam; enkele alignaties op Darwin Core geïntroduceerd voor sommige eigenschappen; enkele definities (bijv. auteurschap) gewijzigd.</owl:versionInfo>
    </owl:Ontology>
    


    <!-- 
    ///////////////////////////////////////////////////////////////////////////////////////
    //
    // Annotation properties
    //
    ///////////////////////////////////////////////////////////////////////////////////////
     -->

    


    <!-- http://purl.org/dc/terms/issued -->

    <owl:AnnotationProperty rdf:about="http://purl.org/dc/terms/issued"/>
    


    <!-- http://purl.org/dc/terms/language -->

    <owl:AnnotationProperty rdf:about="http://purl.org/dc/terms/language"/>
    


    <!-- http://purl.org/dc/terms/license -->

    <owl:AnnotationProperty rdf:about="http://purl.org/dc/terms/license"/>
    


    <!-- http://purl.org/dc/terms/modified -->

    <owl:AnnotationProperty rdf:about="http://purl.org/dc/terms/modified"/>
    


    <!-- http://www.w3.org/2002/07/owl#minQualifiedCardinality -->

    <owl:AnnotationProperty rdf:about="http://www.w3.org/2002/07/owl#minQualifiedCardinality"/>
    


    <!-- http://www.w3.org/ns/prov#wasDerivedFrom -->

    <owl:AnnotationProperty rdf:about="http://www.w3.org/ns/prov#wasDerivedFrom"/>
    


    <!-- http://xmlns.com/foaf/0.1/name -->

    <owl:AnnotationProperty rdf:about="http://xmlns.com/foaf/0.1/name"/>
    


    <!-- 
    ///////////////////////////////////////////////////////////////////////////////////////
    //
    // Datatypes
    //
    ///////////////////////////////////////////////////////////////////////////////////////
     -->

    


    <!-- http://www.w3.org/2001/XMLSchema#date -->

    <rdfs:Datatype rdf:about="http://www.w3.org/2001/XMLSchema#date"/>
    


    <!-- 
    ///////////////////////////////////////////////////////////////////////////////////////
    //
    // Object Properties
    //
    ///////////////////////////////////////////////////////////////////////////////////////
     -->

    


    <!-- http://purl.org/dc/terms/coverage -->

    <owl:ObjectProperty rdf:about="http://purl.org/dc/terms/coverage"/>
    


    <!-- http://purl.org/dc/terms/relation -->

    <owl:ObjectProperty rdf:about="http://purl.org/dc/terms/relation"/>
    


    <!-- http://purl.org/dc/terms/source -->

    <owl:ObjectProperty rdf:about="http://purl.org/dc/terms/source"/>
    


    <!-- http://www.ontologydesignpatterns.org/ont/dul/DUL.owl#associatedWith -->

    <owl:ObjectProperty rdf:about="http://www.ontologydesignpatterns.org/ont/dul/DUL.owl#associatedWith"/>
    


    <!-- https://aphia.org/ns/taxon-name/denotes -->

    <owl:ObjectProperty rdf:about="https://aphia.org/ns/taxon-name/denotes">
        <rdfs:subPropertyOf rdf:resource="http://www.ontologydesignpatterns.org/ont/dul/DUL.owl#associatedWith"/>
        <owl:inverseOf rdf:resource="https://aphia.org/ns/taxon-name/isDenotedBy"/>
        <rdfs:domain rdf:resource="https://aphia.org/ns/top-level/Name"/>
        <rdfs:range rdf:resource="https://aphia.org/ns/taxon-name/Taxon"/>
        <rdfs:comment xml:lang="en">Property used to represent a name for a taxon.</rdfs:comment>
        <rdfs:comment xml:lang="it">Proprietà utilizzata per definire un nome per un taxon.</rdfs:comment>
        <rdfs:comment xml:lang="nl">Eigenschap die wordt gebruikt om een naam voor een taxon te definiëren.</rdfs:comment>
        <rdfs:isDefinedBy rdf:resource="https://aphia.org/ns/taxon-name"/>
        <rdfs:label xml:lang="it">definisce/denota</rdfs:label>
        <rdfs:label xml:lang="en">denotes</rdfs:label>
        <rdfs:label xml:lang="nl">definieert</rdfs:label>
    </owl:ObjectProperty>
    


    <!-- https://aphia.org/ns/taxon-name/hasAcceptedName -->

    <owl:ObjectProperty rdf:about="https://aphia.org/ns/taxon-name/hasAcceptedName">
        <rdfs:subPropertyOf rdf:resource="https://aphia.org/ns/taxon-name/isDenotedBy"/>
        <rdf:type rdf:resource="http://www.w3.org/2002/07/owl#FunctionalProperty"/>
        <rdfs:domain rdf:resource="https://aphia.org/ns/taxon-name/Taxon"/>
        <rdfs:range rdf:resource="https://aphia.org/ns/taxon-name/TaxonName"/>
        <rdfs:comment xml:lang="en">Property used to represent the currently valid (zoological) or accepted (botanical) scientific name for a taxon.</rdfs:comment>
        <rdfs:comment xml:lang="it">Proprietà utilizzata per rappresentare il nome scientifico attualmente valido (zoologico) o accettato (botanico) di un taxon.</rdfs:comment>
        <rdfs:comment xml:lang="nl">Eigenschap gebruikt om de huidige geldige (zoölogische) of aanvaarde (botanische) wetenschappelijke naam voor een taxon weer te geven.</rdfs:comment>
        <rdfs:isDefinedBy rdf:resource="https://aphia.org/ns/taxon-name"/>
        <rdfs:label xml:lang="it">ha nome valido/accettato</rdfs:label>
        <rdfs:label xml:lang="en">has accepted name</rdfs:label>
        <rdfs:label xml:lang="nl">heeft geaccepteerde naam</rdfs:label>
    </owl:ObjectProperty>
    


    <!-- https://aphia.org/ns/taxon-name/hasChild -->

    <owl:ObjectProperty rdf:about="https://aphia.org/ns/taxon-name/hasChild">
        <rdfs:subPropertyOf rdf:resource="http://www.w3.org/2004/02/skos/core#narrower"/>
        <owl:inverseOf rdf:resource="https://aphia.org/ns/taxon-name/hasParent"/>
        <rdfs:domain rdf:resource="https://aphia.org/ns/taxon-name/Taxon"/>
        <rdfs:range rdf:resource="https://aphia.org/ns/taxon-name/Taxon"/>
        <rdfs:comment xml:lang="en">Property that allows representing the direct child taxon in a classification.</rdfs:comment>
        <rdfs:comment xml:lang="it">Proprietà che consente di rappresentare il taxon diretto inferiore in una classification.</rdfs:comment>
        <rdfs:comment xml:lang="nl">Eigenschap die toelaat het directe lagere taxon in een classificatie weer te geven.</rdfs:comment>
        <rdfs:isDefinedBy rdf:resource="https://aphia.org/ns/taxon-name"/>
        <rdfs:label xml:lang="it">ha taxon inferiore</rdfs:label>
        <rdfs:label xml:lang="en">has child taxon</rdfs:label>
        <rdfs:label xml:lang="nl">heeft lager taxon</rdfs:label>
    </owl:ObjectProperty>
    


    <!-- https://aphia.org/ns/taxon-name/hasParent -->

    <owl:ObjectProperty rdf:about="https://aphia.org/ns/taxon-name/hasParent">
        <rdfs:subPropertyOf rdf:resource="http://www.w3.org/2004/02/skos/core#broader"/>
        <rdf:type rdf:resource="http://www.w3.org/2002/07/owl#FunctionalProperty"/>
        <rdfs:domain rdf:resource="https://aphia.org/ns/taxon-name/Taxon"/>
        <rdfs:range rdf:resource="https://aphia.org/ns/taxon-name/Taxon"/>
        <rdfs:comment xml:lang="en">Property that allows representing the direct parent taxon in a classification. The parent of a species is usually a genus; the parent of a genus is usually a family, and so on.</rdfs:comment>
        <rdfs:comment xml:lang="it">Proprietà che consente di rappresentare il taxon diretto superiore in una classificatione. Il taxon diretto superiore di una specie è di solito il genere, quello del genere è la famiglia e così via.</rdfs:comment>
        <rdfs:comment xml:lang="nl">Eigenschap die toelaat het directe hogere taxon in een classificatie weer te geven. De ouder van een soort is meestal een geslacht; de ouder van een geslacht is meestal een familie, enzovoort.</rdfs:comment>
        <rdfs:isDefinedBy rdf:resource="https://aphia.org/ns/taxon-name"/>
        <rdfs:label xml:lang="it">ha taxon superiore</rdfs:label>
        <rdfs:label xml:lang="en">has parent taxon</rdfs:label>
        <rdfs:label xml:lang="nl">heeft hoger taxon</rdfs:label>
    </owl:ObjectProperty>
    


    <!-- https://aphia.org/ns/taxon-name/hasStatus -->

    <owl:ObjectProperty rdf:about="https://aphia.org/ns/taxon-name/hasStatus">
        <rdfs:subPropertyOf rdf:resource="http://www.ontologydesignpatterns.org/ont/dul/DUL.owl#associatedWith"/>
        <rdf:type rdf:resource="http://www.w3.org/2002/07/owl#FunctionalProperty"/>
        <rdfs:domain rdf:resource="https://aphia.org/ns/taxon-name/TaxonName"/>
        <rdfs:range rdf:resource="https://aphia.org/ns/taxon-name/Status"/>
        <rdfs:comment xml:lang="en">Property used to connect the taxon name with its status (e.g., accepted, unaccepted).</rdfs:comment>
        <rdfs:comment xml:lang="it">Proprietà utilizzata per collegare il nome del taxon con il suo stato (e.g., accettato, non accettato).</rdfs:comment>
        <rdfs:comment xml:lang="nl">Eigenschap gebruikt om de taxonnaam te koppelen aan zijn status (bijv. geaccepteerd, niet geaccepteerd).</rdfs:comment>
        <rdfs:isDefinedBy rdf:resource="https://aphia.org/ns/taxon-name"/>
        <rdfs:label xml:lang="it">ha stato</rdfs:label>
        <rdfs:label xml:lang="en">has status</rdfs:label>
        <rdfs:label xml:lang="nl">heeft status</rdfs:label>
    </owl:ObjectProperty>
    


    <!-- https://aphia.org/ns/taxon-name/hasSynonym -->

    <owl:ObjectProperty rdf:about="https://aphia.org/ns/taxon-name/hasSynonym">
        <rdfs:subPropertyOf rdf:resource="http://purl.org/dc/terms/relation"/>
        <owl:inverseOf rdf:resource="https://aphia.org/ns/taxon-name/isSynonymOf"/>
        <rdfs:domain rdf:resource="https://aphia.org/ns/taxon-name/TaxonName"/>
        <rdfs:range rdf:resource="https://aphia.org/ns/taxon-name/TaxonName"/>
        <rdfs:comment xml:lang="en">Property used to specify synonymity relations between taxon names.</rdfs:comment>
        <rdfs:comment xml:lang="it">Proprietà utilizzata per specificare relazioni di sinonimia tra nomi di taxon.</rdfs:comment>
        <rdfs:comment xml:lang="nl">Eigenschap gebruikt om synoniemenrelaties tussen taxonnamen te specificeren.</rdfs:comment>
        <rdfs:isDefinedBy rdf:resource="https://aphia.org/ns/taxon-name"/>
        <rdfs:label xml:lang="it">ha sinonimo</rdfs:label>
        <rdfs:label xml:lang="en">has synonym</rdfs:label>
        <rdfs:label xml:lang="nl">heeft synoniem</rdfs:label>
    </owl:ObjectProperty>
    


    <!-- https://aphia.org/ns/taxon-name/hasSynonymName -->

    <owl:ObjectProperty rdf:about="https://aphia.org/ns/taxon-name/hasSynonymName">
        <rdfs:subPropertyOf rdf:resource="https://aphia.org/ns/taxon-name/isDenotedBy"/>
        <rdfs:domain rdf:resource="https://aphia.org/ns/taxon-name/Taxon"/>
        <rdfs:range rdf:resource="https://aphia.org/ns/taxon-name/TaxonName"/>
        <rdfs:comment xml:lang="en">Proprietà used to connect the taxon with its names considered synonyms.</rdfs:comment>
        <rdfs:comment xml:lang="it">Proprietà utilizzata per collegare il taxon con i suoi nomi considerati sinonimi.</rdfs:comment>
        <rdfs:comment xml:lang="nl">Eigenschap gebruikt om het taxon te koppelen aan zijn namen die als synoniemen worden beschouwd.</rdfs:comment>
        <rdfs:isDefinedBy rdf:resource="https://aphia.org/ns/taxon-name"/>
        <rdfs:label xml:lang="it">ha nome sinonimo</rdfs:label>
        <rdfs:label xml:lang="en">has synonym name</rdfs:label>
        <rdfs:label xml:lang="nl">heeft synoniem naam</rdfs:label>
    </owl:ObjectProperty>
    


    <!-- https://aphia.org/ns/taxon-name/hasUnacceptedReason -->

    <owl:ObjectProperty rdf:about="https://aphia.org/ns/taxon-name/hasUnacceptedReason">
        <rdfs:subPropertyOf rdf:resource="http://www.ontologydesignpatterns.org/ont/dul/DUL.owl#associatedWith"/>
        <rdfs:domain rdf:resource="https://aphia.org/ns/taxon-name/TaxonName"/>
        <rdfs:range rdf:resource="https://aphia.org/ns/taxon-name/UnacceptedReason"/>
        <rdfs:comment xml:lang="en">Property used to specify the motivation for which a name is not accepted for a taxon name.</rdfs:comment>
        <rdfs:comment xml:lang="it">Proprietà utilizzata per specificare il motivo per cui un nome non è accettato per un nome di taxon.</rdfs:comment>
        <rdfs:comment xml:lang="nl">Eigenschap gebruikt om de motivatie te specificeren waarvoor een naam niet wordt geaccepteerd voor een taxonnaam.</rdfs:comment>
        <rdfs:isDefinedBy rdf:resource="https://aphia.org/ns/taxon-name"/>
        <rdfs:label xml:lang="it">ha motivo non accettato</rdfs:label>
        <rdfs:label xml:lang="en">has unaccepted reason</rdfs:label>
        <rdfs:label xml:lang="nl">heeft niet-geaccepteerd reden</rdfs:label>
    </owl:ObjectProperty>
    


    <!-- https://aphia.org/ns/taxon-name/isDenotedBy -->

    <owl:ObjectProperty rdf:about="https://aphia.org/ns/taxon-name/isDenotedBy">
        <rdfs:subPropertyOf rdf:resource="http://www.ontologydesignpatterns.org/ont/dul/DUL.owl#associatedWith"/>
        <rdfs:domain rdf:resource="https://aphia.org/ns/taxon-name/Taxon"/>
        <rdfs:range rdf:resource="https://aphia.org/ns/top-level/Name"/>
        <rdfs:comment xml:lang="en">Inverse property of &apos;denotes&apos; that allows one to specify the name for a taxon.</rdfs:comment>
        <rdfs:comment xml:lang="it">Proprietà inversa di &apos;definito/denotato&apos; che consente di specificare il nome per un taxon.</rdfs:comment>
        <rdfs:comment xml:lang="nl">Inverse eigenschap van 'definieert' die toelaat de naam van een taxon te definiëren.</rdfs:comment>
        <rdfs:isDefinedBy rdf:resource="https://aphia.org/ns/taxon-name"/>
        <rdfs:label xml:lang="en">is denoted by</rdfs:label>
        <rdfs:label xml:lang="it">è definito/denotato da</rdfs:label>
        <rdfs:label xml:lang="nl">is gedefinieerd door</rdfs:label>
    </owl:ObjectProperty>
    


    <!-- https://aphia.org/ns/taxon-name/isOfRank -->

    <owl:ObjectProperty rdf:about="https://aphia.org/ns/taxon-name/isOfRank">
        <rdfs:subPropertyOf rdf:resource="http://www.ontologydesignpatterns.org/ont/dul/DUL.owl#associatedWith"/>
        <rdf:type rdf:resource="http://www.w3.org/2002/07/owl#FunctionalProperty"/>
        <rdfs:domain rdf:resource="https://aphia.org/ns/taxon-name/TaxonName"/>
        <rdfs:range rdf:resource="https://aphia.org/ns/taxon-name/Rank"/>
        <rdfs:comment xml:lang="en">Property used to specify the rank in a taxonomic classification for the taxon name.</rdfs:comment>
        <rdfs:comment xml:lang="it">Proprietà utilizzata per specificare il rango in una classificazione tassonomica per un nome di taxon.</rdfs:comment>
        <rdfs:comment xml:lang="nl">Eigenschap gebruikt om de taxonnaam te koppelen aan zijn rang in een taxonomische classificatie.</rdfs:comment>
        <rdfs:isDefinedBy rdf:resource="https://aphia.org/ns/taxon-name"/>
        <rdfs:label xml:lang="en">is of rank</rdfs:label>
        <rdfs:label xml:lang="it">è di rango</rdfs:label>
        <rdfs:label xml:lang="nl">heeft rang</rdfs:label>
    </owl:ObjectProperty>
    


    <!-- https://aphia.org/ns/taxon-name/isSynonymOf -->

    <owl:ObjectProperty rdf:about="https://aphia.org/ns/taxon-name/isSynonymOf">
        <rdfs:subPropertyOf rdf:resource="http://purl.org/dc/terms/relation"/>
        <rdfs:domain rdf:resource="https://aphia.org/ns/taxon-name/TaxonName"/>
        <rdfs:range rdf:resource="https://aphia.org/ns/taxon-name/TaxonName"/>
        <rdfs:comment xml:lang="en">Inverse property of &apos;has synonym&apos;.</rdfs:comment>
        <rdfs:comment xml:lang="it">Proprietà inversa di &apos;ha sinonimo&apos;.</rdfs:comment>
        <rdfs:comment xml:lang="nl">Inverse eigenschap van 'heeft synoniem'</rdfs:comment>
        <rdfs:isDefinedBy rdf:resource="https://aphia.org/ns/taxon-name"/>
        <rdfs:label xml:lang="en">is synonym of</rdfs:label>
        <rdfs:label xml:lang="it">è sinonimo di</rdfs:label>
        <rdfs:label xml:lang="nl">is synoniem van</rdfs:label>
    </owl:ObjectProperty>
    


    <!-- https://aphia.org/ns/top-level/hasIdentifier -->

    <owl:ObjectProperty rdf:about="https://aphia.org/ns/top-level/hasIdentifier"/>
    


    <!-- 
    ///////////////////////////////////////////////////////////////////////////////////////
    //
    // Data properties
    //
    ///////////////////////////////////////////////////////////////////////////////////////
     -->

    


    <!-- http://purl.org/dc/terms/identifier -->

    <owl:DatatypeProperty rdf:about="http://purl.org/dc/terms/identifier"/>
    


    <!-- http://rs.tdwg.org/dwc/terms/scientificName -->

    <owl:DatatypeProperty rdf:about="http://rs.tdwg.org/dwc/terms/scientificName"/>
    


    <!-- http://rs.tdwg.org/dwc/terms/scientificNameAuthorship -->

    <owl:DatatypeProperty rdf:about="http://rs.tdwg.org/dwc/terms/scientificNameAuthorship"/>
    


    <!-- http://rs.tdwg.org/dwc/terms/scientificNameID -->

    <owl:DatatypeProperty rdf:about="http://rs.tdwg.org/dwc/terms/scientificNameID"/>
    


    <!-- http://rs.tdwg.org/dwc/terms/vernacularName -->

    <owl:DatatypeProperty rdf:about="http://rs.tdwg.org/dwc/terms/vernacularName"/>
    


    <!-- https://aphia.org/ns/taxon-name/aphiaID -->

    <owl:DatatypeProperty rdf:about="https://aphia.org/ns/taxon-name/aphiaID">
        <rdfs:subPropertyOf rdf:resource="http://purl.org/dc/terms/identifier"/>
        <rdfs:subPropertyOf rdf:resource="http://rs.tdwg.org/dwc/terms/scientificNameID"/>
        <rdf:type rdf:resource="http://www.w3.org/2002/07/owl#FunctionalProperty"/>
        <rdfs:domain rdf:resource="https://aphia.org/ns/taxon-name/TaxonName"/>
        <rdfs:range rdf:resource="http://www.w3.org/2000/01/rdf-schema#Literal"/>
        <rdfs:comment xml:lang="it">Codice univoco e persistente nel sistema WoRMS.</rdfs:comment>
        <rdfs:comment xml:lang="en">Unique and persistent code within WoRMS.</rdfs:comment>
        <rdfs:comment xml:lang="nl">Unieke en persistente code in WoRMS.</rdfs:comment>
        <rdfs:isDefinedBy rdf:resource="https://aphia.org/ns/taxon-name"/>
        <rdfs:label xml:lang="en">aphia identifier</rdfs:label>
        <rdfs:label xml:lang="it">identificativo aphia</rdfs:label>
        <rdfs:label xml:lang="nl">aphia identificatie</rdfs:label>
    </owl:DatatypeProperty>
    


    <!-- https://aphia.org/ns/taxon-name/authorship -->

    <owl:DatatypeProperty rdf:about="https://aphia.org/ns/taxon-name/authorship">
        <rdfs:subPropertyOf rdf:resource="http://rs.tdwg.org/dwc/terms/scientificNameAuthorship"/>
        <rdf:type rdf:resource="http://www.w3.org/2002/07/owl#FunctionalProperty"/>
        <rdfs:domain rdf:resource="https://aphia.org/ns/taxon-name/TaxonName"/>
        <rdfs:range rdf:resource="http://www.w3.org/1999/02/22-rdf-syntax-ns#PlainLiteral"/>
        <rdfs:comment xml:lang="it">Le informazioni sulla paternità del nome scientifico, espresse sottoforma di stringa, formattate secondo le convenzioni del codice nomenclaturale applicabile.</rdfs:comment>
        <rdfs:comment xml:lang="en">The authorship information, expressed as a string, for the scientific name, formatted according to the conventions of the applicable nomenclatural code.</rdfs:comment>
        <rdfs:comment xml:lang="nl">De auteursinformatie, uitgedrukt als een string, voor de wetenschappelijke naam, geformatteerd volgens de conventies van de toepasselijke nomenclatuurcode.</rdfs:comment>
        <rdfs:isDefinedBy rdf:resource="https://aphia.org/ns/taxon-name"/>
        <rdfs:label xml:lang="en">authorship</rdfs:label>
        <rdfs:label xml:lang="it">paternità</rdfs:label>
        <rdfs:label xml:lang="nl">auteurschap</rdfs:label>
    </owl:DatatypeProperty>
    


    <!-- https://aphia.org/ns/taxon-name/fullScientificName -->

    <owl:DatatypeProperty rdf:about="https://aphia.org/ns/taxon-name/fullScientificName">
        <rdfs:subPropertyOf rdf:resource="http://rs.tdwg.org/dwc/terms/scientificName"/>
        <rdfs:subPropertyOf rdf:resource="http://www.w3.org/2008/05/skos-xl#literalForm"/>
        <rdfs:domain rdf:resource="https://aphia.org/ns/taxon-name/TaxonName"/>
        <rdfs:range rdf:resource="http://www.w3.org/1999/02/22-rdf-syntax-ns#PlainLiteral"/>
        <rdfs:comment xml:lang="it">Il nome scientifico completo in latino che include anche la paternità, data dalla combinazione di autore e anno.</rdfs:comment>
        <rdfs:comment xml:lang="en">The complete scientific name in Latin including the authorship information (author, year).</rdfs:comment>
        <rdfs:comment xml:lang="nl">De volledige wetenschappelijke naam in het Latijn, met informatie over het auteurschap (auteur, jaar).</rdfs:comment>
        <rdfs:isDefinedBy rdf:resource="https://aphia.org/ns/taxon-name"/>
        <rdfs:label xml:lang="en">full scientific name (with author)</rdfs:label>
        <rdfs:label xml:lang="it">nome scientifico completo (con autore)</rdfs:label>
        <rdfs:label xml:lang="nl">volledige wetenschappelijke naam (met auteur)</rdfs:label>
    </owl:DatatypeProperty>
    


    <!-- https://aphia.org/ns/taxon-name/scientificName -->

    <owl:DatatypeProperty rdf:about="https://aphia.org/ns/taxon-name/scientificName">
        <rdfs:subPropertyOf rdf:resource="http://www.w3.org/2008/05/skos-xl#literalForm"/>
        <rdfs:domain rdf:resource="https://aphia.org/ns/taxon-name/TaxonName"/>
        <rdfs:range rdf:resource="http://www.w3.org/1999/02/22-rdf-syntax-ns#PlainLiteral"/>
        <rdfs:comment xml:lang="it">Il nome scientifico in latino che non include le informazioni sulla paternità (autore, anno)</rdfs:comment>
        <rdfs:comment xml:lang="en">The scientific name in Latin that does not include information on the authorship (author, year).</rdfs:comment>
        <rdfs:comment xml:lang="nl">De wetenschappelijke naam in het Latijn zonder informatie over het auteurschap (auteur, jaar)</rdfs:comment>
        <rdfs:isDefinedBy rdf:resource="https://aphia.org/ns/taxon-name"/>
        <rdfs:label xml:lang="it">nome scientifico (senza autore)</rdfs:label>
        <rdfs:label xml:lang="en">scientific name (without author)</rdfs:label>
        <rdfs:label xml:lang="nl">wetenschappelijke naam (zonder auteur)</rdfs:label>
    </owl:DatatypeProperty>
    


    <!-- https://aphia.org/ns/taxon-name/vernacularName -->

    <owl:DatatypeProperty rdf:about="https://aphia.org/ns/taxon-name/vernacularName">
        <rdfs:subPropertyOf rdf:resource="http://rs.tdwg.org/dwc/terms/vernacularName"/>
        <rdfs:subPropertyOf rdf:resource="http://www.w3.org/2008/05/skos-xl#literalForm"/>
        <rdfs:domain rdf:resource="https://aphia.org/ns/taxon-name/VernacularName"/>
        <rdfs:range rdf:resource="http://www.w3.org/1999/02/22-rdf-syntax-ns#PlainLiteral"/>
        <rdfs:comment xml:lang="it">Il nome comune espresso nelle varie lingue</rdfs:comment>
        <rdfs:comment xml:lang="en">The common name expressed in various languages.</rdfs:comment>
        <rdfs:comment xml:lang="nl">De inheemse/inlandse naam in verschillende talen.</rdfs:comment>
        <rdfs:isDefinedBy rdf:resource="https://aphia.org/ns/taxon-name"/>
        <rdfs:label xml:lang="it">nome comune</rdfs:label>
        <rdfs:label xml:lang="en">vernacular name</rdfs:label>
        <rdfs:label xml:lang="nl">vernaculaire naam</rdfs:label>
    </owl:DatatypeProperty>
    


    <!-- 
    ///////////////////////////////////////////////////////////////////////////////////////
    //
    // Classes
    //
    ///////////////////////////////////////////////////////////////////////////////////////
     -->

    


    <!-- http://purl.org/dc/terms/LinguisticSystem -->

    <owl:Class rdf:about="http://purl.org/dc/terms/LinguisticSystem"/>
    


    <!-- http://purl.org/dc/terms/Location -->

    <owl:Class rdf:about="http://purl.org/dc/terms/Location"/>
    


    <!-- http://www.ontologydesignpatterns.org/ont/dul/DUL.owl#Concept -->

    <owl:Class rdf:about="http://www.ontologydesignpatterns.org/ont/dul/DUL.owl#Concept"/>
    


    <!-- http://xmlns.com/foaf/0.1/Organization -->

    <owl:Class rdf:about="http://xmlns.com/foaf/0.1/Organization"/>
    


    <!-- https://aphia.org/ns/taxon-name/Rank -->

    <owl:Class rdf:about="https://aphia.org/ns/taxon-name/Rank">
        <rdfs:subClassOf rdf:resource="http://www.ontologydesignpatterns.org/ont/dul/DUL.owl#Concept"/>
        <rdfs:subClassOf rdf:resource="http://www.w3.org/2004/02/skos/core#Concept"/>
        <rdfs:comment xml:lang="it">Il livello specifico di una classificazione tassonomica che un nome occupa. Esempi sono: specie, famiglia, genere, sottospecie, ecc. Gli individui di questa classe possono essere concetti di un vocabolario controllato relativo.</rdfs:comment>
        <rdfs:comment xml:lang="en">The particular level in a taxonomic classification that a name occupies. Examples are: species, family, genus, subspecies, etc. The indivuals of this class can be concepts of a controlled vocabulary.</rdfs:comment>
        <rdfs:comment xml:lang="nl">Het specifieke niveau in een taxonomische classificatie die een naam inneemt. Voorbeelden zijn: soort, familie, geslacht, ondersoort, enz. De individuen van deze klasse kunnen concepten van een gecontroleerde woordenlijst zijn.</rdfs:comment>
        <rdfs:isDefinedBy rdf:resource="https://aphia.org/ns/taxon-name"/>
        <rdfs:label xml:lang="it">Rango</rdfs:label>
        <rdfs:label xml:lang="en">Rank</rdfs:label>
        <rdfs:label xml:lang="nl">Rang</rdfs:label>
    </owl:Class>
    


    <!-- https://aphia.org/ns/taxon-name/Status -->

    <owl:Class rdf:about="https://aphia.org/ns/taxon-name/Status">
        <rdfs:subClassOf rdf:resource="http://www.ontologydesignpatterns.org/ont/dul/DUL.owl#Concept"/>
        <rdfs:subClassOf rdf:resource="http://www.w3.org/2004/02/skos/core#Concept"/>
        <rdfs:comment xml:lang="it">Lo stato dell&apos;uso del nome del taxon (di solito un parere tassonomico).</rdfs:comment>
        <rdfs:comment xml:lang="en">The status of the use of the taxon name (usually a taxonomic opinion).</rdfs:comment>
        <rdfs:comment xml:lang="nl">De status van het gebruik van de taxonnaam (meestal een taxonomisch advies)</rdfs:comment>
        <rdfs:isDefinedBy rdf:resource="https://aphia.org/ns/taxon-name"/>
        <rdfs:label xml:lang="it">Stato</rdfs:label>
        <rdfs:label xml:lang="en">Status</rdfs:label>
        <rdfs:label xml:lang="nl">Status</rdfs:label>
    </owl:Class>
    


    <!-- https://aphia.org/ns/taxon-name/Taxon -->

    <owl:Class rdf:about="https://aphia.org/ns/taxon-name/Taxon">
        <rdfs:subClassOf rdf:resource="http://www.ontologydesignpatterns.org/ont/dul/DUL.owl#Concept"/>
        <rdfs:subClassOf rdf:resource="http://www.w3.org/2004/02/skos/core#Concept"/>
        <rdfs:subClassOf>
            <owl:Restriction>
                <owl:onProperty rdf:resource="https://aphia.org/ns/taxon-name/isDenotedBy"/>
                <owl:someValuesFrom rdf:resource="https://aphia.org/ns/top-level/Name"/>
            </owl:Restriction>
        </rdfs:subClassOf>
        <rdfs:subClassOf>
            <owl:Restriction>
                <owl:onProperty rdf:resource="http://purl.org/dc/terms/source"/>
                <owl:allValuesFrom rdf:resource="https://aphia.org/ns/top-level/Source"/>
            </owl:Restriction>
        </rdfs:subClassOf>
        <rdfs:subClassOf>
            <owl:Restriction>
                <owl:onProperty rdf:resource="https://aphia.org/ns/taxon-name/hasChild"/>
                <owl:allValuesFrom rdf:resource="https://aphia.org/ns/taxon-name/Taxon"/>
            </owl:Restriction>
        </rdfs:subClassOf>
        <rdfs:subClassOf>
            <owl:Restriction>
                <owl:onProperty rdf:resource="https://aphia.org/ns/taxon-name/isDenotedBy"/>
                <owl:allValuesFrom rdf:resource="https://aphia.org/ns/top-level/Name"/>
            </owl:Restriction>
        </rdfs:subClassOf>
        <rdfs:subClassOf>
            <owl:Restriction>
                <owl:onProperty rdf:resource="https://aphia.org/ns/taxon-name/hasParent"/>
                <owl:maxQualifiedCardinality rdf:datatype="http://www.w3.org/2001/XMLSchema#nonNegativeInteger">1</owl:maxQualifiedCardinality>
                <owl:onClass rdf:resource="https://aphia.org/ns/taxon-name/Taxon"/>
            </owl:Restriction>
        </rdfs:subClassOf>
        <owl:disjointWith rdf:resource="https://aphia.org/ns/top-level/Name"/>
        <rdfs:comment xml:lang="en">A group of organisms asserted by taxonomists to form a natural cohesive biological unit.</rdfs:comment>
        <rdfs:comment xml:lang="it">Un gruppo di organismi che, secondo i tassonomisti, formano un&apos;unità biologica naturale coesa.</rdfs:comment>
        <rdfs:comment xml:lang="nl">Een groep organismen die, volgens taxonomen, een natuurlijke samenhangende biologische eenheid vormen.</rdfs:comment>
        <rdfs:isDefinedBy rdf:resource="https://aphia.org/ns/taxon-name"/>
        <rdfs:label xml:lang="en">Taxon</rdfs:label>
        <rdfs:label xml:lang="it">Taxon</rdfs:label>
        <rdfs:label xml:lang="nl">Taxon</rdfs:label>
        <prov:wasDerivedFrom rdf:resource="http://rs.tdwg.org/dwc/terms/Taxon"/>
        <prov:wasDerivedFrom rdf:resource="https://schema.org/Taxon"/>
    </owl:Class>
    


    <!-- https://aphia.org/ns/taxon-name/TaxonName -->

    <owl:Class rdf:about="https://aphia.org/ns/taxon-name/TaxonName">
        <rdfs:subClassOf rdf:resource="http://www.w3.org/2008/05/skos-xl#Label"/>
        <rdfs:subClassOf rdf:resource="https://aphia.org/ns/top-level/Name"/>
        <rdfs:subClassOf>
            <owl:Restriction>
                <owl:onProperty rdf:resource="http://purl.org/dc/terms/source"/>
                <owl:allValuesFrom rdf:resource="https://aphia.org/ns/top-level/Source"/>
            </owl:Restriction>
        </rdfs:subClassOf>
        <rdfs:subClassOf>
            <owl:Restriction>
                <owl:onProperty rdf:resource="https://aphia.org/ns/taxon-name/hasSynonym"/>
                <owl:allValuesFrom rdf:resource="https://aphia.org/ns/taxon-name/TaxonName"/>
            </owl:Restriction>
        </rdfs:subClassOf>
        <rdfs:subClassOf>
            <owl:Restriction>
                <owl:onProperty rdf:resource="https://aphia.org/ns/taxon-name/isSynonymOf"/>
                <owl:allValuesFrom rdf:resource="https://aphia.org/ns/taxon-name/TaxonName"/>
            </owl:Restriction>
        </rdfs:subClassOf>
        <rdfs:subClassOf>
            <owl:Restriction>
                <owl:onProperty rdf:resource="https://aphia.org/ns/top-level/hasIdentifier"/>
                <owl:allValuesFrom rdf:resource="https://aphia.org/ns/top-level/Identifier"/>
            </owl:Restriction>
        </rdfs:subClassOf>
        <rdfs:subClassOf>
            <owl:Restriction>
                <owl:onProperty rdf:resource="https://aphia.org/ns/taxon-name/hasStatus"/>
                <owl:qualifiedCardinality rdf:datatype="http://www.w3.org/2001/XMLSchema#nonNegativeInteger">1</owl:qualifiedCardinality>
                <owl:onClass rdf:resource="https://aphia.org/ns/taxon-name/Status"/>
            </owl:Restriction>
        </rdfs:subClassOf>
        <rdfs:subClassOf>
            <owl:Restriction>
                <owl:onProperty rdf:resource="https://aphia.org/ns/taxon-name/isOfRank"/>
                <owl:qualifiedCardinality rdf:datatype="http://www.w3.org/2001/XMLSchema#nonNegativeInteger">1</owl:qualifiedCardinality>
                <owl:onClass rdf:resource="https://aphia.org/ns/taxon-name/Rank"/>
            </owl:Restriction>
        </rdfs:subClassOf>
        <rdfs:subClassOf>
            <owl:Restriction>
                <owl:onProperty rdf:resource="https://aphia.org/ns/taxon-name/hasUnacceptedReason"/>
                <owl:maxQualifiedCardinality rdf:datatype="http://www.w3.org/2001/XMLSchema#nonNegativeInteger">1</owl:maxQualifiedCardinality>
                <owl:onClass rdf:resource="https://aphia.org/ns/taxon-name/UnacceptedReason"/>
            </owl:Restriction>
        </rdfs:subClassOf>
        <rdfs:subClassOf>
            <owl:Restriction>
                <owl:onProperty rdf:resource="https://aphia.org/ns/taxon-name/aphiaID"/>
                <owl:cardinality rdf:datatype="http://www.w3.org/2001/XMLSchema#nonNegativeInteger">1</owl:cardinality>
            </owl:Restriction>
        </rdfs:subClassOf>
        <rdfs:subClassOf>
            <owl:Restriction>
                <owl:onProperty rdf:resource="https://aphia.org/ns/taxon-name/fullScientificName"/>
                <owl:qualifiedCardinality rdf:datatype="http://www.w3.org/2001/XMLSchema#nonNegativeInteger">1</owl:qualifiedCardinality>
                <owl:onDataRange rdf:resource="http://www.w3.org/1999/02/22-rdf-syntax-ns#PlainLiteral"/>
            </owl:Restriction>
        </rdfs:subClassOf>
        <rdfs:subClassOf>
            <owl:Restriction>
                <owl:onProperty rdf:resource="https://aphia.org/ns/taxon-name/authorship"/>
                <owl:maxQualifiedCardinality rdf:datatype="http://www.w3.org/2001/XMLSchema#nonNegativeInteger">1</owl:maxQualifiedCardinality>
                <owl:onDataRange rdf:resource="http://www.w3.org/1999/02/22-rdf-syntax-ns#PlainLiteral"/>
            </owl:Restriction>
        </rdfs:subClassOf>
        <rdfs:subClassOf>
            <owl:Restriction>
                <owl:onProperty rdf:resource="https://aphia.org/ns/taxon-name/scientificName"/>
                <owl:maxQualifiedCardinality rdf:datatype="http://www.w3.org/2001/XMLSchema#nonNegativeInteger">1</owl:maxQualifiedCardinality>
                <owl:onDataRange rdf:resource="http://www.w3.org/1999/02/22-rdf-syntax-ns#PlainLiteral"/>
            </owl:Restriction>
        </rdfs:subClassOf>
        <owl:disjointWith rdf:resource="https://aphia.org/ns/taxon-name/VernacularName"/>
        <rdfs:comment xml:lang="en">A name of a particular taxon of any rank (e.g., a genus, a species, a family, etc.). It may be accepted/valid or not. The taxon author is frequently included when indicating a taxon name, as it can help distinguish between different uses of the same name (such as homonyms).</rdfs:comment>
        <rdfs:comment xml:lang="it">Nome di un particolare taxon di qualsiasi rango (ad esempio, un genere, una specie, una famiglia, ecc.). Può essere accettato/valido o meno. L&apos;autore del taxon è spesso incluso quando si indica un nome di taxon, in quanto può aiutare a distinguere tra diversi usi dello stesso nome (come gli omonimi).</rdfs:comment>
        <rdfs:comment xml:lang="nl">Een naam van een bepaald taxon van om het even welke rang (bv. een genus, een soort, een familie, enz.). Deze kan geaccepteerd/geldig zijn of niet. De taxonauteur wordt vaak vermeld bij het aangeven van een taxonnaam, omdat het kan helpen onderscheid te maken tussen verschillende toepassingen van dezelfde naam (zoals homoniemen).</rdfs:comment>
        <rdfs:isDefinedBy rdf:resource="https://aphia.org/ns/taxon-name"/>
        <rdfs:label xml:lang="it">Nome del Taxon</rdfs:label>
        <rdfs:label xml:lang="en">Taxon Name</rdfs:label>
        <rdfs:label xml:lang="nl">Taxon Naam</rdfs:label>
        <prov:wasDerivedFrom rdf:resource="http://openbiodiv.net/LatinName"/>
        <prov:wasDerivedFrom rdf:resource="http://rs.tdwg.org/ontology/voc/TaxonName#TaxonName"/>
        <prov:wasDerivedFrom rdf:resource="https://discovery.biothings.io/view/bioschemas/TaxonName"/>
    </owl:Class>
    


    <!-- https://aphia.org/ns/taxon-name/UnacceptedReason -->

    <owl:Class rdf:about="https://aphia.org/ns/taxon-name/UnacceptedReason">
        <rdfs:subClassOf rdf:resource="http://www.ontologydesignpatterns.org/ont/dul/DUL.owl#Concept"/>
        <rdfs:subClassOf rdf:resource="http://www.w3.org/2004/02/skos/core#Concept"/>
        <rdfs:comment xml:lang="en">An explanation regarding why a given taxon name is judged to be invalid or not accepted. The individuals of this class can be concepts of a specific controlled vocabulary with values like: synonym, misapplied, original combination, new combination, etc.</rdfs:comment>
        <rdfs:comment xml:lang="it">Motivazione per cui un nome di un determinato taxon viene giudicato non accettato o non valido. Gli individui di questa classe possono essere concetti di uno specifico vocabolario controllato con valori come: sinonimo, errata applicazione, combinazione originale, nuova combinazione, ecc.</rdfs:comment>
        <rdfs:comment xml:lang="nl">Een motivatie/uitleg waarom een bepaalde taxonnaam ongeldig of niet geaccepteerd wordt geacht. De individuen van deze klasse kunnen concepten zijn van een specifieke gecontroleerde vocabularium met waarden als: synoniem, verkeerd toegepast, originele combinatie, nieuwe combinatie, enz.</rdfs:comment>
        <rdfs:isDefinedBy rdf:resource="https://aphia.org/ns/taxon-name"/>
        <rdfs:label xml:lang="it">Motivo per non Accettato</rdfs:label>
        <rdfs:label xml:lang="en">Unaccepted Reason</rdfs:label>
        <rdfs:label xml:lang="nl">Niet-geaccepteerd Reden</rdfs:label>
    </owl:Class>
    


    <!-- https://aphia.org/ns/taxon-name/VernacularName -->

    <owl:Class rdf:about="https://aphia.org/ns/taxon-name/VernacularName">
        <rdfs:subClassOf rdf:resource="https://aphia.org/ns/top-level/Name"/>
        <rdfs:subClassOf>
            <owl:Restriction>
                <owl:onProperty rdf:resource="http://purl.org/dc/terms/coverage"/>
                <owl:allValuesFrom rdf:resource="http://purl.org/dc/terms/Location"/>
            </owl:Restriction>
        </rdfs:subClassOf>
        <rdfs:subClassOf>
            <owl:Restriction>
                <owl:onProperty rdf:resource="http://purl.org/dc/terms/language"/>
                <owl:allValuesFrom rdf:resource="http://purl.org/dc/terms/LinguisticSystem"/>
            </owl:Restriction>
        </rdfs:subClassOf>
        <rdfs:subClassOf>
            <owl:Restriction>
                <owl:onProperty rdf:resource="http://purl.org/dc/terms/source"/>
                <owl:allValuesFrom rdf:resource="https://aphia.org/ns/top-level/Source"/>
            </owl:Restriction>
        </rdfs:subClassOf>
        <rdfs:subClassOf>
            <owl:Restriction>
                <owl:onProperty rdf:resource="https://aphia.org/ns/taxon-name/vernacularName"/>
                <owl:allValuesFrom rdf:resource="http://www.w3.org/1999/02/22-rdf-syntax-ns#PlainLiteral"/>
            </owl:Restriction>
        </rdfs:subClassOf>
        <rdfs:comment xml:lang="en">A name other than a taxon name (scientific name) that is commonly used to refer to a species or other taxon. Examples are salmon, rainbow trout, acciuga etc. The language (e.g., English, Italian, etc.) is usually indicated for each vernacular name.</rdfs:comment>
        <rdfs:comment xml:lang="it">Un nome diverso dal nome del taxon (nome scientifico) che viene comunemente usato per indicare una specie o un altro taxon. Esempi sono il salmone, la trota iridea, l&apos;acciuga ecc. Per ogni nome comune viene solitamente indicata la lingua (ad esempio, inglese, italiano, ecc.).</rdfs:comment>
        <rdfs:comment xml:lang="nl">Een naam, anders dan een taxonnaam (wetenschappelijke naam), die algemeen gebruikt wordt om te verwijzen naar een soort of ander taxon. Voorbeelden zijn zalm, regenboogforel, acciuga enz. De taal (bijv. Engels, Italiaans, enz.) wordt meestal aangegeven voor elke vernaculaire naam.</rdfs:comment>
        <rdfs:isDefinedBy rdf:resource="https://aphia.org/ns/taxon-name"/>
        <rdfs:label xml:lang="it">Nome Comune</rdfs:label>
        <rdfs:label xml:lang="en">Vernacular Name</rdfs:label>
        <rdfs:label xml:lang="nl">Vernaculaire naam</rdfs:label>
    </owl:Class>
    


    <!-- https://aphia.org/ns/top-level/Identifier -->

    <owl:Class rdf:about="https://aphia.org/ns/top-level/Identifier"/>
    


    <!-- https://aphia.org/ns/top-level/IdentifierType -->

    <owl:Class rdf:about="https://aphia.org/ns/top-level/IdentifierType"/>
    


    <!-- https://aphia.org/ns/top-level/Name -->

    <owl:Class rdf:about="https://aphia.org/ns/top-level/Name"/>
    


    <!-- https://aphia.org/ns/top-level/Source -->

    <owl:Class rdf:about="https://aphia.org/ns/top-level/Source"/>
    


    <!-- https://aphia.org/ns/top-level/System -->

    <owl:Class rdf:about="https://aphia.org/ns/top-level/System"/>
    


    <!-- 
    ///////////////////////////////////////////////////////////////////////////////////////
    //
    // Individuals
    //
    ///////////////////////////////////////////////////////////////////////////////////////
     -->

    


    <!-- https://aphia.org/resource/organisation/dv -->

    <owl:NamedIndividual rdf:about="https://aphia.org/resource/organisation/dv">
        <rdf:type rdf:resource="http://xmlns.com/foaf/0.1/Organization"/>
        <rdfs:label xml:lang="nl">Digitaal Vlaanderen</rdfs:label>
        <rdfs:label xml:lang="en">Digital Flanders</rdfs:label>
        <foaf:name xml:lang="nl">Digitaal Vlaanderen</foaf:name>
        <foaf:name xml:lang="en">Digital Flanders</foaf:name>
    </owl:NamedIndividual>
</rdf:RDF>



<!-- Generated by the OWL API (version 4.5.26.2023-07-17T20:34:13Z) https://github.com/owlcs/owlapi -->

