<?xml version="1.0"?>
<rdf:RDF xmlns="https://w3id.org/marine/ns/distribution/"
     xml:base="https://w3id.org/marine/ns/distribution/"
     xmlns:dc="http://purl.org/dc/elements/1.1/"
     xmlns:dct="http://purl.org/dc/terms/"
     xmlns:owl="http://www.w3.org/2002/07/owl#"
     xmlns:rdf="http://www.w3.org/1999/02/22-rdf-syntax-ns#"
     xmlns:xml="http://www.w3.org/XML/1998/namespace"
     xmlns:xsd="http://www.w3.org/2001/XMLSchema#"
     xmlns:foaf="http://xmlns.com/foaf/0.1/"
     xmlns:prov="http://www.w3.org/ns/prov#"
     xmlns:rdfs="http://www.w3.org/2000/01/rdf-schema#"
     xmlns:skos="http://www.w3.org/2004/02/skos/core#">
    <owl:Ontology rdf:about="https://w3id.org/marine/ns/distribution">
        <owl:versionIRI rdf:resource="https://w3id.org/marine/ns/distribution/0.1"/>
        <owl:imports rdf:resource="https://w3id.org/marine/ns/top-level/0.1"/>
        <dct:creator rdf:resource="https://w3id.org/italia/data/organization/support-unit/cnr-Z6HZEH/stlab"/>
        <dct:creator rdf:resource="https://w3id.org/marine/resource/organisation/dv"/>
        <dct:creator rdf:resource="https://w3id.org/marine/resource/organisation/vliz"/>
        <dct:description xml:lang="it">Questa è l&apos;ontologia della distribuzione (delle specie) della rete di ontologie MAREGRAPH. Importa l&apos;ontologia di primo livello della rete MAREGRAPH e definisce la distribuzione documentata delle specie come riportata nel database WoRMS. La distribuzione è descritta in base a diverse tipologie di informazioni: la posizione geografica, utilizzando il nome del luogo o la latitudine e la longitudine quando è possibile identificare singoli punti, la fonte da cui è documentata la distribuzione, l&apos;origine della specie, l&apos;invasività della specie, la presenza. È inoltre possibile indicare se la distribuzione è segnalata come &apos;località tipo&apos; della specie. L&apos;ontologia usa l&apos;ontologia delle regioni marine per rappresentare le posizioni geografiche.</dct:description>
        <dct:description xml:lang="en">This is the (species) distribution ontology of the MAREGRAPH network of ontologies. It imports the top-level ontology of the MAREGRAPH network and it defines the documented distribution of the species as defined in the WoRMS database. The distribution is described according to various information: the geographical location, using the place name or latitude and longitude when single points can be identified, the source from which the distribution is documented, the origin of the species, the invasiveness of the species, the occurrence. It is also possible to indicate whether the distribution is marked as a type locality of the species. The ontology uses the Marine Region ontology for representing geographical locations</dct:description>
        <dct:issued rdf:datatype="http://www.w3.org/2001/XMLSchema#date">2023-08-30</dct:issued>
        <dct:language rdf:resource="http://publications.europa.eu/resource/authority/language/ENG"/>
        <dct:language rdf:resource="http://publications.europa.eu/resource/authority/language/ITA"/>
        <dct:language rdf:resource="http://publications.europa.eu/resource/authority/language/NLD"/>
        <dct:license rdf:resource="http://publications.europa.eu/resource/authority/licence/CC_BY_4_0"/>
        <dct:modified rdf:datatype="http://www.w3.org/2001/XMLSchema#date">2023-11-29</dct:modified>
        <dct:title xml:lang="en">MAREGRAPH - (Species) Distribution ontology</dct:title>
        <dct:title xml:lang="it">MAREGRAPH - Ontologia sulla Distribuzione delle Specie</dct:title>
        <dct:title xml:lang="nl">MAREGRAPH - (Soorten) Verspreidingsontologie</dct:title>
        <rdfs:comment xml:lang="it">Questa è l&apos;ontologia della distribuzione (delle specie) della rete di ontologie MAREGRAPH. Importa l&apos;ontologia di primo livello della rete MAREGRAPH e definisce la distribuzione documentata delle specie come riportata nel database WoRMS. La distribuzione è descritta in base a diverse tipologie di informazioni: la posizione geografica, utilizzando il nome del luogo o la latitudine e la longitudine quando è possibile identificare singoli punti, la fonte da cui è documentata la distribuzione, l&apos;origine della specie, l&apos;invasività della specie, la presenza. È inoltre possibile indicare se la distribuzione è segnalata come &apos;località tipo&apos; della specie. L&apos;ontologia usa l&apos;ontologia delle regioni marine per rappresentare le posizioni geografiche.</rdfs:comment>
        <rdfs:comment xml:lang="en">This is the (species) distribution ontology of the MAREGRAPH network of ontologies. It imports the top-level ontology of the MAREGRAPH network and it defines the documented distribution of the species as defined in the WoRMS database. The distribution is described according to various information: the geographical location, using the place name or latitude and longitude when single points can be identified, the source from which the distribution is documented, the origin of the species, the invasiveness of the species, the occurrence. It is also possible to indicate whether the distribution is marked as a type locality of the species. The ontology uses the Marine Region ontology for representing geographical locations</rdfs:comment>
        <rdfs:comment xml:lang="nl">Dit is de (soorten) verspreidingsontologie van het MAREGRAPH-netwerk van ontologieën. De ontologie importeert de overkoepelende ontologie van het MAREGRAPH-netwerk en definieert de gedocumenteerde verspreiding van de soorten zoals gedefinieerd in de WoRMS-database. De verspreiding wordt beschreven aan de hand van verschillende informatie: de geografische locatie, met behulp van de plaatsnaam of de lengte- en breedtegraad wanneer afzonderlijke punten kunnen worden geïdentificeerd, de literaire bron van waaruit de verspreiding is gedocumenteerd, de herkomst van de soort, de invasiviteit van de soort, het voorkomen. Het is ook mogelijk om aan te geven of de verspreiding is gemarkeerd als een type localiteit van de soort. De ontologie maakt gebruik van de Marine Regions ontologie om geografische locaties weer te geven.</rdfs:comment>
        <rdfs:label xml:lang="en">MAREGRAPH - (Species) Distribution ontology</rdfs:label>
        <rdfs:label xml:lang="it">MAREGRAPH - Ontologia sulla Distribuzione delle Specie</rdfs:label>
        <rdfs:label xml:lang="nl">MAREGRAPH - (Soorten) Verspreidingsontologie</rdfs:label>
        <owl:versionInfo xml:lang="en">Preliminary version 0.1</owl:versionInfo>
        <owl:versionInfo xml:lang="it">Versione preliminare 0.1</owl:versionInfo>
        <owl:versionInfo xml:lang="nl">Voorlopige versie 0.1</owl:versionInfo>
    </owl:Ontology>
    


    <!-- 
    ///////////////////////////////////////////////////////////////////////////////////////
    //
    // Annotation properties
    //
    ///////////////////////////////////////////////////////////////////////////////////////
     -->

    


    <!-- http://purl.org/dc/terms/language -->

    <owl:AnnotationProperty rdf:about="http://purl.org/dc/terms/language"/>
    


    <!-- http://purl.org/dc/terms/license -->

    <owl:AnnotationProperty rdf:about="http://purl.org/dc/terms/license"/>
    


    <!-- http://www.w3.org/ns/prov#wasDerivedFrom -->

    <owl:AnnotationProperty rdf:about="http://www.w3.org/ns/prov#wasDerivedFrom"/>
    


    <!-- 
    ///////////////////////////////////////////////////////////////////////////////////////
    //
    // Object Properties
    //
    ///////////////////////////////////////////////////////////////////////////////////////
     -->

    


    <!-- http://www.w3.org/ns/locn#geometry -->

    <owl:ObjectProperty rdf:about="http://www.w3.org/ns/locn#geometry"/>
    


    <!-- https://w3id.org/marine/ns/distribution/hasArea -->

    <owl:ObjectProperty rdf:about="https://w3id.org/marine/ns/distribution/hasArea">
        <rdfs:subPropertyOf rdf:resource="http://www.ontologydesignpatterns.org/ont/dul/DUL.owl#hasLocation"/>
        <rdfs:domain rdf:resource="https://w3id.org/marine/ns/distribution/Distribution"/>
        <rdfs:range rdf:resource="http://marineregions.org/ns/ontology#MRGeoObject"/>
        <rdfs:comment xml:lang="en">Property used to represent the geographical unit of the distribution of the species. The geographical units are specified using the Marine Region gazetteer.</rdfs:comment>
        <rdfs:comment xml:lang="it">Proprietà utilizzata per rappresentare l&apos;unità geografica di distribuzione della specie. Le unità geografiche sono specificate utilizzando il glossario delle regioni marine.</rdfs:comment>
        <rdfs:isDefinedBy rdf:resource="https://w3id.org/marine/ns/distribution"/>
        <rdfs:label xml:lang="it">ha area</rdfs:label>
        <rdfs:label xml:lang="en">has area</rdfs:label>
    </owl:ObjectProperty>
    


    <!-- https://w3id.org/marine/ns/distribution/hasDistribution -->

    <owl:ObjectProperty rdf:about="https://w3id.org/marine/ns/distribution/hasDistribution">
        <rdfs:subPropertyOf rdf:resource="http://www.ontologydesignpatterns.org/ont/dul/DUL.owl#associatedWith"/>
        <owl:inverseOf rdf:resource="https://w3id.org/marine/ns/distribution/isDistributionOf"/>
        <rdfs:domain rdf:resource="https://w3id.org/marine/ns/taxon-name/Taxon"/>
        <rdfs:range rdf:resource="https://w3id.org/marine/ns/distribution/Distribution"/>
        <rdfs:comment xml:lang="en">Property used to specify the distribution for a taxon.</rdfs:comment>
        <rdfs:comment xml:lang="it">Proprietà utilizzata per specificare la distribuzione di un taxon.</rdfs:comment>
        <rdfs:isDefinedBy rdf:resource="https://w3id.org/marine/ns/distribution"/>
        <rdfs:label xml:lang="it">ha distribuzione</rdfs:label>
        <rdfs:label xml:lang="en">has distribution</rdfs:label>
    </owl:ObjectProperty>
    


    <!-- https://w3id.org/marine/ns/distribution/hasInvasiveness -->

    <owl:ObjectProperty rdf:about="https://w3id.org/marine/ns/distribution/hasInvasiveness">
        <rdfs:subPropertyOf rdf:resource="http://www.ontologydesignpatterns.org/ont/dul/DUL.owl#associatedWith"/>
        <rdfs:domain rdf:resource="https://w3id.org/marine/ns/distribution/Distribution"/>
        <rdfs:range rdf:resource="https://w3id.org/marine/ns/distribution/Invasiveness"/>
        <rdfs:comment xml:lang="en">Property used to represent the invasiveness of the species in its documented distribution.</rdfs:comment>
        <rdfs:comment xml:lang="it">Proprietà utilizzata per rappresentare la proponsione all&apos;invasività della specie nella sua distribuzione documentata.</rdfs:comment>
        <rdfs:isDefinedBy rdf:resource="https://w3id.org/marine/ns/distribution"/>
        <rdfs:label xml:lang="it">ha invasività</rdfs:label>
        <rdfs:label xml:lang="en">has invasiveness</rdfs:label>
    </owl:ObjectProperty>
    


    <!-- https://w3id.org/marine/ns/distribution/hasOccurrence -->

    <owl:ObjectProperty rdf:about="https://w3id.org/marine/ns/distribution/hasOccurrence">
        <rdfs:subPropertyOf rdf:resource="http://www.ontologydesignpatterns.org/ont/dul/DUL.owl#associatedWith"/>
        <rdfs:domain rdf:resource="https://w3id.org/marine/ns/distribution/Distribution"/>
        <rdfs:range rdf:resource="https://w3id.org/marine/ns/distribution/Occurrence"/>
        <rdfs:comment xml:lang="en">Property used to represent the occurrence of the species in its documented distribution.</rdfs:comment>
        <rdfs:comment xml:lang="it">Proprietà utilizzata per rappresentare la presenza della specie nella sua distribuzione documentata.</rdfs:comment>
        <rdfs:isDefinedBy rdf:resource="https://w3id.org/marine/ns/distribution"/>
        <rdfs:label xml:lang="it">ha presenza</rdfs:label>
        <rdfs:label xml:lang="en">has occurrence</rdfs:label>
    </owl:ObjectProperty>
    


    <!-- https://w3id.org/marine/ns/distribution/hasOrigin -->

    <owl:ObjectProperty rdf:about="https://w3id.org/marine/ns/distribution/hasOrigin">
        <rdfs:subPropertyOf rdf:resource="http://www.ontologydesignpatterns.org/ont/dul/DUL.owl#associatedWith"/>
        <rdfs:domain rdf:resource="https://w3id.org/marine/ns/distribution/Distribution"/>
        <rdfs:range rdf:resource="https://w3id.org/marine/ns/distribution/Origin"/>
        <rdfs:comment xml:lang="en">Property used to represent the origin of the species in its documented distribution.</rdfs:comment>
        <rdfs:comment xml:lang="it">Proprietà utilizzata per rappresentare l&apos;origine della specie nella sua distribuzione documentata.</rdfs:comment>
        <rdfs:isDefinedBy rdf:resource="https://w3id.org/marine/ns/distribution"/>
        <rdfs:label xml:lang="it">ha origine</rdfs:label>
        <rdfs:label xml:lang="en">has origin</rdfs:label>
    </owl:ObjectProperty>
    


    <!-- https://w3id.org/marine/ns/distribution/isDistributionOf -->

    <owl:ObjectProperty rdf:about="https://w3id.org/marine/ns/distribution/isDistributionOf">
        <rdfs:subPropertyOf rdf:resource="http://www.ontologydesignpatterns.org/ont/dul/DUL.owl#associatedWith"/>
        <rdfs:domain rdf:resource="https://w3id.org/marine/ns/distribution/Distribution"/>
        <rdfs:range rdf:resource="https://w3id.org/marine/ns/taxon-name/Taxon"/>
        <rdfs:comment xml:lang="en">Inverse property of &apos;has distribution&apos; used to obtain information of the taxon from its distributions</rdfs:comment>
        <rdfs:comment xml:lang="it">Proprietà inversa di &apos;ha distribuzione&apos; usata per ottenere informazioni sul taxon dalle sue distribuzioni</rdfs:comment>
        <rdfs:isDefinedBy rdf:resource="https://w3id.org/marine/ns/distribution"/>
        <rdfs:label xml:lang="en">is distribution of</rdfs:label>
        <rdfs:label xml:lang="it">è distribuzione di</rdfs:label>
    </owl:ObjectProperty>
    


    <!-- 
    ///////////////////////////////////////////////////////////////////////////////////////
    //
    // Data properties
    //
    ///////////////////////////////////////////////////////////////////////////////////////
     -->

    


    <!-- http://www.w3.org/2004/02/skos/core#note -->

    <owl:DatatypeProperty rdf:about="http://www.w3.org/2004/02/skos/core#note"/>
    


    <!-- https://w3id.org/marine/ns/distribution/isTypeLocality -->

    <owl:DatatypeProperty rdf:about="https://w3id.org/marine/ns/distribution/isTypeLocality">
        <rdf:type rdf:resource="http://www.w3.org/2002/07/owl#FunctionalProperty"/>
        <rdfs:domain rdf:resource="https://w3id.org/marine/ns/distribution/Distribution"/>
        <rdfs:range rdf:resource="http://www.w3.org/2001/XMLSchema#boolean"/>
        <rdfs:comment xml:lang="en">Property used to mark mark a distribution as the type locality of the species.</rdfs:comment>
        <rdfs:comment xml:lang="it">Proprietà utilizzata per contrassegnare una distribuzione come &apos;località tipo&apos; della specie.</rdfs:comment>
        <rdfs:isDefinedBy rdf:resource="https://w3id.org/marine/ns/distribution"/>
        <rdfs:label xml:lang="en">is type locality</rdfs:label>
        <rdfs:label xml:lang="it">è tipo località</rdfs:label>
    </owl:DatatypeProperty>
    


    <!-- 
    ///////////////////////////////////////////////////////////////////////////////////////
    //
    // Classes
    //
    ///////////////////////////////////////////////////////////////////////////////////////
     -->

    


    <!-- http://marineregions.org/ns/ontology#MRGeoObject -->

    <owl:Class rdf:about="http://marineregions.org/ns/ontology#MRGeoObject"/>
    


    <!-- http://www.w3.org/ns/locn#Geometry -->

    <owl:Class rdf:about="http://www.w3.org/ns/locn#Geometry"/>
    


    <!-- https://w3id.org/marine/ns/distribution/Distribution -->

    <owl:Class rdf:about="https://w3id.org/marine/ns/distribution/Distribution">
        <rdfs:subClassOf rdf:resource="http://www.ontologydesignpatterns.org/ont/dul/DUL.owl#Situation"/>
        <rdfs:subClassOf>
            <owl:Restriction>
                <owl:onProperty rdf:resource="https://w3id.org/marine/ns/distribution/hasArea"/>
                <owl:someValuesFrom rdf:resource="http://marineregions.org/ns/ontology#MRGeoObject"/>
            </owl:Restriction>
        </rdfs:subClassOf>
        <rdfs:subClassOf>
            <owl:Restriction>
                <owl:onProperty rdf:resource="https://w3id.org/marine/ns/distribution/isDistributionOf"/>
                <owl:someValuesFrom rdf:resource="https://w3id.org/marine/ns/taxon-name/Taxon"/>
            </owl:Restriction>
        </rdfs:subClassOf>
        <rdfs:subClassOf>
            <owl:Restriction>
                <owl:onProperty rdf:resource="http://purl.org/dc/terms/source"/>
                <owl:allValuesFrom rdf:resource="https://w3id.org/marine/ns/top-level/Source"/>
            </owl:Restriction>
        </rdfs:subClassOf>
        <rdfs:subClassOf>
            <owl:Restriction>
                <owl:onProperty rdf:resource="http://www.w3.org/ns/locn#geometry"/>
                <owl:allValuesFrom rdf:resource="http://www.w3.org/ns/locn#Geometry"/>
            </owl:Restriction>
        </rdfs:subClassOf>
        <rdfs:subClassOf>
            <owl:Restriction>
                <owl:onProperty rdf:resource="https://w3id.org/marine/ns/distribution/hasArea"/>
                <owl:allValuesFrom rdf:resource="http://marineregions.org/ns/ontology#MRGeoObject"/>
            </owl:Restriction>
        </rdfs:subClassOf>
        <rdfs:subClassOf>
            <owl:Restriction>
                <owl:onProperty rdf:resource="https://w3id.org/marine/ns/distribution/hasInvasiveness"/>
                <owl:allValuesFrom rdf:resource="https://w3id.org/marine/ns/distribution/Invasiveness"/>
            </owl:Restriction>
        </rdfs:subClassOf>
        <rdfs:subClassOf>
            <owl:Restriction>
                <owl:onProperty rdf:resource="https://w3id.org/marine/ns/distribution/hasOccurrence"/>
                <owl:allValuesFrom rdf:resource="https://w3id.org/marine/ns/distribution/Occurrence"/>
            </owl:Restriction>
        </rdfs:subClassOf>
        <rdfs:subClassOf>
            <owl:Restriction>
                <owl:onProperty rdf:resource="https://w3id.org/marine/ns/distribution/hasOrigin"/>
                <owl:allValuesFrom rdf:resource="https://w3id.org/marine/ns/distribution/Origin"/>
            </owl:Restriction>
        </rdfs:subClassOf>
        <rdfs:subClassOf>
            <owl:Restriction>
                <owl:onProperty rdf:resource="https://w3id.org/marine/ns/distribution/isDistributionOf"/>
                <owl:allValuesFrom rdf:resource="https://w3id.org/marine/ns/taxon-name/Taxon"/>
            </owl:Restriction>
        </rdfs:subClassOf>
        <rdfs:subClassOf>
            <owl:Restriction>
                <owl:onProperty rdf:resource="http://www.w3.org/2004/02/skos/core#note"/>
                <owl:allValuesFrom rdf:resource="http://www.w3.org/1999/02/22-rdf-syntax-ns#PlainLiteral"/>
            </owl:Restriction>
        </rdfs:subClassOf>
        <rdfs:subClassOf>
            <owl:Restriction>
                <owl:onProperty rdf:resource="https://w3id.org/marine/ns/distribution/isTypeLocality"/>
                <owl:maxQualifiedCardinality rdf:datatype="http://www.w3.org/2001/XMLSchema#nonNegativeInteger">1</owl:maxQualifiedCardinality>
                <owl:onDataRange rdf:resource="http://www.w3.org/2001/XMLSchema#boolean"/>
            </owl:Restriction>
        </rdfs:subClassOf>
        <rdfs:comment xml:lang="it">Distribuzione geografica di presenza di specie marine e vegetali</rdfs:comment>
        <rdfs:comment xml:lang="en">Geographical distribution of occurrence of marine and plant species</rdfs:comment>
        <rdfs:isDefinedBy rdf:resource="https://w3id.org/marine/ns/distribution"/>
        <rdfs:label xml:lang="en">Distribution</rdfs:label>
        <rdfs:label xml:lang="it">Distribuzione</rdfs:label>
        <prov:wasDerivedFrom rdf:resource="http://inspire.ec.europa.eu/theme/sd"/>
    </owl:Class>
    


    <!-- https://w3id.org/marine/ns/distribution/Invasiveness -->

    <owl:Class rdf:about="https://w3id.org/marine/ns/distribution/Invasiveness">
        <rdfs:subClassOf rdf:resource="http://www.ontologydesignpatterns.org/ont/dul/DUL.owl#Concept"/>
        <rdfs:comment xml:lang="it">Questa classe rappresenta la propensione di una specie introdotta a invadere un ecosistema ricevente. Gli individui di questa classe sono rappresentati dai concetti del relativo vocabolario controllato che sono: Invasiva, Invasività non specificata, Invasività incerta, Gestione registrata, Non invasiva, Preoccupante.</rdfs:comment>
        <rdfs:comment xml:lang="en">This class represents the propensity of an introduced species to invade a recipient ecosystem. The individuals of this class are represented by the concepts of the related controlled vocabulary that are: Invasive, Invasiveness Not Specified, Invasiveness Uncertain, Management recorded, Not invasive, Of concern.</rdfs:comment>
        <rdfs:isDefinedBy rdf:resource="https://w3id.org/marine/ns/distribution"/>
        <rdfs:label xml:lang="en">Invasiveness</rdfs:label>
        <rdfs:label xml:lang="it">Invasività</rdfs:label>
        <prov:wasDerivedFrom rdf:resource="http://www.w3.org/2004/02/skos/core#Concept"/>
    </owl:Class>
    


    <!-- https://w3id.org/marine/ns/distribution/Occurrence -->

    <owl:Class rdf:about="https://w3id.org/marine/ns/distribution/Occurrence">
        <rdfs:subClassOf rdf:resource="http://www.ontologydesignpatterns.org/ont/dul/DUL.owl#Concept"/>
        <rdfs:comment xml:lang="it">Questa classe rappresenta la presenza di specie in località di interesse. Gli individui di questa classe sono rappresentati dai concetti del relativo vocabolario controllato.</rdfs:comment>
        <rdfs:comment xml:lang="en">This class represents the presence of species at locations of interest. The individuals of this class are represented by the concepts of the related controlled vocabulary.</rdfs:comment>
        <rdfs:isDefinedBy rdf:resource="https://w3id.org/marine/ns/distribution"/>
        <rdfs:label xml:lang="it">Occorrenza</rdfs:label>
        <rdfs:label xml:lang="en">Occurrence</rdfs:label>
        <prov:wasDerivedFrom rdf:resource="http://www.w3.org/2004/02/skos/core#Concept"/>
    </owl:Class>
    


    <!-- https://w3id.org/marine/ns/distribution/Origin -->

    <owl:Class rdf:about="https://w3id.org/marine/ns/distribution/Origin">
        <rdfs:subClassOf rdf:resource="http://www.ontologydesignpatterns.org/ont/dul/DUL.owl#Concept"/>
        <rdfs:comment xml:lang="it">L&apos;origine della specie introdotta. Gli individui di questa classe sono rappresentati dai concetti del relativo vocabolario controllato che sono: Aliena, Autoctona, Autoctona - Endemica, Autoctona - Non endemica, Origine incerta, Origine sconosciuta.</rdfs:comment>
        <rdfs:comment xml:lang="en">The origin of the introduced species. The individuals of this class are represented by the concepts of the related controlled vocabulary that are: Alien, Native, Native – Endemic, Native - Non-endemic, Origin uncertain, Origin unknown.</rdfs:comment>
        <rdfs:isDefinedBy rdf:resource="https://w3id.org/marine/ns/distribution"/>
        <rdfs:label xml:lang="en">Origin</rdfs:label>
        <rdfs:label xml:lang="it">Origine</rdfs:label>
        <prov:wasDerivedFrom rdf:resource="http://www.w3.org/2004/02/skos/core#Concept"/>
    </owl:Class>
    


    <!-- https://w3id.org/marine/ns/taxon-name/Taxon -->

    <owl:Class rdf:about="https://w3id.org/marine/ns/taxon-name/Taxon"/>
    


    <!-- 
    ///////////////////////////////////////////////////////////////////////////////////////
    //
    // Individuals
    //
    ///////////////////////////////////////////////////////////////////////////////////////
     -->

    


    <!-- https://w3id.org/marine/resource/organisation/dv -->

    <owl:NamedIndividual rdf:about="https://w3id.org/marine/resource/organisation/dv">
        <rdf:type rdf:resource="http://xmlns.com/foaf/0.1/Organization"/>
        <rdfs:label xml:lang="nl">Digitaal Vlaanderen</rdfs:label>
        <rdfs:label xml:lang="en">Digital Flanders</rdfs:label>
        <foaf:name xml:lang="nl">Digitaal Vlaanderen</foaf:name>
        <foaf:name xml:lang="en">Digital Flanders</foaf:name>
    </owl:NamedIndividual>
    


    <!-- https://w3id.org/marine/resource/organisation/vliz -->

    <owl:NamedIndividual rdf:about="https://w3id.org/marine/resource/organisation/vliz">
        <rdf:type rdf:resource="http://xmlns.com/foaf/0.1/Organization"/>
        <rdfs:label xml:lang="en">Flanders Marine Institute</rdfs:label>
        <rdfs:label xml:lang="it">Istituto marino delle Fiandre</rdfs:label>
        <rdfs:label xml:lang="nl">Vlaams Instituut voor de Zee</rdfs:label>
        <foaf:name xml:lang="en">Flanders Marine Institute</foaf:name>
        <foaf:name xml:lang="it">Istituto marino delle Fiandre</foaf:name>
        <foaf:name xml:lang="nl">Vlaams Instituut voor de Zee</foaf:name>
    </owl:NamedIndividual>
</rdf:RDF>



<!-- Generated by the OWL API (version 4.5.26.2023-07-17T20:34:13Z) https://github.com/owlcs/owlapi -->

